# BSD 3-Clause License
#
# Copyright (c) 2021, gabrieljlsantos
# All rights reserved.
#
# Redistribution and use in source and binary forms, with or without
# modification, are permitted provided that the following conditions are met:
#
# 1. Redistributions of source code must retain the above copyright notice, this
#  list of conditions and the following disclaimer.
#
# 2. Redistributions in binary form must reproduce the above copyright notice,
#  this list of conditions and the following disclaimer in the documentation
#  and/or other materials provided with the distribution.
#
# 3. Neither the name of the copyright holder nor the names of its
#  contributors may be used to endorse or promote products derived from
#  this software without specific prior written permission.
#
# THIS SOFTWARE IS PROVIDED BY THE COPYRIGHT HOLDERS AND CONTRIBUTORS "AS IS"
# AND ANY EXPRESS OR IMPLIED WARRANTIES, INCLUDING, BUT NOT LIMITED TO, THE
# IMPLIED WARRANTIES OF MERCHANTABILITY AND FITNESS FOR A PARTICULAR PURPOSE ARE
# DISCLAIMED. IN NO EVENT SHALL THE COPYRIGHT HOLDER OR CONTRIBUTORS BE LIABLE
# FOR ANY DIRECT, INDIRECT, INCIDENTAL, SPECIAL, EXEMPLARY, OR CONSEQUENTIAL
# DAMAGES (INCLUDING, BUT NOT LIMITED TO, PROCUREMENT OF SUBSTITUTE GOODS OR
# SERVICES; LOSS OF USE, DATA, OR PROFITS; OR BUSINESS INTERRUPTION) HOWEVER
# CAUSED AND ON ANY THEORY OF LIABILITY, WHETHER IN CONTRACT, STRICT LIABILITY,
# OR TORT (INCLUDING NEGLIGENCE OR OTHERWISE) ARISING IN ANY WAY OUT OF THE USE
# OF THIS SOFTWARE, EVEN IF ADVISED OF THE POSSIBILITY OF SUCH DAMAGE.

@prefix owl: <http://www.w3.org/2002/07/owl#> .
@prefix rdf: <http://www.w3.org/1999/02/22-rdf-syntax-ns#> .
@prefix rdfs: <http://www.w3.org/2000/01/rdf-schema#> .
@prefix xsd: <http://www.w3.org/2001/XMLSchema#> .
@prefix dc: <http://purl.org/dc/elements/1.1/> .
@prefix dcterms: <http://purl.org/dc/terms/> .
@prefix vann: <http://purl.org/vocab/vann/> .
@prefix time: <http://www.w3.org/2006/time#> .

@prefix ieso: <https://www.gecad.isep.ipp.pt/ieso/v1.0.0/> .
@base <https://www.gecad.isep.ipp.pt/ieso/> .


###  Demand Response Ontology
<demand-response/v1.0.0/>
  rdf:type owl:Ontology ;
  owl:versionIRI <demand-response/v1.0.0/> ;
  owl:versionInfo "v1.0.0" ;
  #owl:priorVersion <demand-response/v1.0.0/> ;
  rdfs:comment "This ontology describes concepts, relations, and properties identified in MAS-Society use cases."@en ;
  #rdfs:isDefinedBy <any-online-specification-document> ; # <- colocar ficheiro de referencia?
  #rdfs:seeAlso <other-online-specification-document-or-image> ; # <- colocar imagem onto
  dcterms:title "GECAD's IESO Demand Response Ontology"@en ;
  dcterms:description "The GECAD's Demand Response Ontology describes demand response concepts, relations, and properties related with demand response programs, events, and results."@en ;
  dcterms:issued "2019-07-01"^^xsd:date ;
  dcterms:modified "2023-02-17"^^xsd:date ;
  dcterms:publisher <https://www.gecad.isep.ipp.pt/> ;
  dcterms:license <https://www.gecad.isep.ipp.pt/ieso/license/> ;
  dcterms:creator <https://orcid.org/0000-0001-8839-8807> ;
  #dcterms:contributor [ a foaf:Person ; foaf:name "Gabriel Santos" ] ;
  dcterms:source <https://github.com/gabrieljlsantos/gecad-ieso> ;
  vann:preferredNamespacePrefix "ieso" ;
  vann:preferredNamespaceUri ieso: ;
  .
# !


#################################################################
#  Annotation properties
#################################################################


#################################################################
#  Datatype Properties
#################################################################


###  https://www.gecad.isep.ipp.pt/ieso/v1.0.0/participated
ieso:participatedInEvent
  rdf:type owl:DatatypeProperty ;
  rdfs:comment "The 'participated in event' object property relates a demand response player event result with its (boolean) participation."@en ;
  rdfs:label "participated in event"@en ;
  rdfs:isDefinedBy <demand-response/v1.0.0/> ;
  rdfs:domain ieso:DemandResponsePlayerEventResult ;
  rdfs:range xsd:boolean
  .
# !


###  https://www.gecad.isep.ipp.pt/ieso/v1.0.0/fulfilledMargins
ieso:fulfilledMargins
  rdf:type owl:DatatypeProperty ;
  rdfs:comment "The 'fulfilled margins' object property relates a demand response player event result with its (boolean) margins fulfilment."@en ;
  rdfs:label "fulfilled margins"@en ;
  rdfs:isDefinedBy <demand-response/v1.0.0/> ;
  rdfs:domain ieso:DemandResponsePlayerEventResult ;
  rdfs:range xsd:boolean
  .
# !


#################################################################
#  Object Properties
#################################################################


###  https://www.gecad.isep.ipp.pt/ieso/v1.0.0/concerningContract
ieso:concerningContract
  rdf:type owl:ObjectProperty ;
  rdfs:comment "The 'concerning contract' object property relates a demand response program with its contracts."@en ;
  rdfs:label "concerning contract"@en ;
  rdfs:isDefinedBy <demand-response/v1.0.0/> ;
  rdfs:domain ieso:DemandResponseProgram ;
  rdfs:range ieso:Contract ;
  .
# !


###  https://www.gecad.isep.ipp.pt/ieso/v1.0.0/demandResponseProgramDeployer
ieso:demandResponseProgramDeployer
  rdf:type owl:ObjectProperty ;
  rdfs:comment "The 'demand response program deployer' object property relates a demand response program with its deployer."@en ;
  rdfs:label "demand response program deployer"@en ;
  rdfs:isDefinedBy <demand-response/v1.0.0/> ;
  rdfs:domain ieso:DemandResponseProgram ;
  rdfs:range ieso:DemandResponseDeployer ;
  .
# !


###  https://www.gecad.isep.ipp.pt/ieso/v1.0.0/demandResponseProgramTrigger
ieso:demandResponseProgramTrigger
  rdf:type owl:ObjectProperty ;
  rdfs:comment "The 'demand response program trigger' object property relates a demand response program with its triggers."@en ;
  rdfs:label "demand response program trigger"@en ;
  rdfs:isDefinedBy <demand-response/v1.0.0/> ;
  rdfs:domain ieso:DemandResponseProgram ;
  rdfs:range ieso:DemandResponseTrigger ;
  .
# !


###  https://www.gecad.isep.ipp.pt/ieso/v1.0.0/deployedDemandResponseEvent
ieso:deployedDemandResponseEvent
  rdf:type owl:ObjectProperty ;
  rdfs:comment "The 'deployed demand response event' object property relates a demand response program with a deployed demand response event."@en ;
  rdfs:label "deployed demand response event"@en ;
  rdfs:isDefinedBy <demand-response/v1.0.0/> ;
  rdfs:domain ieso:DemandResponseProgram ;
  rdfs:range ieso:DemandResponseEvent ;
  .
# !


###  https://www.gecad.isep.ipp.pt/ieso/v1.0.0/effectiveEnergyVolumeSupplied
ieso:effectiveEnergyVolumeSupplied
  rdf:type owl:ObjectProperty ;
  rdfs:comment "The 'effective energy volume supplied' object property relates a demand response player event result with the effective energy volume supplied."@en ;
  rdfs:label "effective energy volume supplied"@en ;
  rdfs:isDefinedBy <demand-response/v1.0.0/> ;
  rdfs:domain ieso:DemandResponsePlayerEventResult ;
  rdfs:range [
    rdf:type owl:Class ;
    owl:unionOf (
      ieso:Energy
      ieso:Power
    )
  ] ;
  .
# !


###  https://www.gecad.isep.ipp.pt/ieso/v1.0.0/finalBalance
ieso:finalBalance
  rdf:type owl:ObjectProperty ;
  rdfs:comment "The 'final balance' object property relates a demand response participating player event result with its final balance after remuneration and penalty calculation."@en ;
  rdfs:label "final balance"@en ;
  rdfs:isDefinedBy <demand-response/v1.0.0/> ;
  rdfs:domain ieso:DemandResponsePlayerEventResult ;
  rdfs:range ieso:Price ;
  .
# !


###  https://www.gecad.isep.ipp.pt/ieso/v1.0.0/globalRequiredEnergyVolume
ieso:globalRequiredEnergyVolume
  rdf:type owl:ObjectProperty ;
  rdfs:comment "The 'global required energy volume' object property relates a demand response event with the required energy volume."@en ;
  rdfs:label "global required energy volume"@en ;
  rdfs:isDefinedBy <demand-response/v1.0.0/> ;
  rdfs:domain [
    rdf:type owl:Class ;
    owl:unionOf (
      ieso:DemandResponseEvent
      ieso:DemandResponsePlayerEventResult
    )
  ] ;
  rdfs:range [
    rdf:type owl:Class ;
    owl:unionOf (
      ieso:Energy
      ieso:Power
    )
  ] ;
  .
# !


###  https://www.gecad.isep.ipp.pt/ieso/v1.0.0/maximumConsumptionAllowed
ieso:maximumConsumptionAllowed
  rdf:type owl:ObjectProperty ;
  rdfs:comment "The 'maximum consumption allowed' object property relates a demand response event with the maximum consumption allowed."@en ;
  rdfs:label "maximum consumption allowed"@en ;
  rdfs:isDefinedBy <demand-response/v1.0.0/> ;
  rdfs:domain ieso:DemandResponseEvent ;
  rdfs:subPropertyOf ieso:globalRequiredEnergyVolume
  .
# !


###  https://www.gecad.isep.ipp.pt/ieso/v1.0.0/requiredCut
ieso:requiredCut
  rdf:type owl:ObjectProperty ;
  rdfs:comment "The 'required cut' object property relates a demand response event with the required energy volume cut."@en ;
  rdfs:label "required cut"@en ;
  rdfs:isDefinedBy <demand-response/v1.0.0/> ;
  rdfs:domain ieso:DemandResponseEvent ;
  rdfs:subPropertyOf ieso:globalRequiredEnergyVolume
  .
# !


###  https://www.gecad.isep.ipp.pt/ieso/v1.0.0/capacityRemuneration
ieso:capacityRemuneration
  rdf:type owl:ObjectProperty ;
  rdfs:comment "The 'capacity remuneration' object property relates a class or individual with its capacity remuneration.\n\nA fixed fee for participating/responding to the demand response event."@en ;
  rdfs:label "capacity remuneration"@en ;
  rdfs:isDefinedBy <contract/v1.0.0/> ;
  rdfs:range ieso:Price ;
  rdfs:subPropertyOf ieso:hasRemuneration ;
  .
# !


###  https://www.gecad.isep.ipp.pt/ieso/v1.0.0/remunerationPerEnergyUnit
ieso:remunerationPerEnergyUnit
  rdf:type owl:ObjectProperty ;
  rdfs:comment "The 'remuneration per energy unit' object property relates a class or individual with its remuneration per energy unit."@en ;
  rdfs:label "remuneration per energy unit"@en ;
  rdfs:isDefinedBy <contract/v1.0.0/> ;
  rdfs:range ieso:Price ;
  rdfs:subPropertyOf ieso:hasRemuneration ;
  .
# !


###  https://www.gecad.isep.ipp.pt/ieso/v1.0.0/totalRemuneration
ieso:totalRemuneration
  rdf:type owl:ObjectProperty ;
  rdfs:comment "The 'total remuneration' object property relates a demand response participating player event result with its total remuneration."@en ;
  rdfs:label "total remuneration"@en ;
  rdfs:isDefinedBy <demand-response/v1.0.0/> ;
  rdfs:domain ieso:DemandResponsePlayerEventResult ;
  rdfs:range ieso:Price ;
  rdfs:subPropertyOf ieso:hasRemuneration ;
  .
# !


###  https://www.gecad.isep.ipp.pt/ieso/v1.0.0/demandResponseEventPlayer
ieso:demandResponseEventPlayer
  rdf:type owl:ObjectProperty ;
  rdfs:comment "The 'demand response event player' object property relates a demand response  player event result with the respective player."@en ;
  rdfs:label "demand response event player"@en ;
  rdfs:isDefinedBy <demand-response/v1.0.0/> ;
  rdfs:domain ieso:DemandResponsePlayerEventResult ;
  .
# !


###  https://www.gecad.isep.ipp.pt/ieso/v1.0.0/penaltyToPay
ieso:penaltyToPay
  rdf:type owl:ObjectProperty ;
  rdfs:comment "The 'penalty to pay' object property relates a demand response participating player event result with a penalty to pay in case of non fulfilment."@en ;
  rdfs:label "penalty to pay"@en ;
  rdfs:isDefinedBy <demand-response/v1.0.0/> ;
  rdfs:domain ieso:DemandResponsePlayerEventResult ;
  rdfs:range ieso:Price ;
  .
# !


###  https://www.gecad.isep.ipp.pt/ieso/v1.0.0/playerEventResult
ieso:playerEventResult
  rdf:type owl:ObjectProperty ;
  rdfs:comment "The 'player event result' object property relates a demand response aggregator event result with a demand response player event result."@en ;
  rdfs:label "player event result"@en ;
  rdfs:isDefinedBy <demand-response/v1.0.0/> ;
  rdfs:domain ieso:DemandResponseAggregatorEventResult ;
  rdfs:range ieso:DemandResponsePlayerEventResult ;
  .
# !


###  https://www.gecad.isep.ipp.pt/ieso/v1.0.0/rampPeriod
ieso:rampPeriod
  rdf:type owl:ObjectProperty ;
  rdfs:comment "The 'ramp period' object property relates a demand response event with its ramp period."@en ;
  rdfs:label "ramp period"@en ;
  rdfs:isDefinedBy <demand-response/v1.0.0/> ;
  rdfs:domain ieso:DemandResponseEvent ;
  #rdfs:range time:Interval ;
  .
# !


###  https://www.gecad.isep.ipp.pt/ieso/v1.0.0/reductionDeviationLowerMargin
ieso:reductionDeviationLowerMargin
  rdf:type owl:ObjectProperty ;
  rdfs:comment "The 'reduction deviation lower margin' object property relates a demand response event with its reduction deviation lower margin."@en ;
  rdfs:label "reduction deviation lower margin"@en ;
  rdfs:isDefinedBy <demand-response/v1.0.0/> ;
  rdfs:domain ieso:DemandResponseEvent ;
  rdfs:range [
    rdf:type owl:Class ;
    owl:unionOf (
      ieso:Energy
      ieso:Power
    )
  ] ;
  .
# !


###  https://www.gecad.isep.ipp.pt/ieso/v1.0.0/reductionDeviationUpperMargin
ieso:reductionDeviationUpperMargin
  rdf:type owl:ObjectProperty ;
  rdfs:comment "The 'reduction deviation upper margin' object property relates a demand response event with its reduction deviation upper margin."@en ;
  rdfs:label "reduction deviation upper margin"@en ;
  rdfs:isDefinedBy <demand-response/v1.0.0/> ;
  rdfs:domain ieso:DemandResponseEvent ;
  rdfs:range [
    rdf:type owl:Class ;
    owl:unionOf (
      ieso:Energy
      ieso:Power
    )
  ] ;
  .
# !


###  https://www.gecad.isep.ipp.pt/ieso/v1.0.0/resultFromDemandResponseEvent
ieso:resultFromDemandResponseEvent
  rdf:type owl:ObjectProperty ;
  rdfs:comment "The 'result from demand response event' object property relates a demand response event result with a demand response event."@en ;
  rdfs:label "result from demand response event"@en ;
  rdfs:isDefinedBy <demand-response/v1.0.0/> ;
  rdfs:domain ieso:DemandResponseEventResult ;
  rdfs:range ieso:DemandResponseEvent ;
  .
# !


###  https://www.gecad.isep.ipp.pt/ieso/v1.0.0/demandResponseEventEndsAt
ieso:demandResponseEventEndsAt
  rdf:type owl:ObjectProperty ;
  rdfs:comment "The 'demand response event ends at' object property relates a demand response event with its end. It can be the end instant or period."@en ;
  rdfs:label "demand response event ends at"@en ;
  rdfs:isDefinedBy <contract/v1.0.0/> ;
  rdfs:domain ieso:DemandResponseEvent ;
  rdfs:range time:TemporalEntity ;
  rdfs:subPropertyOf time:hasTime ;
  .
# !


###  https://www.gecad.isep.ipp.pt/ieso/v1.0.0/demandResponseEventStartsAt
ieso:demandResponseEventStartsAt
  rdf:type owl:ObjectProperty ;
  rdfs:comment "The 'demand response event starts at' object property relates a demand response event with its beginning. It can be the start instant or period."@en ;
  rdfs:label "demand response event starts at"@en ;
  rdfs:isDefinedBy <contract/v1.0.0/> ;
  rdfs:domain ieso:DemandResponseEvent ;
  rdfs:range time:TemporalEntity ;
  rdfs:subPropertyOf time:hasTime ;
  .
# !


#################################################################
#  Classes
#################################################################


###  https://www.gecad.isep.ipp.pt/ieso/DemandResponseEvent
ieso:DemandResponseEvent
  rdf:type owl:Class ;
  rdfs:comment "This class abstracts and slightly describes demand response events."@en ;
  rdfs:label "Demand response event"@en ;
  rdfs:isDefinedBy <demand-response/v1.0.0/> ;
  rdfs:seeAlso
    <https://en.wikipedia.org/wiki/Demand_response> ,
    <https://uplight.com/blog/what-is-demand-response/> ;
  rdfs:subClassOf
    [
      rdf:type owl:Restriction ;
      owl:onProperty ieso:demandResponseEventEndsAt ;
      owl:qualifiedCardinality "1"^^xsd:nonNegativeInteger ;
      owl:onClass time:TemporalEntity ;
    ] , [
      rdf:type owl:Restriction ;
      owl:onProperty ieso:demandResponseEventStartsAt ;
      owl:qualifiedCardinality "1"^^xsd:nonNegativeInteger ;
      owl:onClass time:TemporalEntity ;
    ] , [
      rdf:type owl:Restriction ;
      owl:onProperty ieso:globalRequiredEnergyVolume ;
      owl:qualifiedCardinality "1"^^xsd:nonNegativeInteger ;
      owl:onClass [
        rdf:type owl:Class ;
        owl:unionOf (
          ieso:Energy
          ieso:Power
        )
      ]
    ] , [
      rdf:type owl:Restriction ;
      owl:onProperty ieso:rampPeriod ;
      owl:qualifiedCardinality "1"^^xsd:nonNegativeInteger ;
      owl:onClass time:Interval ;
    ] , [
      rdf:type owl:Restriction ;
      owl:onProperty ieso:reductionDeviationLowerMargin;
      owl:qualifiedCardinality "1"^^xsd:nonNegativeInteger ;
      owl:onClass [
        rdf:type owl:Class ;
        owl:unionOf (
          ieso:Energy
          ieso:Power
        )
      ]
    ]  , [
      rdf:type owl:Restriction ;
      owl:onProperty ieso:reductionDeviationUpperMargin;
      owl:qualifiedCardinality "1"^^xsd:nonNegativeInteger ;
      owl:onClass [
        rdf:type owl:Class ;
        owl:unionOf (
          ieso:Energy
          ieso:Power
        )
      ]
    ];
  .
# !


###  https://www.gecad.isep.ipp.pt/ieso/DemandResponseEventResult
ieso:DemandResponseEventResult
  rdf:type owl:Class ;
  rdfs:comment "This class abstracts demand response event results."@en ;
  rdfs:label "Demand response event result"@en ;
  rdfs:isDefinedBy <demand-response/v1.0.0/> ;
  rdfs:subClassOf
    [
      rdf:type owl:Restriction ;
      owl:onProperty ieso:resultFromDemandResponseEvent ;
      owl:qualifiedCardinality "1"^^xsd:nonNegativeInteger ;
      owl:onClass ieso:DemandResponseEvent
    ] ;
  .
# !


###  https://www.gecad.isep.ipp.pt/ieso/DemandResponseAggregatorEventResult
ieso:DemandResponseAggregatorEventResult
  rdf:type owl:Class ;
  rdfs:comment "This class describes the event results of a demand response aggregator."@en ;
  rdfs:label "Demand response aggregator event result"@en ;
  rdfs:isDefinedBy <demand-response/v1.0.0/> ;
  rdfs:subClassOf
    ieso:DemandResponseEventResult ,
    [
      rdf:type owl:Restriction ;
      owl:onProperty ieso:playerEventResult ;
      owl:someValuesFrom ieso:DemandResponsePlayerEventResult
    ] ;
  .
# !


###  https://www.gecad.isep.ipp.pt/ieso/DemandResponsePlayerEventResult
ieso:DemandResponsePlayerEventResult
  rdf:type owl:Class ;
  rdfs:comment "This class describes the event results of a demand response player."@en ;
  rdfs:label "Demand response player event result"@en ;
  rdfs:isDefinedBy <demand-response/v1.0.0/> ;
  rdfs:subClassOf
    ieso:DemandResponseEventResult ,
    [
      rdf:type owl:Restriction ;
      owl:onProperty ieso:capacityRemuneration ;
      owl:maxQualifiedCardinality "1"^^xsd:nonNegativeInteger ;
      owl:onClass ieso:Price
    ] , [
      rdf:type owl:Restriction ;
      owl:onProperty ieso:demandResponseEventPlayer ;
      owl:maxQualifiedCardinality "1"^^xsd:nonNegativeInteger ;
      owl:onClass ieso:Actor
    ] , [
      rdf:type owl:Restriction ;
      owl:onProperty ieso:effectiveEnergyVolumeSupplied ;
      owl:qualifiedCardinality "1"^^xsd:nonNegativeInteger ;
      owl:onClass [
        rdf:type owl:Class ;
        owl:unionOf (
          ieso:Energy
          ieso:Power
        )
      ]
    ] , [
      rdf:type owl:Restriction ;
      owl:onProperty ieso:finalBalance ;
      owl:qualifiedCardinality "1"^^xsd:nonNegativeInteger ;
      owl:onClass ieso:Price
    ] , [
      rdf:type owl:Restriction ;
      owl:onProperty ieso:fulfilledMargins ;
      owl:qualifiedCardinality "1"^^xsd:nonNegativeInteger ;
      owl:onDataRange xsd:boolean
    ] , [
      rdf:type owl:Restriction ;
      owl:onProperty ieso:globalRequiredEnergyVolume ;
      owl:qualifiedCardinality "1"^^xsd:nonNegativeInteger ;
      owl:onClass [
        rdf:type owl:Class ;
        owl:unionOf (
          ieso:Energy
          ieso:Power
        )
      ]
    ] , [
      rdf:type owl:Restriction ;
      owl:onProperty ieso:participatedInEvent ;
      owl:qualifiedCardinality "1"^^xsd:nonNegativeInteger ;
      owl:onDataRange xsd:boolean
    ] , [
      rdf:type owl:Restriction ;
      owl:onProperty ieso:penaltyToPay ;
      owl:maxQualifiedCardinality "1"^^xsd:nonNegativeInteger ;
      owl:onClass ieso:Price
    ] , [
      rdf:type owl:Restriction ;
      owl:onProperty ieso:remunerationPerEnergyUnit ;
      owl:maxQualifiedCardinality "1"^^xsd:nonNegativeInteger ;
      owl:onClass ieso:Price
    ] , [
      rdf:type owl:Restriction ;
      owl:onProperty ieso:totalRemuneration ;
      owl:maxQualifiedCardinality "1"^^xsd:nonNegativeInteger ;
      owl:onClass ieso:Price
    ] ;
  .
# !


###  https://www.gecad.isep.ipp.pt/ieso/DemandResponseProgram
ieso:DemandResponseProgram
  rdf:type owl:Class ;
  rdfs:comment "This class abstracts and slightly describes demand response programs."@en ;
  rdfs:label "Demand response program"@en ;
  rdfs:isDefinedBy <demand-response/v1.0.0/> ;
  rdfs:seeAlso
    <https://en.wikipedia.org/wiki/Demand_response> ,
    <https://uplight.com/blog/what-is-demand-response/> ;
  rdfs:subClassOf
    [
      rdf:type owl:Restriction ;
      owl:onProperty ieso:concerningContract ;
      owl:someValuesFrom ieso:Contract
    ] , [
      rdf:type owl:Restriction ;
      owl:onProperty ieso:demandResponseProgramDeployer ;
      owl:someValuesFrom ieso:DemandResponseDeployer
    ] , [
      rdf:type owl:Restriction ;
      owl:onProperty ieso:demandResponseProgramTrigger ;
      owl:someValuesFrom ieso:DemandResponseTrigger
    ] , [
      rdf:type owl:Restriction ;
      owl:onProperty ieso:deployedDemandResponseEvent ;
      owl:someValuesFrom ieso:DemandResponseEvent
    ] ;
  .
# !


###  https://www.gecad.isep.ipp.pt/ieso/DemandResponseTrigger
ieso:DemandResponseTrigger
  rdf:type owl:Class ;
  rdfs:comment "This class abstracts demand response triggers."@en ;
  rdfs:label "Demand response trigger"@en ;
  rdfs:isDefinedBy <demand-response/v1.0.0/> ;
  .
# !


###  https://www.gecad.isep.ipp.pt/ieso/DemandResponseDeployer
ieso:DemandResponseDeployer
  rdf:type owl:Class ;
  rdfs:comment "This class describes a demand response deployer role.\n\nThis is the entity that activates/triggers/manages the demand response program/event."@en ;
  rdfs:label "Demand response deployer"@en ;
  rdfs:isDefinedBy <demand-response/v1.0.0/> ;
  rdfs:subClassOf ieso:Role ;
  .
# !


#################################################################
#  General axioms
#################################################################


#################################################################
#  Individuals
#################################################################


#################################################################
#  Rules
#################################################################
