# BSD 3-Clause License
#
# Copyright (c) 2021, gabrieljlsantos
# All rights reserved.
#
# Redistribution and use in source and binary forms, with or without
# modification, are permitted provided that the following conditions are met:
#
# 1. Redistributions of source code must retain the above copyright notice, this
#  list of conditions and the following disclaimer.
#
# 2. Redistributions in binary form must reproduce the above copyright notice,
#  this list of conditions and the following disclaimer in the documentation
#  and/or other materials provided with the distribution.
#
# 3. Neither the name of the copyright holder nor the names of its
#  contributors may be used to endorse or promote products derived from
#  this software without specific prior written permission.
#
# THIS SOFTWARE IS PROVIDED BY THE COPYRIGHT HOLDERS AND CONTRIBUTORS "AS IS"
# AND ANY EXPRESS OR IMPLIED WARRANTIES, INCLUDING, BUT NOT LIMITED TO, THE
# IMPLIED WARRANTIES OF MERCHANTABILITY AND FITNESS FOR A PARTICULAR PURPOSE ARE
# DISCLAIMED. IN NO EVENT SHALL THE COPYRIGHT HOLDER OR CONTRIBUTORS BE LIABLE
# FOR ANY DIRECT, INDIRECT, INCIDENTAL, SPECIAL, EXEMPLARY, OR CONSEQUENTIAL
# DAMAGES (INCLUDING, BUT NOT LIMITED TO, PROCUREMENT OF SUBSTITUTE GOODS OR
# SERVICES; LOSS OF USE, DATA, OR PROFITS; OR BUSINESS INTERRUPTION) HOWEVER
# CAUSED AND ON ANY THEORY OF LIABILITY, WHETHER IN CONTRACT, STRICT LIABILITY,
# OR TORT (INCLUDING NEGLIGENCE OR OTHERWISE) ARISING IN ANY WAY OUT OF THE USE
# OF THIS SOFTWARE, EVEN IF ADVISED OF THE POSSIBILITY OF SUCH DAMAGE.

@prefix owl: <http://www.w3.org/2002/07/owl#> .
@prefix rdf: <http://www.w3.org/1999/02/22-rdf-syntax-ns#> .
@prefix rdfs: <http://www.w3.org/2000/01/rdf-schema#> .
@prefix xsd: <http://www.w3.org/2001/XMLSchema#> .
@prefix dc: <http://purl.org/dc/elements/1.1/> .
@prefix dcterms: <http://purl.org/dc/terms/> .
@prefix vann: <http://purl.org/vocab/vann/> .

@prefix ieso: <https://www.gecad.isep.ipp.pt/ieso/v1.0.0/> .
@base <https://www.gecad.isep.ipp.pt/ieso/> .


###  Measure Ontology
<measure/v1.0.0/>
  rdf:type owl:Ontology ;
  owl:versionIRI <measure/v1.0.0/> ;
  owl:versionInfo "v1.0.0" ;
  #owl:priorVersion <measure/v1.0.0/> ;
  rdfs:comment "This ontology gathers units of measure needed for the MAS-Society project. It is a separate module as it describes concepts and relations useful for various IESO modules."@en ;
  #rdfs:isDefinedBy <any-online-specification-document> ;
  #rdfs:seeAlso <uri-to-other-document-or-image> ;
  dcterms:title "GECAD's IESO Measure Ontology"@en ;
  dcterms:description "The GECAD's IESO Measure Ontology describes measures, measurement values, types of measures, and units of measure. A measurement is composed of a type of measure, at least a measurement value and respective unit of measure. A type of measure is related to a unit of measure. A measurement value is described by exactly one literal value and the respective unit of measure. A measurement can be related to several measurement values with different units; as long as they derive from the same SI unit, e.g. a power measurement can have a value of 2000W and another of 2kW, representing the same value in different magnitudes. Additionally, this ontology defines a unit converter template class to provide conversion templates for automatic values conversion."@en ;
  dcterms:issued "2019-07-01"^^xsd:date ;
  dcterms:modified "2023-02-17"^^xsd:date ;
  dcterms:publisher <https://www.gecad.isep.ipp.pt/> ;
  dcterms:license <https://www.gecad.isep.ipp.pt/ieso/license/> ;
  dcterms:creator <https://orcid.org/0000-0001-8839-8807> ;
  #dcterms:contributor [ a foaf:Person ; foaf:name "Gabriel Santos" ] ;
  dcterms:source <https://github.com/gabrieljlsantos/gecad-ieso> ;
  vann:preferredNamespacePrefix "ieso" ;
  vann:preferredNamespaceUri ieso: ;
  .
# !


#################################################################
#  Datatype Properties
#################################################################


###  https://www.gecad.isep.ipp.pt/ieso/v1.0.0/conversionCoefficientToSIUnit
ieso:conversionCoefficientToSIUnit
  rdf:type
    owl:DatatypeProperty ,
    owl:FunctionalProperty ;
  rdfs:comment "In mathematics, a coefficient is a multiplicative factor in some term of a polynomial, a series, or any expression; it is usually a number, but may be any expression (including variables such as a, b and c). In the latter case, the variables appearing in the coefficients are often called parameters, and must be clearly distinguished from the other variables.\n\nThe 'conversion coefficient to SI unit' data property relates a 'Unit of measure' to its conversion coefficient relative to the SI unit."@en ;
  rdfs:label "conversion coefficient to SI unit"@en ;
  rdfs:isDefinedBy <measure/v1.0.0/> ;
  rdfs:seeAlso <https://en.wikipedia.org/wiki/Coefficient> ;
  rdfs:domain ieso:DimensionalUnit ;
  rdfs:range xsd:double ;
  .
# !


###  https://www.gecad.isep.ipp.pt/ieso/v1.0.0/conversionOffsetToSIUnit
ieso:conversionOffsetToSIUnit
  rdf:type
    owl:DatatypeProperty ,
    owl:FunctionalProperty ;
  rdfs:comment "The 'conversion offset to SI unit' data property relates a 'Unit of measure' to its conversion offset relative to the SI unit."@en ;
  rdfs:label "conversion offset to SI unit"@en ;
  rdfs:isDefinedBy <measure/v1.0.0/> ;
  rdfs:domain ieso:DimensionalUnit ;
  rdfs:range xsd:double ;
  .
# !


###  https://www.gecad.isep.ipp.pt/ieso/v1.0.0/conversionTemplate
ieso:conversionTemplate
  rdf:type
    owl:DatatypeProperty ,
    owl:FunctionalProperty ;
  rdfs:comment "The 'conversion template' data property relates a 'SI unit converter template' to its conversion template string value."@en ;
  rdfs:label "conversion template"@en ;
  rdfs:isDefinedBy <measure/v1.0.0/> ;
  rdfs:domain ieso:UnitConverterTemplate ;
  rdfs:range xsd:string ;
  .
# !


###  https://www.gecad.isep.ipp.pt/ieso/v1.0.0/conversionTemplateSyntax
ieso:conversionTemplateSyntax
  rdf:type
    owl:DatatypeProperty ,
    owl:FunctionalProperty ;
  rdfs:comment "The 'conversion template syntax' data property relates a 'SI unit converter template' to its conversion template syntax. One of: SPARQL, SQWRL, SWRL."@en ;
  rdfs:label "conversion template syntax"@en ;
  rdfs:isDefinedBy <measure/v1.0.0/> ;
  rdfs:domain ieso:UnitConverterTemplate ;
  rdfs:range [
    rdf:type rdfs:Datatype ;
    owl:oneOf [
      rdf:type rdf:List ;
      rdf:first "SPARQL" ;
      rdf:rest [
        rdf:type rdf:List ;
        rdf:first "SQWRL" ;
        rdf:rest [
          rdf:type rdf:List ;
          rdf:first "SWRL" ;
          rdf:rest rdf:nil
        ]
      ]
    ]
  ] ;
  .
# !


###  https://www.gecad.isep.ipp.pt/ieso/v1.0.0/hasDateTime
ieso:hasDateTime
  rdf:type owl:DatatypeProperty ;
  rdfs:comment "The 'has date-time' data type property relates a measurement to its date-time."@en ;
  rdfs:label "has date-time"@en ;
  rdfs:isDefinedBy <measure/v1.0.0/> ;
  rdfs:domain ieso:Measurement ;
  .
# !


###  https://www.gecad.isep.ipp.pt/ieso/v1.0.0/hasLiteralValue
ieso:hasLiteralValue
  rdf:type
    owl:DatatypeProperty ,
    owl:FunctionalProperty ;
  rdfs:comment "The 'has literal value' data property relates a 'Measurement value' to its literal value."@en ;
  rdfs:label "has literal value"@en ;
  rdfs:isDefinedBy <measure/v1.0.0/> ;
  rdfs:domain ieso:MeasurementValue ;
  .
# !


###  https://www.gecad.isep.ipp.pt/ieso/v1.0.0/unitSymbol
ieso:unitCode
  rdf:type owl:DatatypeProperty ;
  rdfs:comment "The 'unit code' data property relates a 'Unit of measure' to its literal code."@en ;
  rdfs:label "unit code" ;
  rdfs:isDefinedBy <measure/v1.0.0/> ;
  rdfs:domain ieso:UnitOfMeasure ;
  .
# !


###  https://www.gecad.isep.ipp.pt/ieso/v1.0.0/unitSymbol
ieso:unitSymbol
  rdf:type owl:DatatypeProperty ;
  rdfs:comment "The 'unit symbol' data property relates a 'Unit of measure' to its literal symbol."@en ;
  rdfs:label "unit symbol" ;
  rdfs:isDefinedBy <measure/v1.0.0/> ;
  rdfs:domain ieso:UnitOfMeasure ;
  .
# !


#################################################################
#  Object Properties
#################################################################


###  https://www.gecad.isep.ipp.pt/ieso/v1.0.0/hasMeasurement
ieso:hasMeasurement
  rdf:type owl:ObjectProperty ;
  rdfs:comment "The 'has measurement' object property relates a class or individual with its 'Measurement'."@en ;
  rdfs:label "has measurement"@en ;
  rdfs:isDefinedBy <measure/v1.0.0/> ;
  rdfs:range ieso:Measurement ;
  owl:inverseOf ieso:isMeasurementOf ;
  .
# !


###  https://www.gecad.isep.ipp.pt/ieso/v1.0.0/hasAngle
ieso:hasAngle
  rdf:type owl:ObjectProperty ;
  rdfs:comment "The 'has angle' object property relates a class or individual with its angle."@en ;
  rdfs:label "has angle"@en ;
  rdfs:isDefinedBy <measure/v1.0.0/> ;
  rdfs:subPropertyOf ieso:hasMeasurement ;
  .
# !


###  https://www.gecad.isep.ipp.pt/ieso/v1.0.0/hasAngleShift
ieso:hasAngleShift
  rdf:type owl:ObjectProperty ;
  rdfs:comment "The 'has angle shift' object property relates a class or individual with its angle shift."@en ;
  rdfs:label "has angle shift"@en ;
  rdfs:isDefinedBy <measure/v1.0.0/> ;
  rdfs:subPropertyOf ieso:hasAngle ;
  .
# !


###  https://www.gecad.isep.ipp.pt/ieso/v1.0.0/hasVoltageAngle
ieso:hasVoltageAngle
  rdf:type owl:ObjectProperty ;
  rdfs:comment "The 'has voltage angle' object property relates a class or individual with its voltage angle."@en ;
  rdfs:label "has voltage angle"@en ;
  rdfs:isDefinedBy <measure/v1.0.0/> ;
  rdfs:subPropertyOf ieso:hasAngle ;
  .
# !


###  https://www.gecad.isep.ipp.pt/ieso/v1.0.0/hasVoltageAngleAtFromBus
ieso:hasVoltageAngleAtFromBus
  rdf:type owl:ObjectProperty ;
  rdfs:comment "The 'has voltage angle at from bus' object property relates a class or individual with its voltage angle at 'from bus'."@en ;
  rdfs:label "has voltage angle at from bus"@en ;
  rdfs:isDefinedBy <measure/v1.0.0/> ;
  rdfs:subPropertyOf ieso:hasVoltageAngle ;
  .
# !


###  https://www.gecad.isep.ipp.pt/ieso/v1.0.0/hasVoltageAngleAtToBus
ieso:hasVoltageAngleAtToBus
  rdf:type owl:ObjectProperty ;
  rdfs:comment "The 'has voltage angle at to bus' object property relates a class or individual with its voltage angle at 'to bus'."@en ;
  rdfs:label "has voltage angle at to bus"@en ;
  rdfs:isDefinedBy <measure/v1.0.0/> ;
  rdfs:subPropertyOf ieso:hasVoltageAngle ;
  .
# !


###  https://www.gecad.isep.ipp.pt/ieso/v1.0.0/ieso:hasVoltageAngleAtHighVoltageBus
ieso:ieso:hasVoltageAngleAtHighVoltageBus
  rdf:type owl:ObjectProperty ;
  rdfs:comment "The 'has voltage angle at high voltage bus' object property relates a class or individual with its voltage angle at high voltage bus."@en ;
  rdfs:label "has voltage angle at high voltage bus"@en ;
  rdfs:isDefinedBy <measure/v1.0.0/> ;
  rdfs:subPropertyOf ieso:hasVoltageAngle ;
  .
# !


###  https://www.gecad.isep.ipp.pt/ieso/v1.0.0/ieso:hasVoltageAngleAtLowVoltageBus
ieso:ieso:hasVoltageAngleAtLowVoltageBus
  rdf:type owl:ObjectProperty ;
  rdfs:comment "The 'has voltage angle at low voltage bus' object property relates a class or individual with its voltage angle at low voltage bus."@en ;
  rdfs:label "has voltage angle at low voltage bus"@en ;
  rdfs:isDefinedBy <measure/v1.0.0/> ;
  rdfs:subPropertyOf ieso:hasVoltageAngle ;
  .
# !


###  https://www.gecad.isep.ipp.pt/ieso/v1.0.0/ieso:hasVoltageAngleAtMediumVoltageBus
ieso:ieso:hasVoltageAngleAtMediumVoltageBus
  rdf:type owl:ObjectProperty ;
  rdfs:comment "The 'has voltage angle at medium voltage bus' object property relates a class or individual with its voltage angle at medium voltage bus."@en ;
  rdfs:label "has voltage angle at medium voltage bus"@en ;
  rdfs:isDefinedBy <measure/v1.0.0/> ;
  rdfs:subPropertyOf ieso:hasVoltageAngle ;
  .
# !


###  https://www.gecad.isep.ipp.pt/ieso/v1.0.0/hasCapacitance
ieso:hasCapacitance
  rdf:type owl:ObjectProperty ;
  rdfs:comment "The 'has capacitance' object property relates a class or individual with its capacitance."@en ;
  rdfs:label "has capacitance"@en ;
  rdfs:isDefinedBy <measure/v1.0.0/> ;
  rdfs:subPropertyOf ieso:hasMeasurement ;
  .
# !


###  https://www.gecad.isep.ipp.pt/ieso/v1.0.0/hasZeroSequenceCapacitance
ieso:hasZeroSequenceCapacitance
  rdf:type owl:ObjectProperty ;
  rdfs:comment "The 'has zero sequence capacitance' object property relates a class or individual with its zero sequence capacitance."@en ;
  rdfs:label "has zero sequence capacitance"@en ;
  rdfs:isDefinedBy <measure/v1.0.0/> ;
  rdfs:subPropertyOf ieso:hasCapacitance ;
  .
# !


###  https://www.gecad.isep.ipp.pt/ieso/v1.0.0/hasConductance
ieso:hasConductance
  rdf:type owl:ObjectProperty ;
  rdfs:comment "The 'has conductance' object property relates a class or individual with its conductance."@en ;
  rdfs:label "has conductance"@en ;
  rdfs:isDefinedBy <measure/v1.0.0/> ;
  rdfs:subPropertyOf ieso:hasMeasurement ;
  .
# !


###  https://www.gecad.isep.ipp.pt/ieso/v1.0.0/hasZeroSequenceConductance
ieso:hasZeroSequenceConductance
  rdf:type owl:ObjectProperty ;
  rdfs:comment "The 'has zero sequence conductance' object property relates a class or individual with its zero sequence conductance."@en ;
  rdfs:label "has zero sequence conductance"@en ;
  rdfs:isDefinedBy <measure/v1.0.0/> ;
  rdfs:subPropertyOf ieso:hasConductance ;
  .
# !


###  https://www.gecad.isep.ipp.pt/ieso/v1.0.0/hasCosinePhi
ieso:hasCosinePhi
  rdf:type owl:ObjectProperty ;
  rdfs:comment "The 'has cosine phi' object property relates a class or individual with its cosine phi."@en ;
  rdfs:label "has cosine phi"@en ;
  rdfs:isDefinedBy <measure/v1.0.0/> ;
  rdfs:subPropertyOf ieso:hasMeasurement ;
  .
# !


###  https://www.gecad.isep.ipp.pt/ieso/v1.0.0/hasCurrent
ieso:hasCurrent
  rdf:type owl:ObjectProperty ;
  rdfs:comment "The 'has current' object property relates a class or individual with its current."@en ;
  rdfs:label "has current"@en ;
  rdfs:isDefinedBy <measure/v1.0.0/> ;
  rdfs:subPropertyOf ieso:hasMeasurement ;
  .
# !


###  https://www.gecad.isep.ipp.pt/ieso/v1.0.0/hasCurrentAtFromBus
ieso:hasCurrentAtFromBus
  rdf:type owl:ObjectProperty ;
  rdfs:comment "The 'has current at from bus' object property relates a class or individual with its current at 'from bus'."@en ;
  rdfs:label "has current at from bus"@en ;
  rdfs:isDefinedBy <measure/v1.0.0/> ;
  rdfs:subPropertyOf ieso:hasCurrent ;
  .
# !


###  https://www.gecad.isep.ipp.pt/ieso/v1.0.0/hasCurrentAtToBus
ieso:hasCurrentAtToBus
  rdf:type owl:ObjectProperty ;
  rdfs:comment "The 'has current at to bus' object property relates a class or individual with its current at 'to bus'."@en ;
  rdfs:label "has current at to bus"@en ;
  rdfs:isDefinedBy <measure/v1.0.0/> ;
  rdfs:subPropertyOf ieso:hasCurrent ;
  .
# !


###  https://www.gecad.isep.ipp.pt/ieso/v1.0.0/hasCurrentAtHighVoltageSide
ieso:hasCurrentAtHighVoltageSide
  rdf:type owl:ObjectProperty ;
  rdfs:comment "The 'has current at high voltage side' object property relates a class or individual with its current at high voltage side."@en ;
  rdfs:label "has current at high voltage side"@en ;
  rdfs:isDefinedBy <measure/v1.0.0/> ;
  rdfs:subPropertyOf ieso:hasCurrent ;
  .
# !


###  https://www.gecad.isep.ipp.pt/ieso/v1.0.0/hasCurrentAtLowVoltageSide
ieso:hasCurrentAtLowVoltageSide
  rdf:type owl:ObjectProperty ;
  rdfs:comment "The 'has current at low voltage side' object property relates a class or individual with its current at low voltage side."@en ;
  rdfs:label "has current at low voltage side"@en ;
  rdfs:isDefinedBy <measure/v1.0.0/> ;
  rdfs:subPropertyOf ieso:hasCurrent ;
  .
# !


###  https://www.gecad.isep.ipp.pt/ieso/v1.0.0/hasCurrentAtMediumVoltageSide
ieso:hasCurrentAtMediumVoltageSide
  rdf:type owl:ObjectProperty ;
  rdfs:comment "The 'has current at medium voltage side' object property relates a class or individual with its current at medium voltage side."@en ;
  rdfs:label "has current at medium voltage side"@en ;
  rdfs:isDefinedBy <measure/v1.0.0/> ;
  rdfs:subPropertyOf ieso:hasCurrent ;
  .
# !


###  https://www.gecad.isep.ipp.pt/ieso/v1.0.0/hasLockedRotorCurrent
ieso:hasLockedRotorCurrent
  rdf:type owl:ObjectProperty ;
  rdfs:comment "The 'has locked rotor current' object property relates a class or individual with its locked rotor current."@en ;
  rdfs:label "has locked rotor current"@en ;
  rdfs:isDefinedBy <measure/v1.0.0/> ;
  rdfs:subPropertyOf ieso:hasCurrent ;
  .
# !


###  https://www.gecad.isep.ipp.pt/ieso/v1.0.0/hasMaximumCurrent
ieso:hasMaximumCurrent
  rdf:type owl:ObjectProperty ;
  rdfs:comment "The 'has maximum current' object property relates a class or individual with its maximum current."@en ;
  rdfs:label "has maximum current"@en ;
  rdfs:isDefinedBy <measure/v1.0.0/> ;
  rdfs:subPropertyOf ieso:hasCurrent ;
  .
# !


###  https://www.gecad.isep.ipp.pt/ieso/v1.0.0/hasEnergy
ieso:hasEnergy
  rdf:type owl:ObjectProperty ;
  rdfs:comment "The 'has energy' object property relates a class or individual with its energy."@en ;
  rdfs:label "has energy"@en ;
  rdfs:isDefinedBy <measure/v1.0.0/> ;
  rdfs:subPropertyOf ieso:hasMeasurement ;
  .
# !


###  https://www.gecad.isep.ipp.pt/ieso/v1.0.0/hasMaximumEnergy
ieso:hasMaximumEnergy
  rdf:type owl:ObjectProperty ;
  rdfs:comment "The 'has maximum energy' object property relates a class or individual with its maximum energy."@en ;
  rdfs:label "has maximum energy"@en ;
  rdfs:isDefinedBy <measure/v1.0.0/> ;
  rdfs:subPropertyOf ieso:hasEnergy ;
  .
# !


###  https://www.gecad.isep.ipp.pt/ieso/v1.0.0/hasMinimumEnergy
ieso:hasMinimumEnergy
  rdf:type owl:ObjectProperty ;
  rdfs:comment "The 'has minimum energy' object property relates a class or individual with its minimum energy."@en ;
  rdfs:label "has minimum energy"@en ;
  rdfs:isDefinedBy <measure/v1.0.0/> ;
  rdfs:subPropertyOf ieso:hasEnergy ;
  .
# !


###  https://www.gecad.isep.ipp.pt/ieso/v1.0.0/hasFrequency
ieso:hasFrequency
  rdf:type owl:ObjectProperty ;
  rdfs:comment "The 'has frequency' object property relates a class or individual with its frequency."@en ;
  rdfs:label "has frequency"@en ;
  rdfs:isDefinedBy <measure/v1.0.0/> ;
  rdfs:subPropertyOf ieso:hasMeasurement ;
  .
# !


###  https://www.gecad.isep.ipp.pt/ieso/v1.0.0/hasImpedance
ieso:hasImpedance
  rdf:type owl:ObjectProperty ;
  rdfs:comment "The 'has impedance' object property relates a class or individual with its impedance."@en ;
  rdfs:label "has impedance"@en ;
  rdfs:isDefinedBy <measure/v1.0.0/> ;
  rdfs:subPropertyOf ieso:hasMeasurement ;
  .
# !


###  https://www.gecad.isep.ipp.pt/ieso/v1.0.0/hasImaginaryPartOfImpedance
ieso:hasImaginaryPartOfImpedance
  rdf:type owl:ObjectProperty ;
  rdfs:comment "The 'has imaginary part of impedance' object property relates a class or individual with its imaginary part of impedance."@en ;
  rdfs:label "has imaginary part of impedance"@en ;
  rdfs:isDefinedBy <measure/v1.0.0/> ;
  rdfs:subPropertyOf ieso:hasImpedance ;
  owl:equivalentProperty ieso:hasReactance ;
  .
# !


###  https://www.gecad.isep.ipp.pt/ieso/v1.0.0/hasRealPartOfImpedance
ieso:hasRealPartOfImpedance
  rdf:type owl:ObjectProperty ;
  rdfs:comment "The 'has real part of impedance' object property relates a class or individual with its real part of impedance."@en ;
  rdfs:label "has real part of impedance"@en ;
  rdfs:isDefinedBy <measure/v1.0.0/> ;
  rdfs:subPropertyOf ieso:hasImpedance ;
  owl:equivalentProperty ieso:hasResistance ;
  .
# !


###  https://www.gecad.isep.ipp.pt/ieso/v1.0.0/hasZeroSequenceLeakageImpedance
ieso:hasZeroSequenceLeakageImpedance
  rdf:type owl:ObjectProperty ;
  rdfs:comment "The 'has zero sequence leakage impedance' object property relates a class or individual with its zero sequence leakage impedance."@en ;
  rdfs:label "has zero sequence leakage impedance"@en ;
  rdfs:isDefinedBy <measure/v1.0.0/> ;
  rdfs:subPropertyOf ieso:hasImpedance ;
  .
# !


###  https://www.gecad.isep.ipp.pt/ieso/v1.0.0/hasZeroSequenceImpedance
ieso:hasZeroSequenceImpedance
  rdf:type owl:ObjectProperty ;
  rdfs:comment "The 'has zero sequence impedance' object property relates a class or individual with its zero sequence impedance."@en ;
  rdfs:label "has zero sequence impedance"@en ;
  rdfs:isDefinedBy <measure/v1.0.0/> ;
  rdfs:subPropertyOf ieso:hasImpedance ;
  .
# !


###  https://www.gecad.isep.ipp.pt/ieso/v1.0.0/hasLength
ieso:hasLength
  rdf:type owl:ObjectProperty ;
  rdfs:comment "The 'has length' object property relates a class or individual with its length."@en ;
  rdfs:label "has length"@en ;
  rdfs:isDefinedBy <measure/v1.0.0/> ;
  rdfs:subPropertyOf ieso:hasMeasurement ;
  .
# !


###  https://www.gecad.isep.ipp.pt/ieso/v1.0.0/hasMagnitude
ieso:hasMagnitude
  rdf:type owl:ObjectProperty ;
  rdfs:comment "The 'has magnitude' object property relates a class or individual with its magnitude."@en ;
  rdfs:label "has magnitude"@en ;
  rdfs:isDefinedBy <measure/v1.0.0/> ;
  rdfs:subPropertyOf ieso:hasMeasurement ;
  .
# !


###  https://www.gecad.isep.ipp.pt/ieso/v1.0.0/hasMaximumMagnitude
ieso:hasMaximumMagnitude
  rdf:type owl:ObjectProperty ;
  rdfs:comment "The 'has maximum magnitude' object property relates a class or individual with its maximum magnitude."@en ;
  rdfs:label "has maximum magnitude"@en ;
  rdfs:isDefinedBy <measure/v1.0.0/> ;
  rdfs:subPropertyOf ieso:hasMagnitude ;
  .
# !


###  https://www.gecad.isep.ipp.pt/ieso/v1.0.0/hasMinimumMagnitude
ieso:hasMinimumMagnitude
  rdf:type owl:ObjectProperty ;
  rdfs:comment "The 'has minimum magnitude' object property relates a class or individual with its minimum magnitude."@en ;
  rdfs:label "has minimum magnitude"@en ;
  rdfs:isDefinedBy <measure/v1.0.0/> ;
  rdfs:subPropertyOf ieso:hasMagnitude ;
  .
# !


###  https://www.gecad.isep.ipp.pt/ieso/v1.0.0/hasVoltageMagnitude
ieso:hasVoltageMagnitude
  rdf:type owl:ObjectProperty ;
  rdfs:comment "The 'has voltage magnitude' object property relates a class or individual with its voltage magnitude."@en ;
  rdfs:label "has voltage magnitude"@en ;
  rdfs:isDefinedBy <measure/v1.0.0/> ;
  rdfs:subPropertyOf ieso:hasMagnitude ;
  .
# !


###  https://www.gecad.isep.ipp.pt/ieso/v1.0.0/hasVoltageMagnitudeAtFromBus
ieso:hasVoltageMagnitudeAtFromBus
  rdf:type owl:ObjectProperty ;
  rdfs:comment "The 'has voltage magnitude at from bus' object property relates a class or individual with its voltage magnitude at 'from bus'."@en ;
  rdfs:label "has voltage magnitude at from bus"@en ;
  rdfs:isDefinedBy <measure/v1.0.0/> ;
  rdfs:subPropertyOf ieso:hasVoltageMagnitude ;
  .
# !


###  https://www.gecad.isep.ipp.pt/ieso/v1.0.0/hasVoltageMagnitudeAtToBus
ieso:hasVoltageMagnitudeAtToBus
  rdf:type owl:ObjectProperty ;
  rdfs:comment "The 'has voltage magnitude at to bus' object property relates a class or individual with its voltage magnitude at 'to bus'."@en ;
  rdfs:label "has voltage magnitude at to bus"@en ;
  rdfs:isDefinedBy <measure/v1.0.0/> ;
  rdfs:subPropertyOf ieso:hasVoltageMagnitude ;
  .
# !


###  https://www.gecad.isep.ipp.pt/ieso/v1.0.0/hasVoltageMagnitudeAtHighVoltageBus
ieso:hasVoltageMagnitudeAtHighVoltageBus
  rdf:type owl:ObjectProperty ;
  rdfs:comment "The 'has voltage magnitude at high voltage bus' object property relates a class or individual with its voltage magnitude at high voltage bus."@en ;
  rdfs:label "has voltage magnitude at high voltage bus"@en ;
  rdfs:isDefinedBy <measure/v1.0.0/> ;
  rdfs:subPropertyOf ieso:hasVoltageMagnitude ;
  .
# !


###  https://www.gecad.isep.ipp.pt/ieso/v1.0.0/hasVoltageMagnitudeAtLowVoltageBus
ieso:hasVoltageMagnitudeAtLowVoltageBus
  rdf:type owl:ObjectProperty ;
  rdfs:comment "The 'has voltage magnitude at low voltage bus' object property relates a class or individual with its voltage magnitude at low voltage bus."@en ;
  rdfs:label "has voltage magnitude at low voltage bus"@en ;
  rdfs:isDefinedBy <measure/v1.0.0/> ;
  rdfs:subPropertyOf ieso:hasVoltageMagnitude ;
  .
# !


###  https://www.gecad.isep.ipp.pt/ieso/v1.0.0/hasVoltageMagnitudeAtMediumVoltageBus
ieso:hasVoltageMagnitudeAtMediumVoltageBus
  rdf:type owl:ObjectProperty ;
  rdfs:comment "The 'has voltage magnitude at medium voltage bus' object property relates a class or individual with its voltage magnitude at medium voltage bus."@en ;
  rdfs:label "has voltage magnitude at medium voltage bus"@en ;
  rdfs:isDefinedBy <measure/v1.0.0/> ;
  rdfs:subPropertyOf ieso:hasVoltageMagnitude ;
  .
# !


###  https://www.gecad.isep.ipp.pt/ieso/v1.0.0/hasMaximumVoltageMagnitude
ieso:hasMaximumVoltageMagnitude
  rdf:type owl:ObjectProperty ;
  rdfs:comment "The 'has maximum voltage magnitude' object property relates a class or individual with its maximum voltage magnitude."@en ;
  rdfs:label "has maximum voltage magnitude"@en ;
  rdfs:isDefinedBy <measure/v1.0.0/> ;
  rdfs:subPropertyOf
    ieso:hasMaximumMagnitude ,
    ieso:hasVoltageMagnitude ;
  .
# !


###  https://www.gecad.isep.ipp.pt/ieso/v1.0.0/hasMinimumVoltageMagnitude
ieso:hasMinimumVoltageMagnitude
  rdf:type owl:ObjectProperty ;
  rdfs:comment "The 'has minimum voltage magnitude' object property relates a class or individual with its minimum voltage magnitude."@en ;
  rdfs:label "has minimum voltage magnitude"@en ;
  rdfs:isDefinedBy <measure/v1.0.0/> ;
  rdfs:subPropertyOf
    ieso:hasMinimumMagnitude ,
    ieso:hasVoltageMagnitude ;
  .
# !


###  https://www.gecad.isep.ipp.pt/ieso/v1.0.0/hasPercentage
ieso:hasPercentage
  rdf:type owl:ObjectProperty ;
  rdfs:comment "The 'has percentage' object property relates a class or individual with its percentage."@en ;
  rdfs:label "has percentage"@en ;
  rdfs:isDefinedBy <measure/v1.0.0/> ;
  rdfs:subPropertyOf ieso:hasMeasurement ;
  .
# !


###  https://www.gecad.isep.ipp.pt/ieso/v1.0.0/hasConstantIPercentage
ieso:hasConstantIPercentage
  rdf:type owl:ObjectProperty ;
  rdfs:comment "The 'has constant I percentage' object property relates a class or individual with its constant I percentage."@en ;
  rdfs:label "has constant I percentage"@en ;
  rdfs:isDefinedBy <measure/v1.0.0/> ;
  rdfs:subPropertyOf ieso:hasPercentage ;
  .
# !


###  https://www.gecad.isep.ipp.pt/ieso/v1.0.0/hasConstantZPercentage
ieso:hasConstantZPercentage
  rdf:type owl:ObjectProperty ;
  rdfs:comment "The 'has constant Z percentage' object property relates a class or individual with its constant Z percentage."@en ;
  rdfs:label "has constant Z percentage"@en ;
  rdfs:isDefinedBy <measure/v1.0.0/> ;
  rdfs:subPropertyOf ieso:hasPercentage ;
  .
# !


###  https://www.gecad.isep.ipp.pt/ieso/v1.0.0/hasEfficiencyPercentage
ieso:hasEfficiencyPercentage
  rdf:type owl:ObjectProperty ;
  rdfs:comment "The 'has efficiency percentage' object property relates a class or individual with its efficiency percentage."@en ;
  rdfs:label "has efficiency percentage"@en ;
  rdfs:isDefinedBy <measure/v1.0.0/> ;
  rdfs:subPropertyOf ieso:hasPercentage ;
  .
# !


###  https://www.gecad.isep.ipp.pt/ieso/v1.0.0/hasLoadingPercentage
ieso:hasLoadingPercentage
  rdf:type owl:ObjectProperty ;
  rdfs:comment "The 'has loading percentage' object property relates a class or individual with its loading percentage."@en ;
  rdfs:label "has loading percentage"@en ;
  rdfs:isDefinedBy <measure/v1.0.0/> ;
  rdfs:subPropertyOf ieso:hasPercentage ;
  .
# !


###  https://www.gecad.isep.ipp.pt/ieso/v1.0.0/hasLossPercentage
ieso:hasLossPercentage
  rdf:type owl:ObjectProperty ;
  rdfs:comment "The 'has loss percentage' object property relates a class or individual with its loss percentage."@en ;
  rdfs:label "has loss percentage"@en ;
  rdfs:isDefinedBy <measure/v1.0.0/> ;
  rdfs:subPropertyOf ieso:hasPercentage ;
  .
# !


###  https://www.gecad.isep.ipp.pt/ieso/v1.0.0/hasOpenLoopLossPercentage
ieso:hasOpenLoopLossPercentage
  rdf:type owl:ObjectProperty ;
  rdfs:comment "The 'has open loop loss percentage' object property relates a class or individual with its open loop loss percentage."@en ;
  rdfs:label "has open loop loss percentage"@en ;
  rdfs:isDefinedBy <measure/v1.0.0/> ;
  rdfs:subPropertyOf ieso:hasLossPercentage ;
  .
# !


###  https://www.gecad.isep.ipp.pt/ieso/v1.0.0/hasRealPartOfRelativeShortCircuitVoltagePercentage
ieso:hasRealPartOfRelativeShortCircuitVoltagePercentage
  rdf:type owl:ObjectProperty ;
  rdfs:comment "The 'has real part of relative short-circuit voltage percentage' object property relates a class or individual with its real part of relative short-circuit voltage percentage."@en ;
  rdfs:label "has real part of relative short-circuit voltage percentage"@en ;
  rdfs:isDefinedBy <measure/v1.0.0/> ;
  rdfs:subPropertyOf ieso:hasPercentage ;
  .
# !


###  https://www.gecad.isep.ipp.pt/ieso/v1.0.0/hasRelativeShortCircuitVoltagePercentage
ieso:hasRelativeShortCircuitVoltagePercentage
  rdf:type owl:ObjectProperty ;
  rdfs:comment "The 'has relative short-circuit voltage percentage' object property relates a class or individual with its relative short-circuit voltage percentage."@en ;
  rdfs:label "has relative short-circuit voltage percentage"@en ;
  rdfs:isDefinedBy <measure/v1.0.0/> ;
  rdfs:subPropertyOf ieso:hasPercentage ;
  .
# !


###  https://www.gecad.isep.ipp.pt/ieso/v1.0.0/hasStateOfChargePercentage
ieso:hasStateOfChargePercentage
  rdf:type owl:ObjectProperty ;
  rdfs:comment "The 'has state of charge percentage' object property relates a class or individual with its state of charge percentage."@en ;
  rdfs:label "has state of charge percentage"@en ;
  rdfs:isDefinedBy <measure/v1.0.0/> ;
  rdfs:subPropertyOf ieso:hasPercentage ;
  .
# !


###  https://www.gecad.isep.ipp.pt/ieso/v1.0.0/hasZeroSequenceMagnetizingPercentage
ieso:hasZeroSequenceMagnetizingPercentage
  rdf:type owl:ObjectProperty ;
  rdfs:comment "The 'has zero sequence magnetizing percentage' object property relates a class or individual with its zero sequence magnetizing percentage."@en ;
  rdfs:label "has zero sequence magnetizing percentage"@en ;
  rdfs:isDefinedBy <measure/v1.0.0/> ;
  rdfs:subPropertyOf ieso:hasPercentage ;
  .
# !


###  https://www.gecad.isep.ipp.pt/ieso/v1.0.0/hasPower
ieso:hasPower
  rdf:type owl:ObjectProperty ;
  rdfs:comment "The 'has power' object property relates a class or individual with its power."@en ;
  rdfs:label "has power"@en ;
  rdfs:isDefinedBy <measure/v1.0.0/> ;
  rdfs:subPropertyOf ieso:hasMeasurement ;
  .
# !


###  https://www.gecad.isep.ipp.pt/ieso/v1.0.0/hasActivePower
ieso:hasActivePower
  rdf:type owl:ObjectProperty ;
  rdfs:comment "The 'has active power' object property relates a class or individual with its active power."@en ;
  rdfs:label "has active power"@en ;
  rdfs:isDefinedBy <measure/v1.0.0/> ;
  rdfs:subPropertyOf ieso:hasPower ;
  .
# !


###  https://www.gecad.isep.ipp.pt/ieso/v1.0.0/hasActivePowerFlow
ieso:hasActivePowerFlow
  rdf:type owl:ObjectProperty ;
  rdfs:comment "The 'has active power flow' object property relates a class or individual with its active power flow."@en ;
  rdfs:label "has active power flow"@en ;
  rdfs:isDefinedBy <measure/v1.0.0/> ;
  rdfs:subPropertyOf ieso:hasActivePower ;
  .
# !


###  https://www.gecad.isep.ipp.pt/ieso/v1.0.0/hasActivePowerFlowAtFromBus
ieso:hasActivePowerFlowAtFromBus
  rdf:type owl:ObjectProperty ;
  rdfs:comment "The 'has active power flow at from bus' object property relates a class or individual with its active power flow at 'from bus'."@en ;
  rdfs:label "has active power flow at from bus"@en ;
  rdfs:isDefinedBy <measure/v1.0.0/> ;
  rdfs:subPropertyOf ieso:hasActivePowerFlow ;
  .
# !


###  https://www.gecad.isep.ipp.pt/ieso/v1.0.0/hasActivePowerFlowAtToBus
ieso:hasActivePowerFlowAtToBus
  rdf:type owl:ObjectProperty ;
  rdfs:comment "The 'has active power flow at to bus' object property relates a class or individual with its active power flow at 'to bus'."@en ;
  rdfs:label "has active power flow at to bus"@en ;
  rdfs:isDefinedBy <measure/v1.0.0/> ;
  rdfs:subPropertyOf ieso:hasActivePowerFlow ;
  .
# !


###  https://www.gecad.isep.ipp.pt/ieso/v1.0.0/hasActivePowerFlowAtHighVoltageBus
ieso:hasActivePowerFlowAtHighVoltageBus
  rdf:type owl:ObjectProperty ;
  rdfs:comment "The 'has active power flow at high voltage bus' object property relates a class or individual with its active power flow at high voltage bus."@en ;
  rdfs:label "has active power flow at high voltage bus"@en ;
  rdfs:isDefinedBy <measure/v1.0.0/> ;
  rdfs:subPropertyOf ieso:hasActivePowerFlow ;
  .
# !


###  https://www.gecad.isep.ipp.pt/ieso/v1.0.0/hasActivePowerFlowAtLowVoltageBus
ieso:hasActivePowerFlowAtLowVoltageBus
  rdf:type owl:ObjectProperty ;
  rdfs:comment "The 'has active power flow at low voltage bus' object property relates a class or individual with its active power flow at low voltage bus."@en ;
  rdfs:label "has active power flow at low voltage bus"@en ;
  rdfs:isDefinedBy <measure/v1.0.0/> ;
  rdfs:subPropertyOf ieso:hasActivePowerFlow ;
  .
# !


###  https://www.gecad.isep.ipp.pt/ieso/v1.0.0/hasActivePowerFlowAtMediumVoltageBus
ieso:hasActivePowerFlowAtMediumVoltageBus
  rdf:type owl:ObjectProperty ;
  rdfs:comment "The 'has active power flow at medium voltage bus' object property relates a class or individual with its active power flow at medium voltage bus."@en ;
  rdfs:label "has active power flow at medium voltage bus"@en ;
  rdfs:isDefinedBy <measure/v1.0.0/> ;
  rdfs:subPropertyOf ieso:hasActivePowerFlow ;
  .
# !


###  https://www.gecad.isep.ipp.pt/ieso/v1.0.0/hasActivePowerLoss
ieso:hasActivePowerLoss
  rdf:type owl:ObjectProperty ;
  rdfs:comment "The 'has active power loss' object property relates a class or individual with its active power loss."@en ;
  rdfs:label "has active power loss"@en ;
  rdfs:isDefinedBy <measure/v1.0.0/> ;
  rdfs:subPropertyOf ieso:hasActivePower ;
  .
# !


###  https://www.gecad.isep.ipp.pt/ieso/v1.0.0/hasMaximumActivePower
ieso:hasMaximumActivePower
  rdf:type owl:ObjectProperty ;
  rdfs:comment "The 'has maximum active power' object property relates a class or individual with its maximum active power."@en ;
  rdfs:label "has maximum active power"@en ;
  rdfs:isDefinedBy <measure/v1.0.0/> ;
  rdfs:subPropertyOf ieso:hasActivePower ;
  .
# !


###  https://www.gecad.isep.ipp.pt/ieso/v1.0.0/hasMinimumActivePower
ieso:hasMinimumActivePower
  rdf:type owl:ObjectProperty ;
  rdfs:comment "The 'has minimum active power' object property relates a class or individual with its minimum active power."@en ;
  rdfs:label "has minimum active power"@en ;
  rdfs:isDefinedBy <measure/v1.0.0/> ;
  rdfs:subPropertyOf ieso:hasActivePower ;
  .
# !


###  https://www.gecad.isep.ipp.pt/ieso/v1.0.0/hasApparentNominalPower
ieso:hasApparentNominalPower
  rdf:type owl:ObjectProperty ;
  rdfs:comment "The 'has apparent nominal power' object property relates a class or individual with its apparent nominal power."@en ;
  rdfs:label "has apparent nominal power"@en ;
  rdfs:isDefinedBy <measure/v1.0.0/> ;
  rdfs:subPropertyOf ieso:hasPower ;
  .
# !


###  https://www.gecad.isep.ipp.pt/ieso/v1.0.0/hasApparentPower
ieso:hasApparentPower
  rdf:type owl:ObjectProperty ;
  rdfs:comment "The 'has apparent power' object property relates a class or individual with its apparent power."@en ;
  rdfs:label "has apparent power"@en ;
  rdfs:isDefinedBy <measure/v1.0.0/> ;
  rdfs:subPropertyOf ieso:hasPower ;
  .
# !


###  https://www.gecad.isep.ipp.pt/ieso/v1.0.0/hasMaximumShortCircuitApparentPower
ieso:hasMaximumShortCircuitApparentPower
  rdf:type owl:ObjectProperty ;
  rdfs:comment "The 'has maximum short circuit apparent power' object property relates a class or individual with its maximum short circuit apparent power."@en ;
  rdfs:label "has maximum short circuit apparent power"@en ;
  rdfs:isDefinedBy <measure/v1.0.0/> ;
  rdfs:subPropertyOf ieso:hasApparentPower ;
  .
# !


###  https://www.gecad.isep.ipp.pt/ieso/v1.0.0/hasMinimumShortCircuitApparentPower
ieso:hasMinimumShortCircuitApparentPower
  rdf:type owl:ObjectProperty ;
  rdfs:comment "The 'has minimum short circuit apparent power' object property relates a class or individual with its minimum short circuit apparent power."@en ;
  rdfs:label "has minimum short circuit apparent power"@en ;
  rdfs:isDefinedBy <measure/v1.0.0/> ;
  rdfs:subPropertyOf ieso:hasApparentPower ;
  .
# !


###  https://www.gecad.isep.ipp.pt/ieso/v1.0.0/hasBasePower
ieso:hasBasePower
  rdf:type owl:ObjectProperty ;
  rdfs:comment "The 'has base power' object property relates a class or individual with its base power."@en ;
  rdfs:label "has base power"@en ;
  rdfs:isDefinedBy <measure/v1.0.0/> ;
  rdfs:subPropertyOf ieso:hasPower ;
  .
# !


###  https://www.gecad.isep.ipp.pt/ieso/v1.0.0/hasNominalPower
ieso:hasNominalPower
  rdf:type owl:ObjectProperty ;
  rdfs:comment "The 'has nominal power' object property relates a class or individual with its nominal power."@en ;
  rdfs:label "has nominal power"@en ;
  rdfs:isDefinedBy <measure/v1.0.0/> ;
  rdfs:subPropertyOf ieso:hasPower ;
  .
# !


###  https://www.gecad.isep.ipp.pt/ieso/v1.0.0/hasPowerLoss
ieso:hasPowerLoss
  rdf:type owl:ObjectProperty ;
  rdfs:comment "The 'has power loss' object property relates a class or individual with its power loss."@en ;
  rdfs:label "has power loss"@en ;
  rdfs:isDefinedBy <measure/v1.0.0/> ;
  rdfs:subPropertyOf ieso:hasPower ;
  .
# !


###  https://www.gecad.isep.ipp.pt/ieso/v1.0.0/hasReactivePower
ieso:hasReactivePower
  rdf:type owl:ObjectProperty ;
  rdfs:comment "The 'has reactive power' object property relates a class or individual with its reactive power."@en ;
  rdfs:label "has reactive power"@en ;
  rdfs:isDefinedBy <measure/v1.0.0/> ;
  rdfs:subPropertyOf ieso:hasPower ;
  .
# !


###  https://www.gecad.isep.ipp.pt/ieso/v1.0.0/hasMaximumReactivePower
ieso:hasMaximumReactivePower
  rdf:type owl:ObjectProperty ;
  rdfs:comment "The 'has maximum reactive power' object property relates a class or individual with its maximum reactive power."@en ;
  rdfs:label "has maximum reactive power"@en ;
  rdfs:isDefinedBy <measure/v1.0.0/> ;
  rdfs:subPropertyOf ieso:hasReactivePower ;
  .
# !


###  https://www.gecad.isep.ipp.pt/ieso/v1.0.0/hasMinimumReactivePower
ieso:hasMinimumReactivePower
  rdf:type owl:ObjectProperty ;
  rdfs:comment "The 'has minimum reactive power' object property relates a class or individual with its minimum reactive power."@en ;
  rdfs:label "has minimum reactive power"@en ;
  rdfs:isDefinedBy <measure/v1.0.0/> ;
  rdfs:subPropertyOf ieso:hasReactivePower ;
  .
# !


###  https://www.gecad.isep.ipp.pt/ieso/v1.0.0/hasReactivePowerConsumption
ieso:hasReactivePowerConsumption
  rdf:type owl:ObjectProperty ;
  rdfs:comment "The 'has reactive power consumption' object property relates a class or individual with its reactive power consumption."@en ;
  rdfs:label "has reactive power consumption"@en ;
  rdfs:isDefinedBy <measure/v1.0.0/> ;
  rdfs:subPropertyOf ieso:hasReactivePower ;
  .
# !


###  https://www.gecad.isep.ipp.pt/ieso/v1.0.0/hasReactivePowerFlow
ieso:hasReactivePowerFlow
  rdf:type owl:ObjectProperty ;
  rdfs:comment "The 'has reactive power flow' object property relates a class or individual with its reactive power flow."@en ;
  rdfs:label "has reactive power flow"@en ;
  rdfs:isDefinedBy <measure/v1.0.0/> ;
  rdfs:subPropertyOf ieso:hasReactivePower ;
  .
# !


###  https://www.gecad.isep.ipp.pt/ieso/v1.0.0/hasReactivePowerFlowAtFromBus
ieso:hasReactivePowerFlowAtFromBus
  rdf:type owl:ObjectProperty ;
  rdfs:comment "The 'has reactive power flow at from bus' object property relates a class or individual with its reactive power flow at 'from bus'."@en ;
  rdfs:label "has reactive power flow at from bus"@en ;
  rdfs:isDefinedBy <measure/v1.0.0/> ;
  rdfs:subPropertyOf ieso:hasReactivePower ;
  .
# !


###  https://www.gecad.isep.ipp.pt/ieso/v1.0.0/hasReactivePowerFlowAtToBus
ieso:hasReactivePowerFlowAtToBus
  rdf:type owl:ObjectProperty ;
  rdfs:comment "The 'has reactive power flow at to bus' object property relates a class or individual with its reactive power flow at 'to bus'."@en ;
  rdfs:label "has reactive power flow at to bus"@en ;
  rdfs:isDefinedBy <measure/v1.0.0/> ;
  rdfs:subPropertyOf ieso:hasReactivePower ;
  .
# !


###  https://www.gecad.isep.ipp.pt/ieso/v1.0.0/hasReactivePowerFlowAtHighVoltageBus
ieso:hasReactivePowerFlowAtHighVoltageBus
  rdf:type owl:ObjectProperty ;
  rdfs:comment "The 'has reactive power flow at high voltage bus' object property relates a class or individual with its reactive power flow at high voltage bus."@en ;
  rdfs:label "has reactive power flow at high voltage bus"@en ;
  rdfs:isDefinedBy <measure/v1.0.0/> ;
  rdfs:subPropertyOf ieso:hasReactivePower ;
  .
# !


###  https://www.gecad.isep.ipp.pt/ieso/v1.0.0/hasReactivePowerFlowAtLowVoltageBus
ieso:hasReactivePowerFlowAtLowVoltageBus
  rdf:type owl:ObjectProperty ;
  rdfs:comment "The 'has reactive power flow at low voltage bus' object property relates a class or individual with its reactive power flow at low voltage bus."@en ;
  rdfs:label "has reactive power flow at low voltage bus"@en ;
  rdfs:isDefinedBy <measure/v1.0.0/> ;
  rdfs:subPropertyOf ieso:hasReactivePower ;
  .
# !


###  https://www.gecad.isep.ipp.pt/ieso/v1.0.0/hasReactivePowerFlowAtMediumVoltageBus
ieso:hasReactivePowerFlowAtMediumVoltageBus
  rdf:type owl:ObjectProperty ;
  rdfs:comment "The 'has reactive power flow at medium voltage bus' object property relates a class or individual with its reactive power flow at medium voltage bus."@en ;
  rdfs:label "has reactive power flow at medium voltage bus"@en ;
  rdfs:isDefinedBy <measure/v1.0.0/> ;
  rdfs:subPropertyOf ieso:hasReactivePower ;
  .
# !


###  https://www.gecad.isep.ipp.pt/ieso/v1.0.0/hasMaximumReactivePowerFlow
ieso:hasMaximumReactivePowerFlow
  rdf:type owl:ObjectProperty ;
  rdfs:comment "The 'has maximum reactive power flow' object property relates a class or individual with its maximum reactive power flow."@en ;
  rdfs:label "has maximum reactive power flow"@en ;
  rdfs:isDefinedBy <measure/v1.0.0/> ;
  rdfs:subPropertyOf ieso:hasReactivePowerFlow ;
  .
# !


###  https://www.gecad.isep.ipp.pt/ieso/v1.0.0/hasMinimumReactivePowerFlow
ieso:hasMinimumReactivePowerFlow
  rdf:type owl:ObjectProperty ;
  rdfs:comment "The 'has minimum reactive power flow' object property relates a class or individual with its minimum reactive power flow."@en ;
  rdfs:label "has minimum reactive power flow"@en ;
  rdfs:isDefinedBy <measure/v1.0.0/> ;
  rdfs:subPropertyOf ieso:hasReactivePowerFlow ;
  .
# !


###  https://www.gecad.isep.ipp.pt/ieso/v1.0.0/hasRatio
ieso:hasRatio
  rdf:type owl:ObjectProperty ;
  rdfs:comment "The 'has ratio' object property relates a class or individual with its ratio."@en ;
  rdfs:label "has ratio"@en ;
  rdfs:isDefinedBy <measure/v1.0.0/> ;
  rdfs:subPropertyOf ieso:hasMeasurement ;
  .
# !


###  https://www.gecad.isep.ipp.pt/ieso/v1.0.0/hasMaximumRatio
ieso:hasMaximumRatio
  rdf:type owl:ObjectProperty ;
  rdfs:comment "The 'has maximum ratio' object property relates a class or individual with its maximum ratio."@en ;
  rdfs:label "has maximum ratio"@en ;
  rdfs:isDefinedBy <measure/v1.0.0/> ;
  rdfs:subPropertyOf ieso:hasRatio ;
  .
# !


###  https://www.gecad.isep.ipp.pt/ieso/v1.0.0/hasMaximumZeroSequenceRXRatio
ieso:hasMaximumZeroSequenceRXRatio
  rdf:type owl:ObjectProperty ;
  rdfs:comment "The 'has maximum zero sequence RX ratio' object property relates a class or individual with its maximum zero sequence RX ratio."@en ;
  rdfs:label "has maximum zero sequence RX ratio"@en ;
  rdfs:isDefinedBy <measure/v1.0.0/> ;
  rdfs:subPropertyOf ieso:hasMaximumRatio ;
  .
# !


###  https://www.gecad.isep.ipp.pt/ieso/v1.0.0/hasMaximumZeroSequenceXXRatio
ieso:hasMaximumZeroSequenceXXRatio
  rdf:type owl:ObjectProperty ;
  rdfs:comment "The 'has maximum zero sequence XX ratio' object property relates a class or individual with its maximum zero sequence XX ratio."@en ;
  rdfs:label "has maximum zero sequence XX ratio"@en ;
  rdfs:isDefinedBy <measure/v1.0.0/> ;
  rdfs:subPropertyOf ieso:hasMaximumRatio ;
  .
# !


###  https://www.gecad.isep.ipp.pt/ieso/v1.0.0/hasZeroSequenceMagnetizingRatio
ieso:hasZeroSequenceMagnetizingRatio
  rdf:type owl:ObjectProperty ;
  rdfs:comment "The 'has zero sequence magnetizing ratio' object property relates a class or individual with its zero sequence magnetizing ratio."@en ;
  rdfs:label "has zero sequence magnetizing ratio"@en ;
  rdfs:isDefinedBy <measure/v1.0.0/> ;
  rdfs:subPropertyOf ieso:hasRatio ;
  .
# !


###  https://www.gecad.isep.ipp.pt/ieso/v1.0.0/hasReactance
ieso:hasReactance
  rdf:type owl:ObjectProperty ;
  rdfs:comment "The 'has reactance' object property relates a class or individual with its reactance."@en ;
  rdfs:label "has reactance"@en ;
  rdfs:isDefinedBy <measure/v1.0.0/> ;
  rdfs:subPropertyOf ieso:hasMeasurement ;
  owl:equivalentProperty ieso:hasImaginaryPartOfImpedance ;
  .
# !


###  https://www.gecad.isep.ipp.pt/ieso/v1.0.0/hasZeroSequenceReactance
ieso:hasZeroSequenceReactance
  rdf:type owl:ObjectProperty ;
  rdfs:comment "The 'has zero sequence reactance' object property relates a class or individual with its zero sequence reactance."@en ;
  rdfs:label "has zero sequence reactance"@en ;
  rdfs:isDefinedBy <measure/v1.0.0/> ;
  rdfs:subPropertyOf ieso:hasReactance ;
  .
# !


###  https://www.gecad.isep.ipp.pt/ieso/v1.0.0/hasResistance
ieso:hasResistance
  rdf:type owl:ObjectProperty ;
  rdfs:comment "The 'has resistance' object property relates a class or individual with its resistance."@en ;
  rdfs:label "has resistance"@en ;
  rdfs:isDefinedBy <measure/v1.0.0/> ;
  rdfs:subPropertyOf ieso:hasMeasurement ;
  owl:equivalentProperty ieso:hasRealPartOfImpedance ;
  .
# !


###  https://www.gecad.isep.ipp.pt/ieso/v1.0.0/hasZeroSequenceResistance
ieso:hasZeroSequenceResistance
  rdf:type owl:ObjectProperty ;
  rdfs:comment "The 'has zero sequence resistance' object property relates a class or individual with its zero sequence resistance."@en ;
  rdfs:label "has zero sequence resistance"@en ;
  rdfs:isDefinedBy <measure/v1.0.0/> ;
  rdfs:subPropertyOf ieso:hasResistance ;
  .
# !


###  https://www.gecad.isep.ipp.pt/ieso/v1.0.0/hasTemperature
ieso:hasTemperature
  rdf:type owl:ObjectProperty ;
  rdfs:comment "The 'has temperature' object property relates a class or individual with its temperature."@en ;
  rdfs:label "has temperature"@en ;
  rdfs:isDefinedBy <measure/v1.0.0/> ;
  rdfs:subPropertyOf ieso:hasMeasurement ;
  .
# !


###  https://www.gecad.isep.ipp.pt/ieso/v1.0.0/hasEndTemperature
ieso:hasEndTemperature
  rdf:type owl:ObjectProperty ;
  rdfs:comment "The 'has end temperature' object property relates a class or individual with its end temperature."@en ;
  rdfs:label "has end temperature"@en ;
  rdfs:isDefinedBy <measure/v1.0.0/> ;
  rdfs:subPropertyOf ieso:hasTemperature ;
  .
# !


###  https://www.gecad.isep.ipp.pt/ieso/v1.0.0/hasVoltage
ieso:hasVoltage
  rdf:type owl:ObjectProperty ;
  rdfs:comment "The 'has voltage' object property relates a class or individual with its voltage."@en ;
  rdfs:label "has voltage"@en ;
  rdfs:isDefinedBy <measure/v1.0.0/> ;
  rdfs:subPropertyOf ieso:hasMeasurement ;
  .
# !


###  https://www.gecad.isep.ipp.pt/ieso/v1.0.0/hasMaximumVoltage
ieso:hasMaximumVoltage
  rdf:type owl:ObjectProperty ;
  rdfs:comment "The 'has maximum voltage' object property relates a class or individual with its maximum voltage."@en ;
  rdfs:label "has maximum voltage"@en ;
  rdfs:isDefinedBy <measure/v1.0.0/> ;
  rdfs:subPropertyOf ieso:hasVoltage ;
  .
# !


###  https://www.gecad.isep.ipp.pt/ieso/v1.0.0/hasMinimumVoltage
ieso:hasMinimumVoltage
  rdf:type owl:ObjectProperty ;
  rdfs:comment "The 'has minimum voltage' object property relates a class or individual with its minimum voltage."@en ;
  rdfs:label "has minimum voltage"@en ;
  rdfs:isDefinedBy <measure/v1.0.0/> ;
  rdfs:subPropertyOf ieso:hasVoltage ;
  .
# !


###  https://www.gecad.isep.ipp.pt/ieso/v1.0.0/hasRatedVoltage
ieso:hasRatedVoltage
  rdf:type owl:ObjectProperty ;
  rdfs:comment "The 'has rated voltage' object property relates a class or individual with its rated voltage."@en ;
  rdfs:label "has rated voltage"@en ;
  rdfs:isDefinedBy <measure/v1.0.0/> ;
  rdfs:subPropertyOf ieso:hasVoltage ;
  .
# !


###  https://www.gecad.isep.ipp.pt/ieso/v1.0.0/hasRatedVoltageOnHighVoltageSide
ieso:hasRatedVoltageOnHighVoltageSide
  rdf:type owl:ObjectProperty ;
  rdfs:comment "The 'has rated voltage on high voltage side' object property relates a Transformer with its rated voltage on the high voltage side."@en ;
  rdfs:label "has rated voltage on high voltage side"@en ;
  rdfs:isDefinedBy <measure/v1.0.0/> ;
  rdfs:subPropertyOf ieso:hasRatedVoltage ;
  .
# !


###  https://www.gecad.isep.ipp.pt/ieso/v1.0.0/hasRatedVoltageOnLowVoltageSide
ieso:hasRatedVoltageOnLowVoltageSide
  rdf:type owl:ObjectProperty ;
  rdfs:comment "The 'has rated voltage on low voltage side' object property relates a Transformer with its rated voltage on the low voltage side."@en ;
  rdfs:label "has rated voltage on low voltage side"@en ;
  rdfs:isDefinedBy <measure/v1.0.0/> ;
  rdfs:subPropertyOf ieso:hasRatedVoltage ;
  .
# !


###  https://www.gecad.isep.ipp.pt/ieso/v1.0.0/hasRatedVoltageOnMediumVoltageSide
ieso:hasRatedVoltageOnMediumVoltageSide
  rdf:type owl:ObjectProperty ;
  rdfs:comment "The 'has rated voltage on medium voltage side' object property relates a Transformer with its rated voltage on the medium voltage side."@en ;
  rdfs:label "has rated voltage on medium voltage side"@en ;
  rdfs:isDefinedBy <measure/v1.0.0/> ;
  rdfs:subPropertyOf ieso:hasRatedVoltage ;
  .
# !


###  https://www.gecad.isep.ipp.pt/ieso/v1.0.0/hasMeasurementValue
ieso:hasMeasurementValue
  rdf:type owl:ObjectProperty ;
  rdfs:comment "The 'has measurement value' object property relates a 'Measurement' with a 'Measurement value'."@en ;
  rdfs:label "has measurement value"@en ;
  rdfs:isDefinedBy <measure/v1.0.0/> ;
  rdfs:domain ieso:Measurement ;
  rdfs:range ieso:MeasurementValue ;
  owl:inverseOf ieso:isMeasurementValueOf ;
  .
# !


###  https://www.gecad.isep.ipp.pt/ieso/v1.0.0/hasSIUnitOfMeasure
ieso:hasSIUnitOfMeasure
  rdf:type owl:ObjectProperty ;
  rdfs:comment "The 'has SI unit of measure' object property relates a 'Unit of measure' with its SI 'Unit of Measure'. This relation allows to set a 'unit conversion coefficient' relative to a base 'Unit of Measure'."@en ;
  rdfs:label "has SI unit of measure"@en ;
  rdfs:isDefinedBy <measure/v1.0.0/> ;
  rdfs:seeAlso <https://en.wikipedia.org/wiki/Conversion_of_units> ;
  rdfs:domain ieso:DimensionalUnit ;
  rdfs:range ieso:DimensionalUnit ;
  .
# !


###  https://www.gecad.isep.ipp.pt/ieso/v1.0.0/hasTypeOfMeasure
ieso:hasTypeOfMeasure
  rdf:type owl:ObjectProperty ;
  rdfs:comment "The 'has type of measure' object property relates a 'Measurement' with a 'Type of measure'."@en ;
  rdfs:label "has type of measure"@en ;
  rdfs:isDefinedBy <measure/v1.0.0/> ;
  rdfs:domain ieso:Measurement ;
  rdfs:range ieso:TypeOfMeasure ;
  owl:inverseOf ieso:isTypeOfMeasureOf ;
  .
# !


###  https://www.gecad.isep.ipp.pt/ieso/v1.0.0/hasUnitOfMeasure
ieso:hasUnitOfMeasure
  rdf:type owl:ObjectProperty ;
  rdfs:comment "The 'has unit of measure' object property relates a 'Measurement', a 'Type of measure', or a 'Measurement value' with a 'Unit of measure'."@en ;
  rdfs:label "has unit of measure"@en ;
  rdfs:isDefinedBy <measure/v1.0.0/> ;
  rdfs:range ieso:UnitOfMeasure ;
  owl:inverseOf ieso:isUnitOfMeasureOf ;
  .
# !


###  https://www.gecad.isep.ipp.pt/ieso/v1.0.0/isMeasurementOf
ieso:isMeasurementOf
  rdf:type owl:ObjectProperty ;
  rdfs:comment "The 'is measurement of' object property relates a 'Measurement' with its class or individual."@en ;
  rdfs:label "is measurement of"@en ;
  rdfs:isDefinedBy <measure/v1.0.0/> ;
  rdfs:domain ieso:Measurement ;
  .
# !


###  https://www.gecad.isep.ipp.pt/ieso/v1.0.0/isMeasurementValueOf
ieso:isMeasurementValueOf
  rdf:type owl:ObjectProperty ;
  rdfs:comment "The 'is measurement value of' object property relates a 'Measurement value' with a 'Measurement'."@en ;
  rdfs:label "is measurement value of"@en ;
  rdfs:isDefinedBy <measure/v1.0.0/> ;
  rdfs:domain ieso:MeasurementValue ;
  rdfs:range ieso:Measurement ;
  .
# !


###  https://www.gecad.isep.ipp.pt/ieso/v1.0.0/isTypeOfMeasureOf
ieso:isTypeOfMeasureOf
  rdf:type owl:ObjectProperty ;
  rdfs:comment "The 'is type of measure of' object property relates a 'Type of measure' with a 'Measurement'."@en ;
  rdfs:label "is type of measure of"@en ;
  rdfs:isDefinedBy <measure/v1.0.0/> ;
  rdfs:domain ieso:TypeOfMeasure ;
  rdfs:range ieso:Measurement ;
  .
# !


###  https://www.gecad.isep.ipp.pt/ieso/v1.0.0/isUnitOfMeasureOf
ieso:isUnitOfMeasureOf
  rdf:type owl:ObjectProperty ;
  rdfs:comment "The 'is unit of measure of' object property relates a 'Unit of measure' with a 'Measurement', a 'Type of measure', or a 'Measurement value'."@en ;
  rdfs:label "is unit of measure of"@en ;
  rdfs:isDefinedBy <measure/v1.0.0/> ;
  rdfs:domain ieso:UnitOfMeasure ;
  .
# !


#################################################################
#  Classes
#################################################################


###  https://www.gecad.isep.ipp.pt/ieso/v1.0.0/AngleMeasure
ieso:AngleMeasure
  rdf:type owl:Class ;
  rdfs:comment "In Euclidean geometry, an angle is the figure formed by two rays, called the sides of the angle, sharing a common endpoint, called the vertex of the angle. Angles formed by two rays lie in the plane that contains the rays. Angles are also formed by the intersection of two planes. These are called dihedral angles. Two intersecting curves define also an angle, which is the angle of the tangents at the intersection point."@en ;
  rdfs:label "Angle measure"@en ;
  rdfs:isDefinedBy <measure/v1.0.0/> ;
  rdfs:seeAlso <https://en.wikipedia.org/wiki/Angle> ;
  rdfs:subClassOf
    ieso:TypeOfMeasure ,
    [
      rdf:type owl:Restriction ;
      owl:onProperty ieso:hasUnitOfMeasure ;
      owl:allValuesFrom ieso:AngleUnit
    ] ;
  .
# !


###  https://www.gecad.isep.ipp.pt/ieso/v1.0.0/AngleUnit
ieso:AngleUnit
  rdf:type owl:Class ;
  rdfs:comment "Throughout history, angles have been measured in many different units. These are known as angular units, with the most contemporary units being the degree (), the radian (rad), and the gradian (grad), though many others have been used throughout history."@en ;
  rdfs:label "Angle unit"@en ;
  rdfs:isDefinedBy <measure/v1.0.0/> ;
  rdfs:seeAlso
    <https://en.wikipedia.org/wiki/Angle#Units> ,
    <https://en.wikipedia.org/wiki/Angular_unit> ;
  rdfs:subClassOf
    ieso:DimensionalUnit ,
    [
      rdf:type owl:Restriction ;
      owl:onProperty ieso:isUnitOfMeasureOf ;
      owl:someValuesFrom ieso:AngleMeasure
    ] ,
    [
      rdf:type owl:Restriction ;
      owl:onProperty ieso:hasSIUnitOfMeasure ;
      owl:qualifiedCardinality "1"^^xsd:nonNegativeInteger ;
      owl:onClass ieso:AngleUnit
    ] ;
  .
# !


###  https://www.gecad.isep.ipp.pt/ieso/v1.0.0/AreaDensityMeasure
ieso:AreaDensityMeasure
  rdf:type owl:Class ;
  rdfs:comment "The area density (also known as areal density, surface density, superficial density, areic density, mass thickness, column density, or density thickness) of a two-dimensional object is calculated as the mass per unit area."@en ;
  rdfs:label "Area density measure"@en ;
  rdfs:isDefinedBy <measure/v1.0.0/> ;
  rdfs:seeAlso <https://en.wikipedia.org/wiki/Area_density> ;
  rdfs:subClassOf
    ieso:DensityMeasure ,
    [
      rdf:type owl:Restriction ;
      owl:onProperty ieso:hasUnitOfMeasure ;
      owl:allValuesFrom ieso:AreaDensityUnit
    ] ;
  .
# !


###  https://www.gecad.isep.ipp.pt/ieso/v1.0.0/AreaDensityUnit
ieso:AreaDensityUnit
  rdf:type owl:Class ;
  rdfs:comment "The SI derived unit is: kilogram per square metre (kgm^2)."@en ;
  rdfs:label "Area density unit"@en ;
  rdfs:isDefinedBy <measure/v1.0.0/> ;
  rdfs:seeAlso <https://en.wikipedia.org/wiki/Area_density> ;
  rdfs:subClassOf
    ieso:DensityUnit ,
    [
      rdf:type owl:Restriction ;
      owl:onProperty ieso:isUnitOfMeasureOf ;
      owl:someValuesFrom ieso:AreaDensityMeasure
    ] ,
    [
      rdf:type owl:Restriction ;
      owl:onProperty ieso:hasSIUnitOfMeasure ;
      owl:qualifiedCardinality "1"^^xsd:nonNegativeInteger ;
      owl:onClass ieso:AreaDensityUnit
    ] ;
  .
# !


###  https://www.gecad.isep.ipp.pt/ieso/v1.0.0/AreaMeasure
ieso:AreaMeasure
  rdf:type owl:Class ;
  rdfs:comment "Area is the quantity that expresses the extent of a two-dimensional region, shape, or planar lamina, in the plane. Surface area is its analog on the two-dimensional surface of a three-dimensional object."@en ;
  rdfs:label "Area measure"@en ;
  rdfs:isDefinedBy <measure/v1.0.0/> ;
  rdfs:seeAlso <https://en.wikipedia.org/wiki/Area> ;
  rdfs:subClassOf
    ieso:TypeOfMeasure ,
    [
      rdf:type owl:Restriction ;
      owl:onProperty ieso:hasUnitOfMeasure ;
      owl:allValuesFrom ieso:AreaUnit
    ] ;
  .
# !


###  https://www.gecad.isep.ipp.pt/ieso/v1.0.0/AreaUnit
ieso:AreaUnit
  rdf:type owl:Class ;
  rdfs:comment "The SI unit of area is the square metre, which is considered an SI derived unit. Every unit of length has a corresponding unit of area, namely the area of a square with the given side length. Thus areas can be measured in square metres (m2), square centimetres (cm2), square millimetres (mm2), square kilometres (km2), square feet (ft2), square yards (yd2), square miles (mi2), and so forth. Algebraically, these units can be thought of as the squares of the corresponding length units."@en ;
  rdfs:label "Area unit"@en ;
  rdfs:isDefinedBy <measure/v1.0.0/> ;
  rdfs:seeAlso <https://en.wikipedia.org/wiki/Area#Units> ;
  rdfs:subClassOf
    ieso:DimensionalUnit ,
    [
      rdf:type owl:Restriction ;
      owl:onProperty ieso:isUnitOfMeasureOf ;
      owl:someValuesFrom ieso:AreaMeasure
    ] ,
    [
      rdf:type owl:Restriction ;
      owl:onProperty ieso:hasSIUnitOfMeasure ;
      owl:qualifiedCardinality "1"^^xsd:nonNegativeInteger ;
      owl:onClass ieso:AreaUnit
    ] ;
  .
# !


###  FIX HERE  ###
###  https://www.gecad.isep.ipp.pt/ieso/v1.0.0/CapacitanceMeasure
ieso:CapacitanceMeasure
  rdf:type owl:Class ;
  rdfs:comment "Capacitance is the ratio of the amount of electric charge stored on a conductor to a difference in electric potential."@en ;
  rdfs:label "Capacitance measure"@en ;
  rdfs:isDefinedBy <measure/v1.0.0/> ;
  rdfs:seeAlso <https://en.wikipedia.org/wiki/Capacitance> ;
  rdfs:subClassOf
    ieso:TypeOfMeasure ,
    [
      rdf:type owl:Restriction ;
      owl:onProperty ieso:hasUnitOfMeasure ;
      owl:allValuesFrom ieso:CapacitanceUnit
    ] ;
  .
# !


###  FIX HERE  ###
###  https://www.gecad.isep.ipp.pt/ieso/v1.0.0/CapacitanceUnit
ieso:CapacitanceUnit
  rdf:type owl:Class ;
  rdfs:comment "The SI unit of capacitance is the farad (symbol: F). A 1 farad capacitor, when charged with 1 coulomb of electrical charge, has a potential difference of 1 volt between its plates. The reciprocal of capacitance is called elastance."@en ;
  rdfs:label "Capacitance unit"@en ;
  rdfs:isDefinedBy <measure/v1.0.0/> ;
  rdfs:seeAlso <https://en.wikipedia.org/wiki/Capacitance> ;
  rdfs:subClassOf
    ieso:DimensionalUnit ,
    [
      rdf:type owl:Restriction ;
      owl:onProperty ieso:isUnitOfMeasureOf ;
      owl:someValuesFrom ieso:CapacitanceMeasure
    ] ;
  .
# !


###  https://www.gecad.isep.ipp.pt/ieso/v1.0.0/CarbonDioxideMeasure
ieso:CarbonDioxideMeasure
  rdf:type owl:Class ;
  rdfs:comment "Carbon dioxide (chemical formula CO2) is a chemical compound made up of molecules that each have one carbon atom covalently double bonded to two oxygen atoms. It is found in the gas state at room temperature."@en ;
  rdfs:label "Carbon dioxide measure"@en ;
  rdfs:isDefinedBy <measure/v1.0.0/> ;
  rdfs:seeAlso <https://en.wikipedia.org/wiki/Carbon_dioxide> ;
  rdfs:subClassOf
    ieso:TypeOfMeasure ,
    [
      rdf:type owl:Restriction ;
      owl:onProperty ieso:hasUnitOfMeasure ;
      owl:allValuesFrom [
        rdf:Type owl:Class ;
        owl:unionOf (
          ieso:PercentageUnit
          ieso:PartsPerNotationUnit
        )
      ]
    ]
  .
# !


###  https://www.gecad.isep.ipp.pt/ieso/v1.0.0/CurrencyMeasure
ieso:CurrencyMeasure
  rdf:type owl:Class ;
  rdfs:comment "A currency in the most specific sense is money in any form when in use or circulation as a medium of exchange, especially circulating banknotes and coins. A more general definition is that a currency is a system of money (monetary units) in common use, especially for people in a nation."@en ;
  rdfs:label "Currency measure"@en ;
  rdfs:isDefinedBy <measure/v1.0.0/> ;
  rdfs:seeAlso <https://en.wikipedia.org/wiki/Currency> ;
  rdfs:subClassOf
    ieso:TypeOfMeasure ,
    [
      rdf:type owl:Restriction ;
      owl:onProperty ieso:hasUnitOfMeasure ;
      owl:allValuesFrom ieso:CurrencyUnit
    ] ;
  .
# !


###  https://www.gecad.isep.ipp.pt/ieso/v1.0.0/CurrencyUnit
ieso:CurrencyUnit
  rdf:type owl:Class ;
  rdfs:comment "There is no SI unit for currency. Examples of currencies are Euro (), US Dollar ($), and Pound ()."@en ;
  rdfs:label "Currency unit"@en ;
  rdfs:isDefinedBy <measure/v1.0.0/> ;
  rdfs:seeAlso <https://en.wikipedia.org/wiki/Currency> ;
  rdfs:subClassOf
    ieso:DimensionlessUnit ,
    [
      rdf:type owl:Restriction ;
      owl:onProperty ieso:isUnitOfMeasureOf ;
      owl:someValuesFrom ieso:CurrencyMeasure
    ] ;
  .
# !


###  https://www.gecad.isep.ipp.pt/ieso/v1.0.0/DensityMeasure
ieso:DensityMeasure
  rdf:type owl:Class ;
  rdfs:comment "The density measures the influence exerted by some mass."@en ;
  rdfs:label "Density measure"@en ;
  rdfs:isDefinedBy <measure/v1.0.0/> ;
  rdfs:seeAlso <https://en.wikipedia.org/wiki/Density> ;
  rdfs:subClassOf
    ieso:TypeOfMeasure ,
    [
      rdf:type owl:Restriction ;
      owl:onProperty ieso:hasUnitOfMeasure ;
      owl:allValuesFrom ieso:DensityUnit
    ] ;
  .
# !


###  https://www.gecad.isep.ipp.pt/ieso/v1.0.0/DensityUnit
ieso:DensityUnit
  rdf:type owl:Class ;
  rdfs:comment "A unit representing a standard measure of the influence exerted by some mass."@en ;
  rdfs:label "Density unit"@en ;
  rdfs:isDefinedBy <measure/v1.0.0/> ;
  rdfs:seeAlso <https://en.wikipedia.org/wiki/Density#Common_units> ;
  rdfs:subClassOf
    ieso:DimensionalUnit ,
    [
      rdf:type owl:Restriction ;
      owl:onProperty ieso:isUnitOfMeasureOf ;
      owl:someValuesFrom ieso:DensityMeasure
    ] ,
    [
      rdf:type owl:Restriction ;
      owl:onProperty ieso:hasSIUnitOfMeasure ;
      owl:qualifiedCardinality "1"^^xsd:nonNegativeInteger ;
      owl:onClass ieso:DensityUnit
    ] ;
  .
# !


###  https://www.gecad.isep.ipp.pt/ieso/v1.0.0/DimensionalUnit
ieso:DimensionalUnit
  rdf:type owl:Class ;
  rdfs:comment "In engineering and science, dimensional analysis is the analysis of the relationships between different physical quantities by identifying their base quantities (such as length, mass, time, and electric charge) and units of measure (such as miles vs. kilometres, or pounds vs. kilograms) and tracking these dimensions as calculations or comparisons are performed. The conversion of units from one dimensional unit to another is often easier within the metric or SI system than in others, due to the regular 10-base in all units."@en ;
  rdfs:label "Dimensional unit"@en ;
  rdfs:isDefinedBy <measure/v1.0.0/> ;
  rdfs:seeAlso <https://en.wikipedia.org/wiki/Dimensional_analysis> ;
  rdfs:subClassOf
    ieso:UnitOfMeasure ,
    [
      rdf:type owl:Restriction ;
      owl:onProperty ieso:hasSIUnitOfMeasure ;
      owl:allValuesFrom ieso:UnitOfMeasure
    ] ,
    [
      rdf:type owl:Restriction ;
      owl:onProperty ieso:conversionCoefficientToSIUnit ;
      owl:qualifiedCardinality "1"^^xsd:nonNegativeInteger ;
      owl:onDataRange xsd:double
    ] ,
    [
      rdf:type owl:Restriction ;
      owl:onProperty ieso:conversionOffsetToSIUnit ;
      owl:qualifiedCardinality "1"^^xsd:nonNegativeInteger ;
      owl:onDataRange xsd:double
    ] ;
  .
# !


###  https://www.gecad.isep.ipp.pt/ieso/v1.0.0/DimensionlessUnit
ieso:DimensionlessUnit
  rdf:type owl:Class ;
  rdfs:comment "In dimensional analysis, a dimensionless quantity is a quantity to which no physical dimension is assigned, also known as a bare, pure, or scalar quantity or a quantity of dimension one, with a corresponding unit of measurement in the SI of the unit one (or 1), which is not explicitly shown."@en ;
  rdfs:label "Dimensionless unit"@en ;
  rdfs:isDefinedBy <measure/v1.0.0/> ;
  rdfs:seeAlso <https://en.wikipedia.org/wiki/Dimensionless_quantity> ;
  rdfs:subClassOf ieso:UnitOfMeasure ;
  .
# !


###  https://www.gecad.isep.ipp.pt/ieso/v1.0.0/ElectricalAdmittanceMeasure
ieso:ElectricalAdmittanceMeasure
  rdf:type owl:Class ;
  rdfs:comment "In electrical engineering, admittance is a measure of how easily a circuit or device will allow a current to flow. It is defined as the reciprocal of impedance, analogous to how conductance & resistance are defined."@en ;
  rdfs:label "Electrical admittance measure"@en ;
  rdfs:isDefinedBy <measure/v1.0.0/> ;
  rdfs:seeAlso <https://en.wikipedia.org/wiki/Admittance> ;
  rdfs:subClassOf
    ieso:TypeOfMeasure ,
    [
      rdf:type owl:Restriction ;
      owl:onProperty ieso:hasUnitOfMeasure ;
      owl:allValuesFrom ieso:ElectricalAdmittanceUnit
    ] ;
  .
# !


###  https://www.gecad.isep.ipp.pt/ieso/v1.0.0/ElectricalAdmittanceUnit
ieso:ElectricalAdmittanceUnit
  rdf:type owl:Class ;
  rdfs:comment "The SI unit of admittance is the siemens (symbol S); the older, synonymous unit is mho, and its symbol is  (an upside-down uppercase omega )."@en ;
  rdfs:label "Electrical admittance unit"@en ;
  rdfs:isDefinedBy <measure/v1.0.0/> ;
  rdfs:seeAlso <https://en.wikipedia.org/wiki/Admittance> ;
  rdfs:subClassOf
    ieso:DimensionalUnit ,
    [
      rdf:type owl:Restriction ;
      owl:onProperty ieso:isUnitOfMeasureOf ;
      owl:someValuesFrom ieso:ElectricalAdmittanceMeasure
    ] ,
    [
      rdf:type owl:Restriction ;
      owl:onProperty ieso:hasSIUnitOfMeasure ;
      owl:qualifiedCardinality "1"^^xsd:nonNegativeInteger ;
      owl:onClass ieso:ElectricalAdmittanceUnit
    ] ;
  .
# !


###  https://www.gecad.isep.ipp.pt/ieso/v1.0.0/ElectricalConductanceMeasure
ieso:ElectricalConductanceMeasure
  rdf:type owl:Class ;
  rdfs:comment "Electrical conductance is the ease with which an electric current passes, and is the reciprocal quantity of electrical resistance."@en ;
  rdfs:label "Electrical conductance measure"@en ;
  rdfs:isDefinedBy <measure/v1.0.0/> ;
  rdfs:seeAlso <https://en.wikipedia.org/wiki/Electrical_resistance_and_conductance> ;
  rdfs:subClassOf
    ieso:TypeOfMeasure ,
    [
      rdf:type owl:Restriction ;
      owl:onProperty ieso:hasUnitOfMeasure ;
      owl:allValuesFrom ieso:ElectricalConductanceUnit
    ] ;
  .
# !


###  https://www.gecad.isep.ipp.pt/ieso/v1.0.0/ElectricalConductanceUnit
ieso:ElectricalConductanceUnit
  rdf:type owl:Class ;
  rdfs:comment "Electrical conductance is measured in siemens (S) (formerly called mhos and then represented by )."@en ;
  rdfs:label "Electrical conductance unit"@en ;
  rdfs:isDefinedBy <measure/v1.0.0/> ;
  rdfs:seeAlso <https://en.wikipedia.org/wiki/Electrical_resistance_and_conductance> ;
  rdfs:subClassOf
    ieso:DimensionalUnit ,
    [
      rdf:type owl:Restriction ;
      owl:onProperty ieso:isUnitOfMeasureOf ;
      owl:someValuesFrom ieso:ElectricalConductanceMeasure
    ] ,
    [
      rdf:type owl:Restriction ;
      owl:onProperty ieso:hasSIUnitOfMeasure ;
      owl:qualifiedCardinality "1"^^xsd:nonNegativeInteger ;
      owl:onClass ieso:ElectricalConductanceUnit
    ] ;
  .
# !


###  https://www.gecad.isep.ipp.pt/ieso/v1.0.0/ElectricalImpedanceMeasure
ieso:ElectricalImpedanceMeasure
  rdf:type owl:Class ;
  rdfs:comment "In electrical engineering, electrical impedance is the measure of the opposition that a circuit presents to a current when a voltage is applied. It extends the concept of resistance to alternating current (AC) circuits, and possesses both magnitude and phase, unlike resistance, which has only magnitude."@en ;
  rdfs:label "Electrical impedance measure"@en ;
  rdfs:isDefinedBy <measure/v1.0.0/> ;
  rdfs:seeAlso <https://en.wikipedia.org/wiki/Electrical_impedance> ;
  rdfs:subClassOf
    ieso:TypeOfMeasure ,
    [
      rdf:type owl:Restriction ;
      owl:onProperty ieso:hasUnitOfMeasure ;
      owl:allValuesFrom ieso:ElectricalImpedanceUnit
    ] ;
  .
# !


###  https://www.gecad.isep.ipp.pt/ieso/v1.0.0/ElectricalImpedanceUnit
ieso:ElectricalImpedanceUnit
  rdf:type owl:Class ;
  rdfs:comment "Impedance is a complex number, with the same units as resistance, for which the SI unit is the ohm ()."@en ;
  rdfs:label "Electrical impedance unit"@en ;
  rdfs:isDefinedBy <measure/v1.0.0/> ;
  rdfs:seeAlso <https://en.wikipedia.org/wiki/Electrical_impedance> ;
  rdfs:subClassOf
    ieso:DimensionalUnit ,
    [
      rdf:type owl:Restriction ;
      owl:onProperty ieso:isUnitOfMeasureOf ;
      owl:someValuesFrom ieso:ElectricalImpedanceMeasure
    ] ,
    [
      rdf:type owl:Restriction ;
      owl:onProperty ieso:hasSIUnitOfMeasure ;
      owl:qualifiedCardinality "1"^^xsd:nonNegativeInteger ;
      owl:onClass ieso:ElectricalImpedanceUnit
    ] ;
  .
# !


###  https://www.gecad.isep.ipp.pt/ieso/v1.0.0/ElectricalReactanceMeasure
ieso:ElectricalReactanceMeasure
  rdf:type owl:Class ;
  rdfs:comment "In electric and electronic systems, reactance is the opposition of a circuit element to the flow of current due to that element's inductance or capacitance. Greater reactance leads to smaller currents for the same voltage applied. Reactance is similar to electric resistance in this respect, but differs in that reactance does not lead to dissipation of electrical energy as heat. Instead, energy is stored in the reactance, and later returned to the circuit whereas a resistance continuously loses energy."@en ;
  rdfs:label "Electrical reactance measure"@en ;
  rdfs:isDefinedBy <measure/v1.0.0/> ;
  rdfs:seeAlso <https://en.wikipedia.org/wiki/Electrical_reactance> ;
  rdfs:subClassOf
    ieso:TypeOfMeasure ,
    [
      rdf:type owl:Restriction ;
      owl:onProperty ieso:hasUnitOfMeasure ;
      owl:allValuesFrom ieso:ElectricalReactanceUnit
    ] ;
  .
# !


###  https://www.gecad.isep.ipp.pt/ieso/v1.0.0/ElectricalReactanceUnit
ieso:ElectricalReactanceUnit
  rdf:type owl:Class ;
  rdfs:comment "Reactance is a complex number, with the same units as resistance, for which the SI unit is the ohm ()."@en ;
  rdfs:label "Electrical reactance unit"@en ;
  rdfs:isDefinedBy <measure/v1.0.0/> ;
  rdfs:seeAlso <https://en.wikipedia.org/wiki/Electrical_reactance> ;
  rdfs:subClassOf
    ieso:DimensionalUnit ,
    [
      rdf:type owl:Restriction ;
      owl:onProperty ieso:isUnitOfMeasureOf ;
      owl:someValuesFrom ieso:ElectricalReactanceMeasure
    ] ,
    [
      rdf:type owl:Restriction ;
      owl:onProperty ieso:hasSIUnitOfMeasure ;
      owl:qualifiedCardinality "1"^^xsd:nonNegativeInteger ;
      owl:onClass ieso:ElectricalReactanceUnit
    ] ;
  .
# !


###  https://www.gecad.isep.ipp.pt/ieso/v1.0.0/ElectricalResistanceMeasure
ieso:ElectricalResistanceMeasure
  rdf:type owl:Class ;
  rdfs:comment "In electronics and electromagnetism, the electrical resistance of an object is a measure of its opposition to the flow of electric current. The reciprocal quantity is electrical conductance, and is the ease with which an electric current passes. Electrical resistance shares some conceptual parallels with the notion of mechanical friction."@en ;
  rdfs:label "Electrical resistance measure"@en ;
  rdfs:isDefinedBy <measure/v1.0.0/> ;
  rdfs:seeAlso <https://en.wikipedia.org/wiki/Electrical_resistance_and_conductance> ;
  rdfs:subClassOf
    ieso:TypeOfMeasure ,
    [
      rdf:type owl:Restriction ;
      owl:onProperty ieso:hasUnitOfMeasure ;
      owl:allValuesFrom ieso:ElectricalResistanceUnit
    ] ;
  .
# !


###  https://www.gecad.isep.ipp.pt/ieso/v1.0.0/ElectricalResistanceUnit
ieso:ElectricalResistanceUnit
  rdf:type owl:Class ;
  rdfs:comment "The SI unit of electrical resistance is the ohm ()."@en ;
  rdfs:label "Electrical resistance unit"@en ;
  rdfs:isDefinedBy <measure/v1.0.0/> ;
  rdfs:seeAlso <https://en.wikipedia.org/wiki/Electrical_resistance_and_conductance> ;
  rdfs:subClassOf
    ieso:DimensionalUnit ,
    [
      rdf:type owl:Restriction ;
      owl:onProperty ieso:isUnitOfMeasureOf ;
      owl:someValuesFrom ieso:ElectricalResistanceMeasure
    ] ,
    [
      rdf:type owl:Restriction ;
      owl:onProperty ieso:hasSIUnitOfMeasure ;
      owl:qualifiedCardinality "1"^^xsd:nonNegativeInteger ;
      owl:onClass ieso:ElectricalResistanceUnit
    ] ;
  .
# !


###  https://www.gecad.isep.ipp.pt/ieso/v1.0.0/ElectricalSusceptanceMeasure
ieso:ElectricalSusceptanceMeasure
  rdf:type owl:Class ;
  rdfs:comment "In electrical engineering, susceptance (B) is the imaginary part of admittance, where the real part is conductance. The reciprocal of admittance is impedance, where the imaginary part is reactance and the real part is resistance."@en ;
  rdfs:label "Electrical susceptance measure"@en ;
  rdfs:isDefinedBy <measure/v1.0.0/> ;
  rdfs:seeAlso <https://en.wikipedia.org/wiki/Susceptance> ;
  rdfs:subClassOf
    ieso:TypeOfMeasure ,
    [
      rdf:type owl:Restriction ;
      owl:onProperty ieso:hasUnitOfMeasure ;
      owl:allValuesFrom ieso:ElectricalSusceptanceUnit
    ] ;
  .
# !


###  https://www.gecad.isep.ipp.pt/ieso/v1.0.0/ElectricalSusceptanceUnit
ieso:ElectricalSusceptanceUnit
  rdf:type owl:Class ;
  rdfs:comment "In SI units, susceptance is measured in siemens."@en ;
  rdfs:label "Electrical susceptance unit"@en ;
  rdfs:isDefinedBy <measure/v1.0.0/> ;
  rdfs:seeAlso <https://en.wikipedia.org/wiki/Susceptance> ;
  rdfs:subClassOf
    ieso:DimensionalUnit ,
    [
      rdf:type owl:Restriction ;
      owl:onProperty ieso:isUnitOfMeasureOf ;
      owl:someValuesFrom ieso:ElectricalSusceptanceMeasure
    ] ,
    [
      rdf:type owl:Restriction ;
      owl:onProperty ieso:hasSIUnitOfMeasure ;
      owl:qualifiedCardinality "1"^^xsd:nonNegativeInteger ;
      owl:onClass ieso:ElectricalSusceptanceUnit
    ] ;
  .
# !


###  https://www.gecad.isep.ipp.pt/ieso/v1.0.0/ElectricChargeMeasure
ieso:ElectricChargeMeasure
  rdf:type owl:Class ;
  rdfs:comment "Electric charge is the physical property of matter that causes it to experience a force when placed in an electromagnetic field. There are two types of electric charge: positive and negative (commonly carried by protons and electrons respectively). Like charges repel each other and unlike charges attract each other. An object with an absence of net charge is referred to as neutral. Early knowledge of how charged substances interact is now called classical electrodynamics, and is still accurate for problems that do not require consideration of quantum effects."@en ;
  rdfs:label "Electric charge measure"@en ;
  rdfs:isDefinedBy <measure/v1.0.0/> ;
  rdfs:seeAlso <https://en.wikipedia.org/wiki/Electric_charge> ;
  rdfs:subClassOf
    ieso:TypeOfMeasure ,
    [
      rdf:type owl:Restriction ;
      owl:onProperty ieso:hasUnitOfMeasure ;
      owl:allValuesFrom ieso:ElectricChargeUnit
    ] ;
  .
# !


###  https://www.gecad.isep.ipp.pt/ieso/v1.0.0/ElectricChargeUnit
ieso:ElectricChargeUnit
  rdf:type owl:Class ;
  rdfs:comment "The SI derived unit of quantity of electric charge is the coulomb (symbol: C). The coulomb is defined as the quantity of charge that passes through the cross section of an electrical conductor carrying one ampere for one second."@en ;
  rdfs:label "Electric charge unit"@en ;
  rdfs:isDefinedBy <measure/v1.0.0/> ;
  rdfs:seeAlso <https://en.wikipedia.org/wiki/Electric_charge#Units> ;
  rdfs:subClassOf
    ieso:DimensionalUnit ,
    [
      rdf:type owl:Restriction ;
      owl:onProperty ieso:isUnitOfMeasureOf ;
      owl:someValuesFrom ieso:ElectricChargeMeasure
    ] ,
    [
      rdf:type owl:Restriction ;
      owl:onProperty ieso:hasSIUnitOfMeasure ;
      owl:qualifiedCardinality "1"^^xsd:nonNegativeInteger ;
      owl:onClass ieso:ElectricChargeUnit
    ] ;
  .
# !


###  https://www.gecad.isep.ipp.pt/ieso/v1.0.0/ElectricCurrentMeasure
ieso:ElectricCurrentMeasure
  rdf:type owl:Class ;
  rdfs:comment "An electric current is a stream of charged particles, such as electrons or ions, moving through an electrical conductor or space. It is measured as the net rate of flow of electric charge through a surface or into a control volume."@en ;
  rdfs:label "Electric current measure"@en ;
  rdfs:isDefinedBy <measure/v1.0.0/> ;
  rdfs:seeAlso <https://en.wikipedia.org/wiki/Electric_current> ;
  rdfs:subClassOf
    ieso:TypeOfMeasure ,
    [
      rdf:type owl:Restriction ;
      owl:onProperty ieso:hasUnitOfMeasure ;
      owl:allValuesFrom ieso:ElectricCurrentUnit
    ] ;
  .
# !


###  https://www.gecad.isep.ipp.pt/ieso/v1.0.0/ElectricCurrentUnit
ieso:ElectricCurrentUnit
  rdf:type owl:Class ;
  rdfs:comment "The SI unit of electric current is the ampere, or amp, which is the flow of electric charge across a surface at the rate of one coulomb per second. The ampere (symbol: A) is an SI base unit Electric current is measured using a device called an ammeter."@en ;
  rdfs:label "Electric current unit"@en ;
  rdfs:isDefinedBy <measure/v1.0.0/> ;
  rdfs:seeAlso "https://en.wikipedia.org/wiki/Electric_current"@en ;
  rdfs:subClassOf
    ieso:DimensionalUnit ,
    [
      rdf:type owl:Restriction ;
      owl:onProperty ieso:isUnitOfMeasureOf ;
      owl:someValuesFrom ieso:ElectricCurrentMeasure
    ] ,
    [
      rdf:type owl:Restriction ;
      owl:onProperty ieso:hasSIUnitOfMeasure ;
      owl:qualifiedCardinality "1"^^xsd:nonNegativeInteger ;
      owl:onClass ieso:ElectricCurrentUnit
    ] ;
  .
# !


###  https://www.gecad.isep.ipp.pt/ieso/v1.0.0/ElectricEnergyMeasure
ieso:ElectricEnergyMeasure
  rdf:type owl:Class ;
  rdfs:comment "Electrical energy is energy derived from electric potential energy or kinetic energy. When used loosely, electrical energy refers to energy that has been converted from electric potential energy. This energy is supplied by the combination of electric current and electric potential that is delivered by an electrical circuit (e.g., provided by an electric power utility)."@en ;
  rdfs:label "Electric energy measure"@en ;
  rdfs:isDefinedBy <measure/v1.0.0/> ;
  rdfs:seeAlso <https://en.wikipedia.org/wiki/Electrical_energy> ;
  rdfs:subClassOf
    ieso:EnergyMeasure ,
    [
      rdf:type owl:Restriction ;
      owl:onProperty ieso:hasUnitOfMeasure ;
      owl:allValuesFrom ieso:ElectricEnergyUnit
    ] ;
  .
# !


###  https://www.gecad.isep.ipp.pt/ieso/v1.0.0/ElectricEnergyUnit
ieso:ElectricEnergyUnit
  rdf:type owl:Class ;
  rdfs:comment "The SI unit of energy rate (energy per unit time) is the watt, which is a joule per second. Thus, one joule is one watt-second, and 3600 joules equal one watt-hour."@en ;
  rdfs:label "Electric energy unit"@en ;
  rdfs:isDefinedBy <measure/v1.0.0/> ;
  rdfs:seeAlso <https://en.wikipedia.org/wiki/Energy#Units_of_measure> ;
  rdfs:subClassOf
    ieso:EnergyUnit ,
    [
      rdf:type owl:Restriction ;
      owl:onProperty ieso:isUnitOfMeasureOf ;
      owl:someValuesFrom ieso:ElectricEnergyMeasure
    ] ;
  .
# !


###  https://www.gecad.isep.ipp.pt/ieso/v1.0.0/ElectricPowerMeasure
ieso:ElectricPowerMeasure
  rdf:type owl:Class ;
  rdfs:comment "Electric power is the rate, per unit time, at which electrical energy is transferred by an electric circuit. The SI unit of power is the watt, one joule per second."@en ;
  rdfs:label "Electric power measure"@en ;
  rdfs:isDefinedBy <measure/v1.0.0/> ;
  rdfs:seeAlso <https://en.wikipedia.org/wiki/Electric_power> ;
  rdfs:subClassOf
    ieso:PowerMeasure ,
    [
      rdf:type owl:Restriction ;
      owl:onProperty ieso:hasUnitOfMeasure ;
      owl:allValuesFrom ieso:ElectricPowerUnit
    ] ;
  .
# !


###  https://www.gecad.isep.ipp.pt/ieso/v1.0.0/ElectricPowerUnit
ieso:ElectricPowerUnit
  rdf:type owl:Class ;
  rdfs:comment "Electric power is the rate, per unit time, at which electrical energy is transferred by an electric circuit. The SI unit of power is the watt, one joule per second."@en ;
  rdfs:label "Electric power unit"@en ;
  rdfs:isDefinedBy <measure/v1.0.0/> ;
  rdfs:seeAlso <https://en.wikipedia.org/wiki/Electric_power> ;
  rdfs:subClassOf
    ieso:PowerUnit ,
    [
      rdf:type owl:Restriction ;
      owl:onProperty ieso:isUnitOfMeasureOf ;
      owl:someValuesFrom ieso:ElectricPowerMeasure
    ] ;
  .
# !


###  https://www.gecad.isep.ipp.pt/ieso/v1.0.0/EnergyMeasure
ieso:EnergyMeasure
  rdf:type owl:Class ;
  rdfs:comment "In physics, energy is the quantitative property that must be transferred to an object in order to perform work on, or to heat, the object. Energy is a conserved quantity; the law of conservation of energy states that energy can be converted in form, but not created or destroyed."@en ;
  rdfs:label "Energy measure"@en ;
  rdfs:isDefinedBy <measure/v1.0.0/> ;
  rdfs:seeAlso <https://en.wikipedia.org/wiki/Energy> ;
  rdfs:subClassOf
    ieso:TypeOfMeasure ,
    [
      rdf:type owl:Restriction ;
      owl:onProperty ieso:hasUnitOfMeasure ;
      owl:allValuesFrom ieso:EnergyUnit
    ] ;
  .
# !


###  https://www.gecad.isep.ipp.pt/ieso/v1.0.0/EnergyUnit
ieso:EnergyUnit
  rdf:type owl:Class ;
  rdfs:comment """In the International System of Units (SI), the unit of energy is the joule, named after Joule. It is a derived unit. It is equal to the energy expended (or work done) in applying a force of one newton through a distance of one metre. However energy is also expressed in many other units not part of the SI, such as ergs, calories, British Thermal Units, kilowatt-hours and kilocalories, which require a conversion factor when expressed in SI units.\n\nThe SI unit of energy rate (energy per unit time) is the watt, which is a joule per second. Thus, one joule is one watt-second, and 3600 joules equal one watt-hour. The CGS energy unit is the erg and the imperial and US customary unit is the foot pound. Other energy units such as the electronvolt, food calorie or thermodynamic kcal (based on the temperature change of water in a heating process), and BTU are used in specific areas of science and commerce."""@en ;
  rdfs:label "Energy unit"@en ;
  rdfs:isDefinedBy <measure/v1.0.0/> ;
  rdfs:seeAlso <https://en.wikipedia.org/wiki/Energy#Units_of_measure> ;
  rdfs:subClassOf
    ieso:DimensionalUnit ,
    [
      rdf:type owl:Restriction ;
      owl:onProperty ieso:isUnitOfMeasureOf ;
      owl:someValuesFrom ieso:EnergyMeasure
    ] ,
    [
      rdf:type owl:Restriction ;
      owl:onProperty ieso:hasSIUnitOfMeasure ;
      owl:qualifiedCardinality "1"^^xsd:nonNegativeInteger ;
      owl:onClass ieso:EnergyUnit
    ] ;
  .
# !


###  https://www.gecad.isep.ipp.pt/ieso/v1.0.0/FrequencyMeasure
ieso:FrequencyMeasure
  rdf:type owl:Class ;
  rdfs:comment "Frequency is the number of occurrences of a repeating event per unit of time. It is also referred to as temporal frequency, which emphasizes the contrast to spatial frequency and angular frequency. Frequency is measured in hertz (Hz) which is equal to one event per second. The period is the duration of time of one cycle in a repeating event, so the period is the reciprocal of the frequency."@en ;
  rdfs:label "Frequency measure"@en ;
  rdfs:isDefinedBy <measure/v1.0.0/> ;
  rdfs:seeAlso <https://en.wikipedia.org/wiki/Frequency> ;
  rdfs:subClassOf
    ieso:TypeOfMeasure ,
    [
      rdf:type owl:Restriction ;
      owl:onProperty ieso:hasUnitOfMeasure ;
      owl:allValuesFrom ieso:FrequencyUnit
    ] ;
  .
# !


###  https://www.gecad.isep.ipp.pt/ieso/v1.0.0/FrequencyUnit
ieso:FrequencyUnit
  rdf:type owl:Class ;
  rdfs:comment """The term temporal frequency is used to emphasise that the frequency is characterised by the number of occurrences of a repeating event per unit time, and not unit distance.\n\nThe SI derived unit of frequency is the hertz (Hz), named after the German physicist Heinrich Hertz by the International Electrotechnical Commission in 1930. The SI unit for the period, as for all measurements of time, is the second. A traditional unit of measure used with rotating mechanical devices is revolutions per minute, abbreviated r/min or rpm. 60 rpm is equivalent to one hertz."""@en ;
  rdfs:label "Frequency unit"@en ;
  rdfs:isDefinedBy <measure/v1.0.0/> ;
  rdfs:seeAlso <https://en.wikipedia.org/wiki/Frequency#Definitions_and_units> ;
  rdfs:subClassOf
    ieso:DimensionalUnit ,
    [
      rdf:type owl:Restriction ;
      owl:onProperty ieso:isUnitOfMeasureOf ;
      owl:someValuesFrom ieso:FrequencyMeasure
    ] ,
    [
      rdf:type owl:Restriction ;
      owl:onProperty ieso:hasSIUnitOfMeasure ;
      owl:qualifiedCardinality "1"^^xsd:nonNegativeInteger ;
      owl:onClass ieso:FrequencyUnit
    ] ;
  .
# !


###  https://www.gecad.isep.ipp.pt/ieso/v1.0.0/RelativeHumidityMeasure
ieso:RelativeHumidityMeasure
  rdf:type owl:Class ;
  rdfs:comment "Relative humidity, often expressed as a percentage, indicates a present state of absolute humidity relative to a maximum humidity given the same temperature."@en ;
  rdfs:label "Relative humidity measure"@en ;
  rdfs:isDefinedBy <measure/v1.0.0/> ;
  rdfs:seeAlso <https://en.wikipedia.org/wiki/Humidity> ;
  rdfs:subClassOf
    ieso:TypeOfMeasure ,
    [
      rdf:type owl:Restriction ;
      owl:onProperty ieso:hasUnitOfMeasure ;
      owl:allValuesFrom ieso:PercentageUnit
    ]
  .
# !


###  https://www.gecad.isep.ipp.pt/ieso/v1.0.0/IlluminanceMeasure
ieso:IlluminanceMeasure
  rdf:type owl:Class ;
  rdfs:comment "In photometry, illuminance is the total luminous flux incident on a surface, per unit area. It is a measure of how much the incident light illuminates the surface, wavelength-weighted by the luminosity function to correlate with human brightness perception."@en ;
  rdfs:label "Illuminance measure"@en ;
  rdfs:isDefinedBy <measure/v1.0.0/> ;
  rdfs:seeAlso <https://en.wikipedia.org/wiki/Illuminance> ;
  rdfs:subClassOf
    ieso:LightMeasure ,
    [
      rdf:type owl:Restriction ;
      owl:onProperty ieso:hasUnitOfMeasure ;
      owl:allValuesFrom ieso:IlluminanceUnit
    ] ;
  .
# !


###  https://www.gecad.isep.ipp.pt/ieso/v1.0.0/IlluminanceUnit
ieso:IlluminanceUnit
  rdf:type owl:Class ;
  rdfs:comment "In SI derived units these are measured in lux (lx), or equivalently in lumens per square metre (lmm2)."@en ;
  rdfs:label "Illuminance unit"@en ;
  rdfs:isDefinedBy <measure/v1.0.0/> ;
  rdfs:seeAlso
    <https://en.wikipedia.org/wiki/Light#Units_and_measures> ,
    <https://en.wikipedia.org/wiki/Illuminance> ;
  rdfs:subClassOf
    ieso:LightUnit ,
    [
      rdf:type owl:Restriction ;
      owl:onProperty ieso:isUnitOfMeasureOf ;
      owl:someValuesFrom ieso:IlluminanceMeasure
    ] ,
    [
      rdf:type owl:Restriction ;
      owl:onProperty ieso:hasSIUnitOfMeasure ;
      owl:qualifiedCardinality "1"^^xsd:nonNegativeInteger ;
      owl:onClass ieso:IlluminanceUnit
    ] ;
  .
# !


###  https://www.gecad.isep.ipp.pt/ieso/v1.0.0/IrradianceMeasure
ieso:IrradianceMeasure
  rdf:type owl:Class ;
  rdfs:comment "In radiometry, irradiance is the radiant flux (power) received by a surface per unit area. "@en ;
  rdfs:label "Irradiance measure"@en ;
  rdfs:isDefinedBy <measure/v1.0.0/> ;
  rdfs:seeAlso <https://en.wikipedia.org/wiki/Irradiance> ;
  rdfs:subClassOf
    ieso:LightMeasure ,
    [
      rdf:type owl:Restriction ;
      owl:onProperty ieso:hasUnitOfMeasure ;
      owl:allValuesFrom ieso:IrradianceUnit
    ] ;
  .
# !


###  https://www.gecad.isep.ipp.pt/ieso/v1.0.0/IrradianceUnit
ieso:IrradianceUnit
  rdf:type owl:Class ;
  rdfs:comment "The SI unit of irradiance is the watt per square metre (Wm^2)."@en ;
  rdfs:label "Irradiance unit"@en ;
  rdfs:isDefinedBy <measure/v1.0.0/> ;
  rdfs:seeAlso
    <https://en.wikipedia.org/wiki/Light#Units_and_measures> ,
    <https://en.wikipedia.org/wiki/Irradiance#SI_radiometry_units> ;
  rdfs:subClassOf
    ieso:LightUnit ,
    [
      rdf:type owl:Restriction ;
      owl:onProperty ieso:isUnitOfMeasureOf ;
      owl:someValuesFrom ieso:IrradianceMeasure
    ] ,
    [
      rdf:type owl:Restriction ;
      owl:onProperty ieso:hasSIUnitOfMeasure ;
      owl:qualifiedCardinality "1"^^xsd:nonNegativeInteger ;
      owl:onClass ieso:IrradianceUnit
    ] ;
  .
# !


###  https://www.gecad.isep.ipp.pt/ieso/v1.0.0/LengthMeasure
ieso:LengthMeasure
  rdf:type owl:Class ;
  rdfs:comment "Length is a measure of distance. In the International System of Quantities, length is a quantity with dimension distance. In most systems of measurement a base unit for length is chosen, from which all other units are derived. In the International System of Units (SI) system the base unit for length is the metre."@en ;
  rdfs:label "Length measure"@en ;
  rdfs:isDefinedBy <measure/v1.0.0/> ;
  rdfs:seeAlso <https://en.wikipedia.org/wiki/Length> ;
  rdfs:subClassOf
    ieso:TypeOfMeasure ,
    [
      rdf:type owl:Restriction ;
      owl:onProperty ieso:hasUnitOfMeasure ;
      owl:allValuesFrom ieso:LengthUnit
    ] ;
  .
# !


###  https://www.gecad.isep.ipp.pt/ieso/v1.0.0/LengthUnit
ieso:LengthUnit
  rdf:type owl:Class ;
  rdfs:comment "A unit of length refers to any arbitrarily chosen and accepted reference standard for measurement of length. The most common units in modern use are the metric units, used in every country globally."@en ;
  rdfs:label "Length unit"@en ;
  rdfs:isDefinedBy <measure/v1.0.0/> ;
  rdfs:seeAlso <https://en.wikipedia.org/wiki/Unit_of_length> ;
  rdfs:subClassOf
    ieso:DimensionalUnit ,
    [
      rdf:type owl:Restriction ;
      owl:onProperty ieso:isUnitOfMeasureOf ;
      owl:someValuesFrom ieso:LengthMeasure
    ] ,
    [
      rdf:type owl:Restriction ;
      owl:onProperty ieso:hasSIUnitOfMeasure ;
      owl:qualifiedCardinality "1"^^xsd:nonNegativeInteger ;
      owl:onClass ieso:LengthUnit
    ] ;
  .
# !


###  https://www.gecad.isep.ipp.pt/ieso/v1.0.0/LinearDensityMeasure
ieso:LinearDensityMeasure
  rdf:type owl:Class ;
  rdfs:comment "Linear density is the measure of a quantity of any characteristic value per unit of length. Linear mass density (titer in textile engineering, the amount of mass per unit length) and linear charge density (the amount of electric charge per unit length) are two common examples used in science and engineering."@en ;
  rdfs:label "Linear density measure"@en ;
  rdfs:isDefinedBy <measure/v1.0.0/> ;
  rdfs:seeAlso <https://en.wikipedia.org/wiki/Linear_density> ;
  rdfs:subClassOf
    ieso:DensityMeasure ,
    [
      rdf:type owl:Restriction ;
      owl:onProperty ieso:hasUnitOfMeasure ;
      owl:allValuesFrom ieso:LinearDensityUnit
    ] ;
  .
# !


###  https://www.gecad.isep.ipp.pt/ieso/v1.0.0/LinearDensityUnit
ieso:LinearDensityUnit
  rdf:type owl:Class ;
  rdfs:comment "The linear density indicates the amount of a quantity per unit length along a single dimension."@en ;
  rdfs:label "Linear density unit"@en ;
  rdfs:isDefinedBy <measure/v1.0.0/> ;
  rdfs:seeAlso <https://en.wikipedia.org/wiki/Linear_density#Units> ;
  rdfs:subClassOf
    ieso:DensityUnit ,
    [
      rdf:type owl:Restriction ;
      owl:onProperty ieso:isUnitOfMeasureOf ;
      owl:someValuesFrom ieso:LinearDensityMeasure
    ] ,
    [
      rdf:type owl:Restriction ;
      owl:onProperty ieso:hasSIUnitOfMeasure ;
      owl:qualifiedCardinality "1"^^xsd:nonNegativeInteger ;
      owl:onClass ieso:LinearDensityUnit
    ] ;
  .
# !


###  https://www.gecad.isep.ipp.pt/ieso/v1.0.0/LightMeasure
ieso:LightMeasure
  rdf:type owl:Class ;
  rdfs:comment "Light or visible light is electromagnetic radiation within the portion of the electromagnetic spectrum that can be perceived by the human eye. Visible light is usually defined as having wavelengths in the range of 400700 nm, between the infrared (with longer wavelengths) and the ultraviolet (with shorter wavelengths). This wavelength means a frequency range of roughly 430750 terahertz (THz)."@en ;
  rdfs:label "Light measure"@en ;
  rdfs:isDefinedBy <measure/v1.0.0/> ;
  rdfs:seeAlso <https://en.wikipedia.org/wiki/Light> ;
  rdfs:subClassOf
    ieso:TypeOfMeasure ,
    [
      rdf:type owl:Restriction ;
      owl:onProperty ieso:hasUnitOfMeasure ;
      owl:allValuesFrom ieso:LightUnit
    ] ;
  .
# !


###  https://www.gecad.isep.ipp.pt/ieso/v1.0.0/LightUnit
ieso:LightUnit
  rdf:type owl:Class ;
  rdfs:comment "Light is measured with two main alternative sets of units: radiometry consists of measurements of light power at all wavelengths, while photometry measures light with wavelength weighted with respect to a standardized model of human brightness perception. Photometry is useful, for example, to quantify Illumination (lighting) intended for human use."@en ;
  rdfs:label "Light unit"@en ;
  rdfs:isDefinedBy <measure/v1.0.0/> ;
  rdfs:seeAlso <https://en.wikipedia.org/wiki/Light#Units_and_measures> ;
  rdfs:subClassOf
    ieso:DimensionalUnit ,
    [
      rdf:type owl:Restriction ;
      owl:onProperty ieso:isUnitOfMeasureOf ;
      owl:someValuesFrom ieso:LightMeasure
    ] ,
    [
      rdf:type owl:Restriction ;
      owl:onProperty ieso:hasSIUnitOfMeasure ;
      owl:qualifiedCardinality "1"^^xsd:nonNegativeInteger ;
      owl:onClass ieso:LightUnit
    ] ;
  .
# !


###  https://www.gecad.isep.ipp.pt/ieso/v1.0.0/LuminanceMeasure
ieso:LuminanceMeasure
  rdf:type owl:Class ;
  rdfs:comment "Luminance is a photometric measure of the luminous intensity per unit area of light travelling in a given direction. It describes the amount of light that passes through, is emitted from, or is reflected from a particular area, and falls within a given solid angle."@en ;
  rdfs:label "Luminance measure"@en ;
  rdfs:isDefinedBy <measure/v1.0.0/> ;
  rdfs:seeAlso <https://en.wikipedia.org/wiki/Luminance> ;
  rdfs:subClassOf
    ieso:LightMeasure ,
    [
      rdf:type owl:Restriction ;
      owl:onProperty ieso:hasUnitOfMeasure ;
      owl:allValuesFrom ieso:LuminanceUnit
    ] ;
  .
# !


###  https://www.gecad.isep.ipp.pt/ieso/v1.0.0/LuminanceUnit
ieso:LuminanceUnit
  rdf:type owl:Class ;
  rdfs:comment "The SI unit for luminance is candela per square metre (cd/m2), as defined by the International System of Units standard for the modern metric system."@en ;
  rdfs:label "Luminance unit"@en ;
  rdfs:isDefinedBy <measure/v1.0.0/> ;
  rdfs:seeAlso
    <https://en.wikipedia.org/wiki/Light#Units_and_measures> ,
    <https://en.wikipedia.org/wiki/Luminance#Units> ;
  rdfs:subClassOf
    ieso:LightUnit ,
    [
      rdf:type owl:Restriction ;
      owl:onProperty ieso:isUnitOfMeasureOf ;
      owl:someValuesFrom ieso:LuminanceMeasure
    ] ,
    [
      rdf:type owl:Restriction ;
      owl:onProperty ieso:hasSIUnitOfMeasure ;
      owl:qualifiedCardinality "1"^^xsd:nonNegativeInteger ;
      owl:onClass ieso:LuminanceUnit
    ] ;
  .
# !


###  https://www.gecad.isep.ipp.pt/ieso/v1.0.0/LuminousFluxMeasure
ieso:LuminousFluxMeasure
  rdf:type owl:Class ;
  rdfs:comment "In photometry, luminous flux or luminous power is the measure of the perceived power of light. It differs from radiant flux, the measure of the total power of electromagnetic radiation (including infrared, ultraviolet, and visible light), in that luminous flux is adjusted to reflect the varying sensitivity of the human eye to different wavelengths of light."@en ;
  rdfs:label "Luminous flux measure"@en ;
  rdfs:isDefinedBy <measure/v1.0.0/> ;
  rdfs:seeAlso <https://en.wikipedia.org/wiki/Luminous_flux> ;
  rdfs:subClassOf
    ieso:LightMeasure ,
    [
      rdf:type owl:Restriction ;
      owl:onProperty ieso:hasUnitOfMeasure ;
      owl:allValuesFrom ieso:LuminousFluxUnit
    ] ;
  .
# !


###  https://www.gecad.isep.ipp.pt/ieso/v1.0.0/LuminousFluxUnit
ieso:LuminousFluxUnit
  rdf:type owl:Class ;
  rdfs:comment "The SI unit of luminous flux is the lumen (lm). Until 19 May 2019, one lumen was defined as the luminous flux of light produced by a light source that emits one candela of luminous intensity over a solid angle of one steradian. Since 20 May 2019, the lumen has been defined by fixing the luminous efficacy of monochromatic radiation of frequency 540  1012 Hz (green light) to be 683 lm W1. In other systems of units, luminous flux may have units of power."@en ;
  rdfs:label "Luminous flux unit"@en ;
  rdfs:isDefinedBy <measure/v1.0.0/> ;
  rdfs:seeAlso
    <https://en.wikipedia.org/wiki/Light#Units_and_measures> ,
    <https://en.wikipedia.org/wiki/Luminous_flux#Units> ;
  rdfs:subClassOf
    ieso:LightUnit ,
    [
      rdf:type owl:Restriction ;
      owl:onProperty ieso:isUnitOfMeasureOf ;
      owl:someValuesFrom ieso:LuminousFluxMeasure
    ] ,
    [
      rdf:type owl:Restriction ;
      owl:onProperty ieso:hasSIUnitOfMeasure ;
      owl:qualifiedCardinality "1"^^xsd:nonNegativeInteger ;
      owl:onClass ieso:LuminousFluxUnit
    ] ;
  .
# !


###  https://www.gecad.isep.ipp.pt/ieso/v1.0.0/LuminousIntensityMeasure
ieso:LuminousIntensityMeasure
  rdf:type owl:Class ;
  rdfs:comment "In photometry, luminous intensity is a measure of the wavelength-weighted power emitted by a light source in a particular direction per unit solid angle, based on the luminosity function, a standardized model of the sensitivity of the human eye."@en ;
  rdfs:label "Luminous intensity measure"@en ;
  rdfs:isDefinedBy <measure/v1.0.0/> ;
  rdfs:seeAlso <https://en.wikipedia.org/wiki/Luminous_intensity> ;
  rdfs:subClassOf
    ieso:LightMeasure ,
    [
      rdf:type owl:Restriction ;
      owl:onProperty ieso:hasUnitOfMeasure ;
      owl:allValuesFrom ieso:LuminousIntensityUnit
    ] ;
  .
# !


###  https://www.gecad.isep.ipp.pt/ieso/v1.0.0/ Unit
ieso:LuminousIntensityUnit
  rdf:type owl:Class ;
  rdfs:comment "The SI unit of luminous intensity is the candela (cd), an SI base unit. It is defined by the description of a physical process that will produce one candela of luminous intensity. By definition, if one constructs a light source that emits monochromatic green light with a frequency of 540 THz, and that has a radiant intensity of 1/683 watts per steradian in a given direction, that light source will emit one candela in the specified direction."@en ;
  rdfs:label "Luminous intensity unit"@en ;
  rdfs:isDefinedBy <measure/v1.0.0/> ;
  rdfs:seeAlso
    <https://en.wikipedia.org/wiki/Light#Units_and_measures> ,
    <https://en.wikipedia.org/wiki/Luminous_intensity#Units> ;
  rdfs:subClassOf
    ieso:LightUnit ,
    [
      rdf:type owl:Restriction ;
      owl:onProperty ieso:isUnitOfMeasureOf ;
      owl:someValuesFrom ieso:LuminousIntensityMeasure
    ] ,
    [
      rdf:type owl:Restriction ;
      owl:onProperty ieso:hasSIUnitOfMeasure ;
      owl:qualifiedCardinality "1"^^xsd:nonNegativeInteger ;
      owl:onClass ieso:LuminousIntensityUnit
    ] ;
  .
# !


###  https://www.gecad.isep.ipp.pt/ieso/v1.0.0/MassDensityMeasure
ieso:MassDensityMeasure
  rdf:type owl:Class ;
  rdfs:comment "The mass density (more precisely, the volumetric mass density; also known as specific mass), of a substance is its mass per unit volume."@en ;
  rdfs:label "Mass density measure"@en ;
  rdfs:isDefinedBy <measure/v1.0.0/> ;
  rdfs:seeAlso <https://en.wikipedia.org/wiki/Density> ;
  rdfs:subClassOf
    ieso:DensityMeasure ,
    [
      rdf:type owl:Restriction ;
      owl:onProperty ieso:hasUnitOfMeasure ;
      owl:allValuesFrom ieso:MassDensityUnit
    ] ;
  .
# !


###  https://www.gecad.isep.ipp.pt/ieso/v1.0.0/MassDensityUnit
ieso:MassDensityUnit
  rdf:type owl:Class ;
  rdfs:comment "The SI unit for density is kilogram per cubic metre (kg/m^3). The litre and metric tons are not part of the SI, but are acceptable for use with it."@en ;
  rdfs:label "Mass density unit"@en ;
  rdfs:isDefinedBy <measure/v1.0.0/> ;
  rdfs:seeAlso <https://en.wikipedia.org/wiki/Density#Common_units> ;
  rdfs:subClassOf
    ieso:DensityUnit ,
    [
      rdf:type owl:Restriction ;
      owl:onProperty ieso:isUnitOfMeasureOf ;
      owl:someValuesFrom ieso:MassDensityMeasure
    ] ,
    [
      rdf:type owl:Restriction ;
      owl:onProperty ieso:hasSIUnitOfMeasure ;
      owl:qualifiedCardinality "1"^^xsd:nonNegativeInteger ;
      owl:onClass ieso:MassDensityUnit
    ] ;
  .
# !


###  https://www.gecad.isep.ipp.pt/ieso/v1.0.0/Measurement
ieso:Measurement
  rdf:type owl:Class ;
  rdfs:comment "Measurement is the numerical quantification of the attributes of an object or event, which can be used to compare with other objects or events. The scope and application of measure are dependent on the context and discipline."@en ;
  rdfs:label "Measurement"@en ;
  rdfs:isDefinedBy <measure/v1.0.0/> ;
  rdfs:seeAlso <https://en.wikipedia.org/wiki/Measure> ;
  rdfs:subClassOf
    [
      rdf:type owl:Restriction ;
      owl:onProperty ieso:hasMeasurementValue ;
      owl:allValuesFrom ieso:MeasurementValue
    ] ,
    [
      rdf:type owl:Restriction ;
      owl:onProperty ieso:hasTypeOfMeasure ;
      owl:allValuesFrom ieso:TypeOfMeasure
    ] ,
    [
      rdf:type owl:Restriction ;
      owl:onProperty ieso:hasUnitOfMeasure ;
      owl:allValuesFrom ieso:UnitOfMeasure
    ] ,
    [
      rdf:type owl:Restriction ;
      owl:onProperty ieso:hasDateTime ;
      owl:allValuesFrom xsd:dateTime
    ] ;
  .
# !


###  https://www.gecad.isep.ipp.pt/ieso/v1.0.0/Energy
ieso:Energy
  rdf:type owl:Class ;
  rdfs:comment "The 'Energy' class represents energy measure."@en ;
  rdfs:label "Energy"@en ;
  rdfs:isDefinedBy <measure/v1.0.0/> ;
  rdfs:subClassOf ieso:Measurement ;
  .
# !


###  https://www.gecad.isep.ipp.pt/ieso/v1.0.0/Power
ieso:Power
  rdf:type owl:Class ;
  rdfs:comment "The 'Power' class represents a power measure."@en ;
  rdfs:label "Power"@en ;
  rdfs:isDefinedBy <measure/v1.0.0/> ;
  rdfs:subClassOf ieso:Measurement ;
  .
# !


###  https://www.gecad.isep.ipp.pt/ieso/v1.0.0/Price
ieso:Price
  rdf:type owl:Class ;
  rdfs:comment "The 'Price' class represents a price measure."@en ;
  rdfs:label "Price"@en ;
  rdfs:isDefinedBy <measure/v1.0.0/> ;
  rdfs:subClassOf ieso:Measurement ;
  .
# !


###  https://www.gecad.isep.ipp.pt/ieso/v1.0.0/MeasurementValue
ieso:MeasurementValue
  rdf:type owl:Class ;
  rdfs:comment "This class describes a measurement value and the respective unit of measure."@en ;
  rdfs:label "Measurement value"@en ;
  rdfs:isDefinedBy <measure/v1.0.0/> ;
  rdfs:subClassOf
    [
      rdf:type owl:Restriction ;
      owl:onProperty ieso:isMeasurementValueOf ;
      owl:qualifiedCardinality "1"^^xsd:nonNegativeInteger ;
      owl:onClass ieso:Measurement
    ] ,
    [
      rdf:type owl:Restriction ;
      owl:onProperty ieso:hasUnitOfMeasure ;
      owl:maxQualifiedCardinality "1"^^xsd:nonNegativeInteger ;
      owl:onClass ieso:UnitOfMeasure
    ] ,
    [
      rdf:type owl:Restriction ;
      owl:onProperty ieso:hasLiteralValue ;
      owl:maxCardinality "1"^^xsd:nonNegativeInteger
    ] ;
  .
# !


###  https://www.gecad.isep.ipp.pt/ieso/v1.0.0/ObscurationMeasure
ieso:ObscurationMeasure
  rdf:type owl:Class ;
  rdfs:comment "Obscuration is the effect smoke has that reduces light intensity, expressed in percent absorption per unit length; higher concentrations of smoke result in higher obscuration levels."@en ;
  rdfs:label "Obscuration measure"@en ;
  rdfs:isDefinedBy <measure/v1.0.0/> ;
  rdfs:seeAlso
    <https://en.wiktionary.org/wiki/obscuration> ,
    <https://en.wikipedia.org/wiki/Smoke_detector> ;
  rdfs:subClassOf
    ieso:RatioMeasure ,
    [
      rdf:type owl:Restriction ;
      owl:onProperty ieso:hasUnitOfMeasure ;
      owl:allValuesFrom ieso:ObscurationUnit
    ] ;
  .
# !


###  https://www.gecad.isep.ipp.pt/ieso/v1.0.0/ObscurationUnit
ieso:ObscurationUnit
  rdf:type owl:Class ;
  rdfs:comment "Obscuration is a unit of measurement that has become the standard way of specifying smoke detector sensitivity which respond to absorption of light by smoke, in percent absorption per unit length, e.g. % obs/ft, % obs/m."@en ;
  rdfs:label "Obscuration unit"@en ;
  rdfs:isDefinedBy <measure/v1.0.0/> ;
  rdfs:seeAlso
    <https://en.wiktionary.org/wiki/obscuration> ,
    <https://en.wikipedia.org/wiki/Smoke_detector> ;
  rdfs:subClassOf
    ieso:RatioUnit ,
    [
      rdf:type owl:Restriction ;
      owl:onProperty ieso:isUnitOfMeasureOf ;
      owl:someValuesFrom ieso:ObscurationMeasure
    ] ;
  .
# !


###  https://www.gecad.isep.ipp.pt/ieso/v1.0.0/PartsPerNotationMeasure
ieso:PartsPerNotationMeasure
  rdf:type owl:Class ;
  rdfs:comment "In science and engineering, the parts-per notation is a set of pseudo-units to describe small values of miscellaneous dimensionless quantities, e.g. mole fraction or mass fraction. Since these fractions are quantity-per-quantity measures, they are pure numbers with no associated units of measurement."@en ;
  rdfs:label "Parts-per notation measure"@en ;
  rdfs:isDefinedBy <measure/v1.0.0/> ;
  rdfs:seeAlso <https://en.wikipedia.org/wiki/Parts-per_notation> ;
  rdfs:subClassOf
    ieso:TypeOfMeasure ,
    [
      rdf:type owl:Restriction ;
      owl:onProperty ieso:hasUnitOfMeasure ;
      owl:allValuesFrom ieso:PartsPerNotationUnit
    ] ;
  .
# !


###  https://www.gecad.isep.ipp.pt/ieso/v1.0.0/PartsPerNotationUnit
ieso:PartsPerNotationUnit
  rdf:type owl:Class ;
  rdfs:comment "Commonly used are parts-per-million (ppm, 10^6), parts-per-billion (ppb, 10^9), parts-per-trillion (ppt, 10^12) and parts-per-quadrillion (ppq, 10^15). This notation is not part of the International System of Units (SI) system and its meaning is ambiguous."@en ;
  rdfs:label "Parts-per notation unit"@en ;
  rdfs:isDefinedBy <measure/v1.0.0/> ;
  rdfs:seeAlso <https://en.wikipedia.org/wiki/Power_(physics)#Units> ;
  rdfs:subClassOf
    ieso:DimensionlessUnit ,
    [
      rdf:type owl:Restriction ;
      owl:onProperty ieso:isUnitOfMeasureOf ;
      owl:someValuesFrom ieso:PartsPerNotationMeasure
    ] ;
  .
# !


###  https://www.gecad.isep.ipp.pt/ieso/v1.0.0/PercentageMeasure
ieso:PercentageMeasure
  rdf:type owl:Class ;
  rdfs:comment "In mathematics, a percentage (from Latin per centum 'by a hundred') is a number or ratio expressed as a fraction of 100."@en ;
  rdfs:label "Percentage measure"@en ;
  rdfs:isDefinedBy <measure/v1.0.0/> ;
  rdfs:seeAlso <https://en.wikipedia.org/wiki/Percentage> ;
  rdfs:subClassOf
    ieso:RatioMeasure ,
    [
      rdf:type owl:Restriction ;
      owl:onProperty ieso:hasUnitOfMeasure ;
      owl:allValuesFrom ieso:PercentageUnit
    ] ;
  .
# !


###  https://www.gecad.isep.ipp.pt/ieso/v1.0.0/PercentageUnit
ieso:PercentageUnit
  rdf:type owl:Class ;
  rdfs:comment "A percentage is a dimensionless number (pure number); it has no unit of measurement. It is often denoted using the percent sign ('%') although the abbreviations 'pct.', 'pct' and sometimes 'pc' are also used."@en ;
  rdfs:label "Percentage unit"@en ;
  rdfs:isDefinedBy <measure/v1.0.0/> ;
  rdfs:seeAlso <https://en.wikipedia.org/wiki/Percentage#Related_units> ;
  rdfs:subClassOf
    ieso:RatioUnit ,
    [
      rdf:type owl:Restriction ;
      owl:onProperty ieso:isUnitOfMeasureOf ;
      owl:someValuesFrom ieso:PercentageMeasure
    ] ;
  .
# !


###  https://www.gecad.isep.ipp.pt/ieso/v1.0.0/PlaneAngleMeasure
ieso:PlaneAngleMeasure
  rdf:type owl:Class ;
  rdfs:comment "Euclid defines a plane angle as the inclination to each other, in a plane, of two lines which meet each other, and do not lie straight with respect to each other. According to Proclus, an angle must be either a quality or a quantity, or a relationship."@en ;
  rdfs:label "Plane angle measure"@en ;
  rdfs:isDefinedBy <measure/v1.0.0/> ;
  rdfs:seeAlso <https://en.wikipedia.org/wiki/Angle> ;
  rdfs:subClassOf
    ieso:AngleMeasure ,
    [
      rdf:type owl:Restriction ;
      owl:onProperty ieso:hasUnitOfMeasure ;
      owl:allValuesFrom ieso:PlaneAngleUnit
    ] ;
  .
# !


###  https://www.gecad.isep.ipp.pt/ieso/v1.0.0/PlaneAngleUnit
ieso:PlaneAngleUnit
  rdf:type owl:Class ;
  rdfs:comment "The degree and the radian are by far the most commonly used plane angle units."@en ;
  rdfs:label "Plane angle unit"@en ;
  rdfs:isDefinedBy <measure/v1.0.0/> ;
  rdfs:seeAlso
    <https://en.wikipedia.org/wiki/Angle#Units> ,
    <https://en.wikipedia.org/wiki/Angular_unit> ;
  rdfs:subClassOf
    ieso:AngleUnit ,
    [
      rdf:type owl:Restriction ;
      owl:onProperty ieso:isUnitOfMeasureOf ;
      owl:someValuesFrom ieso:PlaneAngleMeasure
    ] ,
    [
      rdf:type owl:Restriction ;
      owl:onProperty ieso:hasSIUnitOfMeasure ;
      owl:qualifiedCardinality "1"^^xsd:nonNegativeInteger ;
      owl:onClass ieso:PlaneAngleUnit
    ] ;
  .
# !


###  https://www.gecad.isep.ipp.pt/ieso/v1.0.0/PowerMeasure
ieso:PowerMeasure
  rdf:type owl:Class ;
  rdfs:comment "In physics, power is the amount of energy transferred or converted per unit time. In the International System of Units, the unit of power is the watt, equal to one joule per second. In older works, power is sometimes called activity. Power is a scalar quantity."@en ;
  rdfs:label "Power measure"@en ;
  rdfs:isDefinedBy <measure/v1.0.0/> ;
  rdfs:seeAlso <https://en.wikipedia.org/wiki/Power_(physics)> ;
  rdfs:subClassOf
    ieso:TypeOfMeasure ,
    [
      rdf:type owl:Restriction ;
      owl:onProperty ieso:hasUnitOfMeasure ;
      owl:allValuesFrom ieso:PowerUnit
    ] ;
  .
# !


###  https://www.gecad.isep.ipp.pt/ieso/v1.0.0/PowerUnit
ieso:PowerUnit
  rdf:type owl:Class ;
  rdfs:comment "The dimension of power is energy divided by time. In the International System of Units (SI), the unit of power is the watt (W), which is equal to one joule per second."@en ;
  rdfs:label "Power unit"@en ;
  rdfs:isDefinedBy <measure/v1.0.0/> ;
  rdfs:seeAlso <https://en.wikipedia.org/wiki/Power_(physics)#Units> ;
  rdfs:subClassOf
    ieso:DimensionalUnit ,
    [
      rdf:type owl:Restriction ;
      owl:onProperty ieso:isUnitOfMeasureOf ;
      owl:someValuesFrom ieso:PowerMeasure
    ] ,
    [
      rdf:type owl:Restriction ;
      owl:onProperty ieso:hasSIUnitOfMeasure ;
      owl:qualifiedCardinality "1"^^xsd:nonNegativeInteger ;
      owl:onClass ieso:PowerUnit
    ] ;
  .
# !


###  https://www.gecad.isep.ipp.pt/ieso/v1.0.0/RatioMeasure
ieso:RatioMeasure
  rdf:type owl:Class ;
  rdfs:comment "In mathematics, a ratio indicates how many times one number contains another."@en ;
  rdfs:label "Ratio measure"@en ;
  rdfs:isDefinedBy <measure/v1.0.0/> ;
  rdfs:seeAlso <https://en.wikipedia.org/wiki/Ratio> ;
  rdfs:subClassOf
    ieso:TypeOfMeasure ,
    [
      rdf:type owl:Restriction ;
      owl:onProperty ieso:hasUnitOfMeasure ;
      owl:allValuesFrom ieso:RatioUnit
    ] ;
  .
# !


###  https://www.gecad.isep.ipp.pt/ieso/v1.0.0/RatioUnit
ieso:RatioUnit
  rdf:type owl:Class ;
  rdfs:comment "Ratios may be unitless, as in the case they relate quantities in units of the same dimension, even if their units of measurement are initially different. For example, the ratio 1 minute  40 seconds can be reduced by changing the first value to 60 seconds, so the ratio becomes 60 seconds  40 seconds. Once the units are the same, they can be omitted, and the ratio can be reduced to 32."@en ;
  rdfs:label "Ratio unit"@en ;
  rdfs:isDefinedBy <measure/v1.0.0/> ;
  rdfs:seeAlso <https://en.wikipedia.org/wiki/Ratio#Units> ;
  rdfs:subClassOf
    ieso:DimensionlessUnit ,
    [
      rdf:type owl:Restriction ;
      owl:onProperty ieso:isUnitOfMeasureOf ;
      owl:someValuesFrom ieso:RatioMeasure
    ] ;
  .
# !


###  https://www.gecad.isep.ipp.pt/ieso/v1.0.0/SIUnitConverterTemplate
ieso:SIUnitConverterTemplate
  rdf:type owl:Class ;
  rdfs:comment "This class describes unit converter templates to enable automatic conversion of values with the same SI unit of measure. 'SI unit converter template' classes are used by MAS-Society software agents to automatically convert values from different inputs.\n\nA few individuals are available in the ontology, useful for our use cases. Others may be added to accomplish other use cases."@en ;
  rdfs:label "SI unit converter template"@en ;
  rdfs:isDefinedBy <measure/v1.0.0/> ;
  rdfs:subClassOf ieso:UnitConverterTemplate ;
  .
# !


###  https://www.gecad.isep.ipp.pt/ieso/v1.0.0/SolidAngleMeasure
ieso:SolidAngleMeasure
  rdf:type owl:Class ;
  rdfs:comment "In geometry, a solid angle (symbol: ) is a measure of the amount of the field of view from some particular point that a given object covers. That is, it is a measure of how large the object appears to an observer looking from that point. The point from which the object is viewed is called the apex of the solid angle, and the object is said to subtend its solid angle from that point."@en ;
  rdfs:label "Solid angle measure"@en ;
  rdfs:isDefinedBy <measure/v1.0.0/> ;
  rdfs:seeAlso <https://en.wikipedia.org/wiki/Solid_angle> ;
  rdfs:subClassOf
    ieso:AngleMeasure ,
    [
      rdf:type owl:Restriction ;
      owl:onProperty ieso:hasUnitOfMeasure ;
      owl:allValuesFrom ieso:SolidAngleUnit
    ] ;
  .
# !


###  https://www.gecad.isep.ipp.pt/ieso/v1.0.0/SolidAngleUnit
ieso:SolidAngleUnit
  rdf:type owl:Class ;
  rdfs:comment "In the International System of Units (SI), a solid angle is expressed in a dimensionless unit called a steradian (symbol: sr). One steradian corresponds to one unit of area on the unit sphere surrounding the apex, so an object that blocks all rays from the apex would cover a number of steradians equal to the total surface area of the unit sphere, 4pi . Solid angles can also be measured in squares of angular measures such as degrees, minutes, and seconds."@en ;
  rdfs:label "Solid angle unit"@en ;
  rdfs:isDefinedBy <measure/v1.0.0/> ;
  rdfs:seeAlso <https://en.wikipedia.org/wiki/Solid_angle> ;
  rdfs:subClassOf
    ieso:AngleUnit ,
    [
      rdf:type owl:Restriction ;
      owl:onProperty ieso:isUnitOfMeasureOf ;
      owl:someValuesFrom ieso:SolidAngleMeasure
    ] ,
    [
      rdf:type owl:Restriction ;
      owl:onProperty ieso:hasSIUnitOfMeasure ;
      owl:qualifiedCardinality "1"^^xsd:nonNegativeInteger ;
      owl:onClass ieso:SolidAngleUnit
    ] ;
  .
# !


###  https://www.gecad.isep.ipp.pt/ieso/v1.0.0/TemperatureMeasure
ieso:TemperatureMeasure
  rdf:type owl:Class ;
  rdfs:comment "Temperature is a physical quantity that expresses hot and cold. It is the manifestation of thermal energy, present in all matter, which is the source of the occurrence of heat, a flow of energy, when a body is in contact with another that is colder or hotter."@en ;
  rdfs:label "Temperature measure"@en ;
  rdfs:isDefinedBy <measure/v1.0.0/> ;
  rdfs:seeAlso
    <https://en.wikipedia.org/wiki/Temperature> ,
    <https://en.wikipedia.org/wiki/Temperature_measurement> ;
  rdfs:subClassOf
    ieso:TypeOfMeasure ,
    [
      rdf:type owl:Restriction ;
      owl:onProperty ieso:hasUnitOfMeasure ;
      owl:allValuesFrom ieso:TemperatureUnit
    ] ;
  .
# !


###  https://www.gecad.isep.ipp.pt/ieso/v1.0.0/TemperatureUnit
ieso:TemperatureUnit
  rdf:type owl:Class ;
  rdfs:comment """The basic unit of temperature in the International System of Units (SI) is the Kelvin. It has the symbol K.\n\nFor everyday applications, it is often convenient to use the Celsius scale, in which 0 C corresponds very closely to the freezing point of water and 100 C is its boiling point at sea level. Because liquid droplets commonly exist in clouds at sub-zero temperatures, 0 C is better defined as the melting point of ice. In this scale, a temperature difference of 1 degree Celsius is the same as a 1kelvin increment, but the scale is offset by the temperature at which ice melts (273.15 K)."""@en ;
  rdfs:label "Temperature unit"@en ;
  rdfs:isDefinedBy <measure/v1.0.0/> ;
  rdfs:seeAlso
    <https://en.wikipedia.org/wiki/Temperature_measurement> ,
    <https://en.wikipedia.org/wiki/Temperature#Units> ;
  rdfs:subClassOf
    ieso:DimensionalUnit ,
    [
      rdf:type owl:Restriction ;
      owl:onProperty ieso:isUnitOfMeasureOf ;
      owl:someValuesFrom ieso:TemperatureMeasure
    ] ,
    [
      rdf:type owl:Restriction ;
      owl:onProperty ieso:hasSIUnitOfMeasure ;
      owl:qualifiedCardinality "1"^^xsd:nonNegativeInteger ;
      owl:onClass ieso:TemperatureUnit
    ] ;
  .
# !


###  https://www.gecad.isep.ipp.pt/ieso/v1.0.0/TimeMeasure
ieso:TimeMeasure
  rdf:type owl:Class ;
  rdfs:comment "Time is the indefinite continued progress of existence and events that occur in an apparently irreversible succession from the past, through the present, into the future. It is a component quantity of various measurements used to sequence events, to compare the duration of events or the intervals between them, and to quantify rates of change of quantities in material reality or in the conscious experience. Time is often referred to as a fourth dimension, along with three spatial dimensions."@en ;
  rdfs:label "Time measure"@en ;
  rdfs:isDefinedBy <measure/v1.0.0/> ;
  rdfs:seeAlso <https://en.wikipedia.org/wiki/Time> ;
  rdfs:subClassOf
    ieso:TypeOfMeasure ,
    [
      rdf:type owl:Restriction ;
      owl:onProperty ieso:hasUnitOfMeasure ;
      owl:allValuesFrom ieso:TimeUnit
    ] ;
  .
# !


###  https://www.gecad.isep.ipp.pt/ieso/v1.0.0/TimeUnit
ieso:TimeUnit
  rdf:type owl:Class ;
  rdfs:comment "The second (s) is the SI base unit. A minute (min) is 60 seconds in length, and an hour is 60 minutes or 3600 seconds in length. A day is usually 24 hours or 86,400 seconds in length; however, the duration of a calendar day can vary due to Daylight saving time and Leap seconds."@en ;
  rdfs:label "Time unit"@en ;
  rdfs:isDefinedBy <measure/v1.0.0/> ;
  rdfs:seeAlso
    <https://en.wikipedia.org/wiki/Unit_of_time> ,
    <https://en.wikipedia.org/wiki/Orders_of_magnitude_(time)> ,
    <https://en.wikipedia.org/wiki/Time#Units> ;
  rdfs:subClassOf
    ieso:DimensionalUnit ,
    [
      rdf:type owl:Restriction ;
      owl:onProperty ieso:isUnitOfMeasureOf ;
      owl:someValuesFrom ieso:TimeMeasure
    ] ,
    [
      rdf:type owl:Restriction ;
      owl:onProperty ieso:hasSIUnitOfMeasure ;
      owl:qualifiedCardinality "1"^^xsd:nonNegativeInteger ;
      owl:onClass ieso:TimeUnit
    ] ;
  .
# !


###  https://www.gecad.isep.ipp.pt/ieso/v1.0.0/TypeOfMeasure
ieso:TypeOfMeasure
  rdf:type owl:Class ;
  rdfs:comment "This class describes types of measure related to measures and respective units of measure."@en ;
  rdfs:label "Type of measure"@en ;
  rdfs:isDefinedBy <measure/v1.0.0/> ;
  rdfs:subClassOf
    [
      rdf:type owl:Restriction ;
      owl:onProperty ieso:hasUnitOfMeasure ;
      owl:allValuesFrom ieso:UnitOfMeasure
    ] ,
    [
      rdf:type owl:Restriction ;
      owl:onProperty ieso:isTypeOfMeasureOf ;
      owl:allValuesFrom ieso:Measurement
    ] ;
  .
# !


###  https://www.gecad.isep.ipp.pt/ieso/v1.0.0/UnitConverterTemplate
ieso:UnitConverterTemplate
  rdf:type owl:Class ;
  rdfs:comment "This class describes unit converter templates to enable automatic conversion of values. 'Unit converter template' classes are used by MAS-Society software agents to automatically convert values from different inputs."@en ;
  rdfs:label "Unit converter template"@en ;
  rdfs:isDefinedBy <measure/v1.0.0/> ;
  rdfs:subClassOf
    [
      rdf:type owl:Restriction ;
      owl:onProperty ieso:conversionTemplate ;
      owl:cardinality "1"^^xsd:nonNegativeInteger ;
      owl:onDataRange xsd:string
    ] ,
    [
      rdf:type owl:Restriction ;
      owl:onProperty ieso:conversionTemplateSyntax ;
      owl:cardinality "1"^^xsd:nonNegativeInteger ;
      owl:onDataRange [
        rdf:type rdfs:Datatype ;
        owl:oneOf [
          rdf:type rdf:List ;
          rdf:first "SPARQL" ;
          rdf:rest [
            rdf:type rdf:List ;
            rdf:first "SQWRL" ;
            rdf:rest [
              rdf:type rdf:List ;
              rdf:first "SWRL" ;
              rdf:rest rdf:nil
            ]
          ]
        ]
      ]
    ] ;
  .
# !


###  https://www.gecad.isep.ipp.pt/ieso/v1.0.0/UnitOfMeasure
ieso:UnitOfMeasure
  rdf:type owl:Class ;
  rdfs:comment "A unit of measure is a definite magnitude of a quantity, defined and adopted by convention or by law, that is used as a standard for measure of the same kind of quantity."@en ;
  rdfs:label "Unit of measure"@en ;
  rdfs:isDefinedBy <measure/v1.0.0/> ;
  rdfs:seeAlso <https://en.wikipedia.org/wiki/Unit_of_measure> ;
  rdfs:subClassOf
    [
      rdf:type owl:Restriction ;
      owl:onProperty ieso:isUnitOfMeasureOf ;
      owl:someValuesFrom ieso:Measurement
    ] ,
    [
      rdf:type owl:Restriction ;
      owl:onProperty ieso:isUnitOfMeasureOf ;
      owl:someValuesFrom ieso:MeasurementValue
    ] ,
    [
      rdf:type owl:Restriction ;
      owl:onProperty ieso:isUnitOfMeasureOf ;
      owl:someValuesFrom ieso:TypeOfMeasure
    ] ,
    [
      rdf:type owl:Restriction ;
      owl:onProperty ieso:unitSymbol ;
      owl:someValuesFrom rdfs:Literal
    ] ;
  .
# !


###  https://www.gecad.isep.ipp.pt/ieso/v1.0.0/VelocityMeasure
ieso:VelocityMeasure
  rdf:type owl:Class ;
  rdfs:comment "The velocity of an object is the rate of change of its position with respect to a frame of reference, and is a function of time. Velocity is equivalent to a specification of an object's speed and direction of motion (e.g. 60 km/h to the north). Velocity is a fundamental concept in kinematics, the branch of classical mechanics that describes the motion of bodies."@en ;
  rdfs:label "Velocity measure"@en ;
  rdfs:isDefinedBy <measure/v1.0.0/> ;
  rdfs:seeAlso
    <https://en.wikipedia.org/wiki/Speed> ,
    <https://en.wikipedia.org/wiki/Velocity> ;
  rdfs:subClassOf
    ieso:TypeOfMeasure ,
    [
      rdf:type owl:Restriction ;
      owl:onProperty ieso:hasUnitOfMeasure ;
      owl:allValuesFrom ieso:VelocityUnit
    ] ;
  .
# !


###  https://www.gecad.isep.ipp.pt/ieso/v1.0.0/VelocityUnit
ieso:VelocityUnit
  rdf:type owl:Class ;
  rdfs:comment "Velocity is a physical vector quantity; both magnitude and direction are needed to define it. The scalar absolute value (magnitude) of velocity is called speed, being a coherent derived unit whose quantity is measured in the SI (metric system) as metres per second (m/s) or as the SI base unit of (ms1)."@en ;
  rdfs:label "Velocity unit"@en ;
  rdfs:isDefinedBy <measure/v1.0.0/> ;
  rdfs:seeAlso
    <https://en.wikipedia.org/wiki/Velocity> ,
    <https://en.wikipedia.org/wiki/Speed#Units> ;
  rdfs:subClassOf
    ieso:DimensionalUnit ,
    [
      rdf:type owl:Restriction ;
      owl:onProperty ieso:isUnitOfMeasureOf ;
      owl:someValuesFrom ieso:VelocityMeasure
    ] ,
    [
      rdf:type owl:Restriction ;
      owl:onProperty ieso:hasSIUnitOfMeasure ;
      owl:qualifiedCardinality "1"^^xsd:nonNegativeInteger ;
      owl:onClass ieso:VelocityUnit
    ] ;
  .
# !


###  https://www.gecad.isep.ipp.pt/ieso/v1.0.0/VolatileOrganicCompoundMeasure
ieso:VolatileOrganicCompoundMeasure
  rdf:type owl:Class ;
  rdfs:comment "Volatile organic compounds (VOCs) are organic compounds that have a high vapor pressure at room temperature. High vapor pressure correlates with a low boiling point, which relates to the number of the sample's molecules in the surrounding air, a trait known as volatility."@en ;
  rdfs:label "Volatile organic compound measure"@en ;
  rdfs:isDefinedBy <measure/v1.0.0/> ;
  rdfs:seeAlso <https://en.wikipedia.org/wiki/Volatile_organic_compound> ;
  rdfs:subClassOf
    ieso:TypeOfMeasure ,
    [
      rdf:type owl:Restriction ;
      owl:onProperty ieso:hasUnitOfMeasure ;
      owl:allValuesFrom ieso:PartsPerNotationUnit
    ]
  .
# !


###  https://www.gecad.isep.ipp.pt/ieso/v1.0.0/VolumeMeasure
ieso:VolumeMeasure
  rdf:type owl:Class ;
  rdfs:comment "Volume is the quantity of three-dimensional space enclosed by a closed surface, for example, the space that a substance (solid, liquid, gas, or plasma) or shape occupies or contains."@en ;
  rdfs:label "Volume measure"@en ;
  rdfs:isDefinedBy <measure/v1.0.0/> ;
  rdfs:seeAlso <https://en.wikipedia.org/wiki/Volume> ;
  rdfs:subClassOf
    ieso:TypeOfMeasure ,
    [
      rdf:type owl:Restriction ;
      owl:onProperty ieso:hasUnitOfMeasure ;
      owl:allValuesFrom ieso:VolumeUnit
    ] ;
  .
# !


###  https://www.gecad.isep.ipp.pt/ieso/v1.0.0/VolumeUnit
ieso:VolumeUnit
  rdf:type owl:Class ;
  rdfs:comment "Any unit of length gives a corresponding unit of volume: the volume of a cube whose sides have the given length. In the International System of Units (SI), the standard unit of volume is the cubic metre (m3). The metric system also includes the litre (L) as a unit of volume, where one litre is the volume of a 10-centimetre cube."@en ;
  rdfs:label "Volume unit"@en ;
  rdfs:isDefinedBy <measure/v1.0.0/> ;
  rdfs:seeAlso <https://en.wikipedia.org/wiki/Volume#Units> ;
  rdfs:subClassOf
    ieso:DimensionalUnit ,
    [
      rdf:type owl:Restriction ;
      owl:onProperty ieso:isUnitOfMeasureOf ;
      owl:someValuesFrom ieso:VolumeMeasure
    ] ,
    [
      rdf:type owl:Restriction ;
      owl:onProperty ieso:hasSIUnitOfMeasure ;
      owl:qualifiedCardinality "1"^^xsd:nonNegativeInteger ;
      owl:onClass ieso:VolumeUnit
    ] ;
  .
# !


###  https://www.gecad.isep.ipp.pt/ieso/v1.0.0/VoltageMeasure
ieso:VoltageMeasure
  rdf:type owl:Class ;
  rdfs:comment "Voltage, electric potential difference, electromotive force emf, electric pressure or electric tension is the difference in electric potential between two points, which (in a static electric field) is defined as the work needed per unit of charge to move a test charge between the two points."@en ;
  rdfs:label "Voltage measure"@en ;
  rdfs:isDefinedBy <measure/v1.0.0/> ;
  rdfs:seeAlso <https://en.wikipedia.org/wiki/Voltage> ;
  rdfs:subClassOf
    ieso:TypeOfMeasure ,
    [
      rdf:type owl:Restriction ;
      owl:onProperty ieso:hasUnitOfMeasure ;
      owl:allValuesFrom ieso:VoltageUnit
    ] ;
  .
# !


###  https://www.gecad.isep.ipp.pt/ieso/v1.0.0/VoltageUnit
ieso:VoltageUnit
  rdf:type owl:Class ;
  rdfs:comment "In the International System of Units, the derived unit for voltage (potential difference) is named volt.[1]:166 In SI units, work per unit charge is expressed as joules per coulomb, where 1 volt = 1 joule (of work) per 1 coulomb (of charge)."@en ;
  rdfs:label "Voltage unit"@en ;
  rdfs:isDefinedBy <measure/v1.0.0/> ;
  rdfs:seeAlso <https://en.wikipedia.org/wiki/Voltage> ;
  rdfs:subClassOf
    ieso:DimensionalUnit ,
    [
      rdf:type owl:Restriction ;
      owl:onProperty ieso:isUnitOfMeasureOf ;
      owl:someValuesFrom ieso:VoltageMeasure
    ] ,
    [
      rdf:type owl:Restriction ;
      owl:onProperty ieso:hasSIUnitOfMeasure ;
      owl:qualifiedCardinality "1"^^xsd:nonNegativeInteger ;
      owl:onClass ieso:VoltageUnit
    ] ;
  .
# !


#################################################################
#  Individuals
#################################################################


###  https://www.gecad.isep.ipp.pt/ieso/v1.0.0/Abvolt
ieso:Abvolt
  rdf:type
    owl:NamedIndividual ,
    ieso:VoltageUnit ;
  rdfs:comment "The abvolt (abV) is the unit of potential difference in the CGS-EMU system of units. It corresponds to 10^8 volt in the SI system."@en ;
  rdfs:label "abvolt"@en ;
  rdfs:isDefinedBy <measure/v1.0.0/> ;
  rdfs:seeAlso
    <https://en.wikipedia.org/wiki/Conversion_of_units#Electromotive_force,_electric_potential_difference> ,
    <https://en.wikipedia.org/wiki/Abvolt> ;
  ieso:hasSIUnitOfMeasure ieso:Volt ;
  ieso:conversionCoefficientToSIUnit "1.0e-8"^^xsd:double ;
  ieso:conversionOffsetToSIUnit "0.0"^^xsd:double ;
  ieso:unitSymbol "abV"^^rdfs:Literal ;
  .
# !


###  https://www.gecad.isep.ipp.pt/ieso/v1.0.0/Ampere
ieso:Ampere
  rdf:type
    owl:NamedIndividual ,
    ieso:ElectricCurrentUnit ;
  rdfs:comment "The ampere (symbol: A), often shortened to 'amp', is the base unit of electric current in the International System of Units (SI)."@en ;
  rdfs:label "ampere"@en ;
  rdfs:isDefinedBy <measure/v1.0.0/> ;
  rdfs:seeAlso
    <https://en.wikipedia.org/wiki/Conversion_of_units#Electric_current> ,
    <https://en.wikipedia.org/wiki/Ampere> ;
  ieso:hasSIUnitOfMeasure ieso:Ampere ;
  ieso:conversionCoefficientToSIUnit "1.0"^^xsd:double ;
  ieso:conversionOffsetToSIUnit "0.0"^^xsd:double ;
  ieso:unitSymbol "A"^^rdfs:Literal ;
  .
# !


###  https://www.gecad.isep.ipp.pt/ieso/v1.0.0/Kiloampere
ieso:Kilompere
  rdf:type
    owl:NamedIndividual ,
    ieso:ElectricCurrentUnit ;
  rdfs:comment "The kiloampere (symbol: kA), is a multiple of ampere in the order of 10^3."@en ;
  rdfs:label "kiloampere"@en ;
  rdfs:isDefinedBy <measure/v1.0.0/> ;
  rdfs:seeAlso
    <https://en.wikipedia.org/wiki/Conversion_of_units#Electric_current> ,
    <https://en.wikipedia.org/wiki/Ampere> ;
  ieso:hasSIUnitOfMeasure ieso:Ampere ;
  ieso:conversionCoefficientToSIUnit "1000.0"^^xsd:double ;
  ieso:conversionOffsetToSIUnit "0.0"^^xsd:double ;
  ieso:unitSymbol "kA"^^rdfs:Literal ;
  .
# !


###  https://www.gecad.isep.ipp.pt/ieso/v1.0.0/AmpereHour
ieso:AmpereHour
  rdf:type
    owl:NamedIndividual ,
    ieso:ElectricChargeUnit ;
  rdfs:comment "An ampere hour or amp hour (symbol: Ah or A h; often also unofficially denoted as Ah) is a unit of electric charge, having dimensions of electric current multiplied by time, equal to the charge transferred by a steady current of one ampere flowing for one hour, or 3,600 coulombs."@en ;
  rdfs:label "ampere hour"@en ;
  rdfs:isDefinedBy <measure/v1.0.0/> ;
  rdfs:seeAlso
    <https://en.wikipedia.org/wiki/Conversion_of_units#Electric_charge> ,
    <https://en.wikipedia.org/wiki/Ampere_hour> ;
  ieso:hasSIUnitOfMeasure ieso:Coulomb ;
  ieso:conversionCoefficientToSIUnit "3.6e3"^^xsd:double ;
  ieso:conversionOffsetToSIUnit "0.0"^^xsd:double ;
  ieso:unitSymbol "Ah"^^rdfs:Literal ;
  .
# !


###  https://www.gecad.isep.ipp.pt/ieso/v1.0.0/Candela
ieso:Candela
  rdf:type
    owl:NamedIndividual ,
    ieso:LuminousIntensityUnit ;
  rdfs:comment "The candela (symbol: cd) is the base unit of luminous intensity in the International System of Units (SI); that is, luminous power per unit solid angle emitted by a point light source in a particular direction."@en ;
  rdfs:label "candela"@en ;
  rdfs:isDefinedBy <measure/v1.0.0/> ;
  rdfs:seeAlso
    <https://en.wikipedia.org/wiki/Conversion_of_units#Luminous_intensity> ,
    <https://en.wikipedia.org/wiki/Candela> ;
  ieso:hasSIUnitOfMeasure ieso:Candela ;
  ieso:conversionCoefficientToSIUnit "1.0"^^xsd:double ;
  ieso:conversionOffsetToSIUnit "0.0"^^xsd:double ;
  ieso:unitSymbol "cd"^^rdfs:Literal ;
  .
# !


###  https://www.gecad.isep.ipp.pt/ieso/v1.0.0/CandelaPerSquareFoot
ieso:CandelaPerSquareFoot
  rdf:type
    owl:NamedIndividual ,
    ieso:LuminanceUnit ;
  rdfs:comment "A derived unit from the SI candela per square metre unit."@en ;
  rdfs:label "candela per square foot"@en ;
  rdfs:isDefinedBy <measure/v1.0.0/> ;
  rdfs:seeAlso <https://en.wikipedia.org/wiki/Conversion_of_units#Luminance> ;
  ieso:hasSIUnitOfMeasure ieso:CandelaPerSquareMetre ;
  ieso:conversionCoefficientToSIUnit "10.763910417"^^xsd:double ;
  ieso:conversionOffsetToSIUnit "0.0"^^xsd:double ;
  ieso:unitSymbol "cd/ft^2"^^rdfs:Literal ;
  .
# !


###  https://www.gecad.isep.ipp.pt/ieso/v1.0.0/CandelaPerSquareInch
ieso:CandelaPerSquareInch
  rdf:type
    owl:NamedIndividual ,
    ieso:LuminanceUnit ;
  rdfs:comment "A derived unit from the SI candela per square metre unit."@en ;
  rdfs:label "candela per square inch"@en ;
  rdfs:isDefinedBy <measure/v1.0.0/> ;
  rdfs:seeAlso <https://en.wikipedia.org/wiki/Conversion_of_units#Luminance> ;
  ieso:hasSIUnitOfMeasure ieso:CandelaPerSquareMetre ;
  ieso:conversionCoefficientToSIUnit "1.5500031e3"^^xsd:double ;
  ieso:conversionOffsetToSIUnit "0.0"^^xsd:double ;
  ieso:unitSymbol "cd/in^2"^^rdfs:Literal ;
  .
# !


###  https://www.gecad.isep.ipp.pt/ieso/v1.0.0/CandelaPerSquareMetre
ieso:CandelaPerSquareMetre
  rdf:type
    owl:NamedIndividual ,
    ieso:LuminanceUnit ;
  rdfs:comment "The candela per square metre (symbol: cd/m^2) is the derived SI unit of luminance. The unit is based on the candela, the SI unit of luminous intensity, and the square metre, the SI unit of area."@en ;
  rdfs:label "candela per square metre"@en ;
  rdfs:isDefinedBy <measure/v1.0.0/> ;
  rdfs:seeAlso
    <https://en.wikipedia.org/wiki/Conversion_of_units#Luminance> ,
    <https://en.wikipedia.org/wiki/Candela_per_square_metre> ;
  ieso:hasSIUnitOfMeasure ieso:CandelaPerSquareMetre ;
  ieso:conversionCoefficientToSIUnit "1.0"^^xsd:double ;
  ieso:conversionOffsetToSIUnit "0.0"^^xsd:double ;
  ieso:unitSymbol "cd/m^2"^^rdfs:Literal ;
  .
# !


###  https://www.gecad.isep.ipp.pt/ieso/v1.0.0/Celsius
ieso:Celsius
  rdf:type
    owl:NamedIndividual ,
    ieso:TemperatureUnit ;
  rdfs:comment "The degree Celsius is a unit of temperature on the Celsius scale, a temperature scale originally known as the centigrade scale. The degree Celsius (symbol: C) can refer to a specific temperature on the Celsius scale or a unit to indicate a difference between two temperatures or an uncertainty."@en ;
  rdfs:label "celsius"@en ;
  rdfs:isDefinedBy <measure/v1.0.0/> ;
  rdfs:seeAlso
    <https://en.wikipedia.org/wiki/Conversion_of_units#Temperature> ,
    <https://en.wikipedia.org/wiki/Celsius> ;
  ieso:hasSIUnitOfMeasure ieso:Kelvin ;
  ieso:conversionCoefficientToSIUnit "1.0"^^xsd:double ;
  ieso:conversionOffsetToSIUnit "273.15"^^xsd:double ;
  ieso:unitSymbol "C"^^rdfs:Literal ;
  .
# !


###  https://www.gecad.isep.ipp.pt/ieso/v1.0.0/Centilitre
ieso:Centilitre
  rdf:type
    owl:NamedIndividual ,
    ieso:VolumeUnit ;
  rdfs:comment "The centilitre (British English spelling) or centiliter (American English spelling) (SI symbols cL and cl) is a metric unit of volume. It is equal to ten cubic centimetres."@en ;
  rdfs:label "centilitre"@en ;
  rdfs:isDefinedBy <measure/v1.0.0/> ;
  rdfs:seeAlso <https://en.wikipedia.org/wiki/Litre#SI_prefixes_applied_to_the_litre> ;
  ieso:hasSIUnitOfMeasure ieso:CubicMetre ;
  ieso:conversionCoefficientToSIUnit "1.0e-5"^^xsd:double ;
  ieso:conversionOffsetToSIUnit "0.0"^^xsd:double ;
  ieso:unitSymbol "cl"^^rdfs:Literal ;
  .
# !


###  https://www.gecad.isep.ipp.pt/ieso/v1.0.0/Centimetre
ieso:Centimetre
  rdf:type
    owl:NamedIndividual ,
    ieso:LengthUnit ;
  rdfs:comment "A centimetre (international spelling) or centimeter (American spelling) (SI symbol cm) is a unit of length in the metric system, equal to one hundredth of a metre, centi being the SI prefix for a factor of 1/100. The centimetre was the base unit of length in the now deprecated centimetregramsecond (CGS) system of units."@en ;
  rdfs:label "centimetre"@en ;
  rdfs:isDefinedBy <measure/v1.0.0/> ;
  rdfs:seeAlso
    <https://en.wikipedia.org/wiki/Conversion_of_units#Length> ,
    <https://en.wikipedia.org/wiki/Metre#SI_prefixed_forms_of_metre> ,
    <https://en.wikipedia.org/wiki/Centimetre> ;
  ieso:hasSIUnitOfMeasure ieso:Metre ;
  ieso:conversionCoefficientToSIUnit "1.0e-2"^^xsd:double ;
  ieso:conversionOffsetToSIUnit "0.0"^^xsd:double ;
  ieso:unitSymbol "cm"^^rdfs:Literal ;
  .
# !


###  https://www.gecad.isep.ipp.pt/ieso/v1.0.0/Coulomb
ieso:Coulomb
  rdf:type
    owl:NamedIndividual ,
    ieso:ElectricChargeUnit ;
  rdfs:comment "The coulomb (symbol: C) is the International System of Units (SI) unit of electric charge."@en ;
  rdfs:label "coulomb"@en ;
  rdfs:isDefinedBy <measure/v1.0.0/> ;
  rdfs:seeAlso
    <https://en.wikipedia.org/wiki/Conversion_of_units#Electric_charge> ,
    <https://en.wikipedia.org/wiki/Coulomb> ;
  ieso:hasSIUnitOfMeasure ieso:Coulomb ;
  ieso:conversionCoefficientToSIUnit "1.0"^^xsd:double ;
  ieso:conversionOffsetToSIUnit "0.0"^^xsd:double ;
  ieso:unitSymbol "C"^^rdfs:Literal ;
  .
# !


###  https://www.gecad.isep.ipp.pt/ieso/v1.0.0/CubicCentimetre
ieso:CubicCentimetre
  rdf:type
    owl:NamedIndividual ,
    ieso:VolumeUnit ;
  rdfs:comment "The cubic centimetre (in Commonwealth English and international spelling as used by the International Bureau of Weights and Measures) or cubic centimeter (in American English) is the SI derived unit of volume. Its SI symbol is cm^3. It is the volume of a cube with edges one centimetre in length."@en ;
  rdfs:label "cubic centimetre"@en ;
  rdfs:isDefinedBy <measure/v1.0.0/> ;
  rdfs:seeAlso
    <https://en.wikipedia.org/wiki/Conversion_of_units#Volume> ,
    <https://en.wikipedia.org/wiki/Cubic_metre#Multiples_and_submultiples> ,
    <https://en.wikipedia.org/wiki/Volume#Units> ;
  ieso:hasSIUnitOfMeasure ieso:CubicMetre ;
  ieso:conversionCoefficientToSIUnit "1.0e-6"^^xsd:double ;
  ieso:conversionOffsetToSIUnit "0.0"^^xsd:double ;
  ieso:unitSymbol "cm^3"^^rdfs:Literal ;
  .
# !


###  https://www.gecad.isep.ipp.pt/ieso/v1.0.0/CubicDecametre
ieso:CubicDecametre
  rdf:type
    owl:NamedIndividual ,
    ieso:VolumeUnit ;
  rdfs:comment "The cubic decametre (in Commonwealth English and international spelling as used by the International Bureau of Weights and Measures) or cubic decameter (in American English) is the SI derived unit of volume. Its SI symbol is dam^3. It is the volume of a cube with edges one decametre in length."@en ;
  rdfs:label "cubic decametre"@en ;
  rdfs:isDefinedBy <measure/v1.0.0/> ;
  rdfs:seeAlso <https://en.wikipedia.org/wiki/Cubic_metre#Multiples_and_submultiples> ;
  ieso:hasSIUnitOfMeasure ieso:CubicMetre ;
  ieso:conversionCoefficientToSIUnit "1.0e3"^^xsd:double ;
  ieso:conversionOffsetToSIUnit "0.0"^^xsd:double ;
  ieso:unitSymbol "dam^3"^^rdfs:Literal ;
  .
# !


###  https://www.gecad.isep.ipp.pt/ieso/v1.0.0/CubicDecimetre
ieso:CubicDecimetre
  rdf:type
    owl:NamedIndividual ,
    ieso:VolumeUnit ;
  rdfs:comment "The cubic decimetre (in Commonwealth English and international spelling as used by the International Bureau of Weights and Measures) or cubic decimeter (in American English) is the SI derived unit of volume. Its SI symbol is dm^-3. It is the volume of a cube with edges one decimetre in length."@en ;
  rdfs:label "cubic decimetre"@en ;
  rdfs:isDefinedBy <measure/v1.0.0/> ;
  rdfs:seeAlso <https://en.wikipedia.org/wiki/Cubic_metre#Multiples_and_submultiples> ;
  ieso:hasSIUnitOfMeasure ieso:CubicMetre ;
  ieso:conversionCoefficientToSIUnit "1.0e-3"^^xsd:double ;
  ieso:conversionOffsetToSIUnit "0.0"^^xsd:double ;
  ieso:unitSymbol "dm^3"^^rdfs:Literal ;
  .
# !


###  https://www.gecad.isep.ipp.pt/ieso/v1.0.0/CubicHectometre
ieso:CubicHectometre
  rdf:type
    owl:NamedIndividual ,
    ieso:VolumeUnit ;
  rdfs:comment "The cubic hectometre (in Commonwealth English and international spelling as used by the International Bureau of Weights and Measures) or cubic hectometer (in American English) is the SI derived unit of volume. Its SI symbol is hm^3. It is the volume of a cube with edges one hectometre in length."@en ;
  rdfs:label "cubic hectometre"@en ;
  rdfs:isDefinedBy <measure/v1.0.0/> ;
  rdfs:seeAlso <https://en.wikipedia.org/wiki/Cubic_metre#Multiples_and_submultiples> ;
  ieso:hasSIUnitOfMeasure ieso:CubicMetre ;
  ieso:conversionCoefficientToSIUnit "1.0e6"^^xsd:double ;
  ieso:conversionOffsetToSIUnit "0.0"^^xsd:double ;
  ieso:unitSymbol "hm^3"^^rdfs:Literal ;
  .
# !


###  https://www.gecad.isep.ipp.pt/ieso/v1.0.0/CubicKilometre
ieso:CubicKilometre
  rdf:type
    owl:NamedIndividual ,
    ieso:VolumeUnit ;
  rdfs:comment "The cubic kilometre (in Commonwealth English and international spelling as used by the International Bureau of Weights and Measures) or cubic kilometer (in American English) is the SI derived unit of volume. Its SI symbol is km^3. It is the volume of a cube with edges one kilometre in length."@en ;
  rdfs:label "cubic kilometre"@en ;
  rdfs:isDefinedBy <measure/v1.0.0/> ;
  rdfs:seeAlso <https://en.wikipedia.org/wiki/Cubic_metre#Multiples_and_submultiples> ;
  ieso:hasSIUnitOfMeasure ieso:CubicMetre ;
  ieso:conversionCoefficientToSIUnit "1.0e9"^^xsd:double ;
  ieso:conversionOffsetToSIUnit "0.0"^^xsd:double ;
  ieso:unitSymbol "km^3"^^rdfs:Literal ;
  .
# !


###  https://www.gecad.isep.ipp.pt/ieso/v1.0.0/CubicMetre
ieso:CubicMetre
  rdf:type
    owl:NamedIndividual ,
    ieso:VolumeUnit ;
  rdfs:comment "The cubic metre (in Commonwealth English and international spelling as used by the International Bureau of Weights and Measures) or cubic meter (in American English) is the SI derived unit of volume. Its SI symbol is m^3. It is the volume of a cube with edges one metre in length."@en ;
  rdfs:label "cubic metre"@en ;
  rdfs:isDefinedBy <measure/v1.0.0/> ;
  rdfs:seeAlso
    <https://en.wikipedia.org/wiki/Conversion_of_units#Volume> ,
    <https://en.wikipedia.org/wiki/Cubic_metre> ,
    <https://en.wikipedia.org/wiki/Volume#Units> ;
  ieso:hasSIUnitOfMeasure ieso:CubicMetre ;
  ieso:conversionCoefficientToSIUnit "1.0"^^xsd:double ;
  ieso:conversionOffsetToSIUnit "0.0"^^xsd:double ;
  ieso:unitSymbol "m^3"^^rdfs:Literal ;
  .
# !


###  https://www.gecad.isep.ipp.pt/ieso/v1.0.0/CubicMillimetre
ieso:CubicMillimetre
  rdf:type
    owl:NamedIndividual ,
    ieso:VolumeUnit ;
  rdfs:comment "The cubic millimetre (in Commonwealth English and international spelling as used by the International Bureau of Weights and Measures) or cubic millimeter (in American English) is the SI derived unit of volume. Its SI symbol is mm^3. It is the volume of a cube with edges one millimetre in length."@en ;
  rdfs:label "cubic millimetre"@en ;
  rdfs:isDefinedBy <measure/v1.0.0/> ;
  rdfs:seeAlso <https://en.wikipedia.org/wiki/Cubic_metre#Multiples_and_submultiples> ;
  ieso:hasSIUnitOfMeasure ieso:CubicMetre ;
  ieso:conversionCoefficientToSIUnit "1.0e-9"^^xsd:double ;
  ieso:conversionOffsetToSIUnit "0.0"^^xsd:double ;
  ieso:unitSymbol "mm^3"^^rdfs:Literal ;
  .
# !


###  https://www.gecad.isep.ipp.pt/ieso/v1.0.0/Day
ieso:Day
  rdf:type
    owl:NamedIndividual ,
    ieso:TimeUnit ;
  rdfs:comment "A day is approximately the period during which the Earth completes one rotation around its axis, which takes around 24 hours. The unit of measurement 'day' (symbol d) is defined as 86400 SI seconds (the SI base unit of time)."@en ;
  rdfs:label "day"@en ;
  rdfs:isDefinedBy <measure/v1.0.0/> ;
  rdfs:seeAlso
    <https://en.wikipedia.org/wiki/Conversion_of_units#Time> ,
    <https://en.wikipedia.org/wiki/Day> ;
  ieso:hasSIUnitOfMeasure ieso:Second ;
  ieso:conversionCoefficientToSIUnit "8.64e4"^^xsd:double ;
  ieso:conversionOffsetToSIUnit "0.0"^^xsd:double ;
  ieso:unitSymbol "d"^^rdfs:Literal ;
  .
# !


###  https://www.gecad.isep.ipp.pt/ieso/v1.0.0/Decalitre
ieso:Decalitre
  rdf:type
    owl:NamedIndividual ,
    ieso:VolumeUnit ;
  rdfs:comment "The decalitre (British English spelling) or decaliter (American English spelling) (SI symbols daL and dal) is a metric unit of volume. It is equal to ten cubic decimetres."@en ;
  rdfs:label "decalitre"@en ;
  rdfs:isDefinedBy <measure/v1.0.0/> ;
  rdfs:seeAlso <https://en.wikipedia.org/wiki/Litre#SI_prefixes_applied_to_the_litre> ;
  ieso:hasSIUnitOfMeasure ieso:CubicMetre ;
  ieso:conversionCoefficientToSIUnit "1.0e-2"^^xsd:double ;
  ieso:conversionOffsetToSIUnit "0.0"^^xsd:double ;
  ieso:unitSymbol "dal"^^rdfs:Literal ;
  .
# !


###  https://www.gecad.isep.ipp.pt/ieso/v1.0.0/Decametre
ieso:Decametre
  rdf:type
    owl:NamedIndividual ,
    ieso:LengthUnit ;
  rdfs:comment "A decametre (International spelling as used by the International Bureau of Weights and Measures), with American spelling dekameter or decameter, symbol dam, is a unit of length in the International (metric) System of Units equal to ten metres."@en ;
  rdfs:label "decametre"@en ;
  rdfs:isDefinedBy <measure/v1.0.0/> ;
  rdfs:seeAlso
    <https://en.wikipedia.org/wiki/Conversion_of_units#Length> ,
    <https://en.wikipedia.org/wiki/Metre#SI_prefixed_forms_of_metre> ,
    <https://en.wikipedia.org/wiki/Decametre> ;
  ieso:hasSIUnitOfMeasure ieso:Metre ;
  ieso:conversionCoefficientToSIUnit "1.0e1"^^xsd:double ;
  ieso:conversionOffsetToSIUnit "0.0"^^xsd:double ;
  ieso:unitSymbol "dam"^^rdfs:Literal ;
  .
# !


###  https://www.gecad.isep.ipp.pt/ieso/v1.0.0/Decilitre
ieso:Decilitre
  rdf:type
    owl:NamedIndividual ,
    ieso:VolumeUnit ;
  rdfs:comment "The decilitre (British English spelling) or deciliter (American English spelling) (SI symbols dL and dl) is a metric unit of volume. It is equal to hundred cubic centimetres."@en ;
  rdfs:label "decilitre"@en ;
  rdfs:isDefinedBy <measure/v1.0.0/> ;
  rdfs:seeAlso
    <https://en.wikipedia.org/wiki/Litre#SI_prefixes_applied_to_the_litre> ,
    <https://en.wikipedia.org/wiki/Volume#Units> ;
  ieso:hasSIUnitOfMeasure ieso:CubicMetre ;
  ieso:conversionCoefficientToSIUnit "1.0e-4"^^xsd:double ;
  ieso:conversionOffsetToSIUnit "0.0"^^xsd:double ;
  ieso:unitSymbol "dl"^^rdfs:Literal ;
  .
# !


###  https://www.gecad.isep.ipp.pt/ieso/v1.0.0/Decimetre
ieso:Decimetre
  rdf:type
    owl:NamedIndividual ,
    ieso:LengthUnit ;
  rdfs:comment "The decimetre (SI symbol dm) or decimeter (American spelling) is a unit of length in the metric system, equal to one tenth of a metre (the International System of Units base unit of length), ten centimetres or 3.937 inches."@en ;
  rdfs:label "decimetre"@en ;
  rdfs:isDefinedBy <measure/v1.0.0/> ;
  rdfs:seeAlso
    <https://en.wikipedia.org/wiki/Conversion_of_units#Length> ,
    <https://en.wikipedia.org/wiki/Metre#SI_prefixed_forms_of_metre> ,
    <https://en.wikipedia.org/wiki/Decimetre> ;
  ieso:hasSIUnitOfMeasure ieso:Metre ;
  ieso:conversionCoefficientToSIUnit "1.0e-1"^^xsd:double ;
  ieso:conversionOffsetToSIUnit "0.0"^^xsd:double ;
  ieso:unitSymbol "dm"^^rdfs:Literal ;
  .
# !


###  https://www.gecad.isep.ipp.pt/ieso/v1.0.0/Degree
ieso:Degree
  rdf:type
    owl:NamedIndividual ,
    ieso:PlaneAngleUnit ;
  rdfs:comment "A degree (in full, a degree of arc, arc degree, or arcdegree), usually denoted by  (the degree symbol), is a measurement of a plane angle in which one full rotation is 360 degrees. It is not an SI unitthe SI unit of angular measure is the radianbut it is mentioned in the SI brochure as an accepted unit. Because a full rotation equals 2 radians, one degree is equivalent to /180 radians."@en ;
  rdfs:label "degree"@en ;
  rdfs:isDefinedBy <measure/v1.0.0/> ;
  rdfs:seeAlso
    <https://en.wikipedia.org/wiki/Conversion_of_units#Plane_angle> ,
    <https://en.wikipedia.org/wiki/Degree_(angle)> ;
  ieso:hasSIUnitOfMeasure ieso:Radian ;
  ieso:conversionCoefficientToSIUnit "1.74532925e-2"^^xsd:double ;
  ieso:conversionOffsetToSIUnit "0.0"^^xsd:double ;
  ieso:unitSymbol ""^^rdfs:Literal ;
  .
# !


###  https://www.gecad.isep.ipp.pt/ieso/v1.0.0/Euro
ieso:Euro
  rdf:type
    owl:NamedIndividual ,
    ieso:CurrencyUnit ;
  rdfs:comment "The euro (symbol: ; code: EUR) is the official currency of 19 of the 27 member states of the European Union. It is the second-largest and second-most traded currency in the foreign exchange market."@en ;
  rdfs:label "Euro"@en ;
  rdfs:isDefinedBy <measure/v1.0.0/> ;
  rdfs:seeAlso <https://en.wikipedia.org/wiki/Euro> ;
  ieso:unitCode "EUR"^^rdfs:Literal ;
  ieso:unitSymbol ""^^rdfs:Literal ;
  .
# !


###  https://www.gecad.isep.ipp.pt/ieso/v1.0.0/Fahrenheit
ieso:Fahrenheit
  rdf:type
    owl:NamedIndividual ,
    ieso:TemperatureUnit ;
  rdfs:comment "The Fahrenheit scale is a temperature scale based on one proposed in 1724 by the physicist Daniel Gabriel Fahrenheit (16861736). It uses the degree Fahrenheit (symbol: F) as the unit."@en ;
  rdfs:label "fahrenheit"@en ;
  rdfs:isDefinedBy <measure/v1.0.0/> ;
  rdfs:seeAlso
    <https://en.wikipedia.org/wiki/Conversion_of_units#Temperature> ,
    <https://en.wikipedia.org/wiki/Fahrenheit> ;
  ieso:hasSIUnitOfMeasure ieso:Kelvin ;
  ieso:conversionCoefficientToSIUnit "0.5555555555555556"^^xsd:double ;
  ieso:conversionOffsetToSIUnit "459.669607"^^xsd:double ;
  ieso:unitSymbol "F"^^rdfs:Literal ;
  .
# !


###  https://www.gecad.isep.ipp.pt/ieso/v1.0.0/Farad
ieso:Farad
  rdf:type
    owl:NamedIndividual ,
    ieso:CapacitanceUnit ;
  rdfs:comment "The farad (symbol: F) is the SI derived unit of electrical capacitance, the ability of a body to store an electrical charge."@en ;
  rdfs:label "farad"@en ;
  rdfs:isDefinedBy <measure/v1.0.0/> ;
  rdfs:seeAlso
    <https://en.wikipedia.org/wiki/Capacitance> ,
    <https://en.wikipedia.org/wiki/Farad> ;
  ieso:hasSIUnitOfMeasure ieso:Farad ;
  ieso:conversionCoefficientToSIUnit "1.0"^^xsd:double ;
  ieso:conversionOffsetToSIUnit "0.0"^^xsd:double ;
  ieso:unitSymbol "F"^^rdfs:Literal ;
  .
# !


### FIX HERE ###
###  https://www.gecad.isep.ipp.pt/ieso/v1.0.0/NanofaradPerKilometer
ieso:NanofaradPerKilometer
  rdf:type
    owl:NamedIndividual ,
    ieso:CapacitanceUnit ; # <|--subclassof-- ConductorCapacitance ????
  rdfs:comment "The nanofarad per kilometer (symbol: nF/km) is a submultiple of farad per kilimeter in the order of 10^-9 F/km."@en ;
  rdfs:label "farad per kilometer"@en ;
  rdfs:isDefinedBy <measure/v1.0.0/> ;
  #rdfs:seeAlso
  #  <https://en.wikipedia.org/wiki/Capacitance> ,
  #  <https://en.wikipedia.org/wiki/Farad> ;
  #ieso:hasSIUnitOfMeasure ieso:Farad ;
  #ieso:conversionCoefficientToSIUnit "1.0"^^xsd:double ;
  #ieso:conversionOffsetToSIUnit "0.0"^^xsd:double ;
  ieso:unitSymbol "nF/Km"^^rdfs:Literal ;
  .
# !


###  https://www.gecad.isep.ipp.pt/ieso/v1.0.0/Footcandle
ieso:Footcandle
  rdf:type
    owl:NamedIndividual ,
    ieso:IlluminanceUnit ;
  rdfs:comment "A foot-candle (sometimes foot candle; abbreviated fc, lm/ft^2, or sometimes ft-c) is a non-SI unit of illuminance or light intensity. The foot-candle is defined as one lumen per square foot."@en ;
  rdfs:label "footcandle"@en ;
  rdfs:isDefinedBy <measure/v1.0.0/> ;
  rdfs:seeAlso
    <https://en.wikipedia.org/wiki/Conversion_of_units#Illuminance> ,
    <https://en.wikipedia.org/wiki/Foot-candle> ;
  ieso:hasSIUnitOfMeasure ieso:Lux ;
  ieso:conversionCoefficientToSIUnit "10.763910417"^^xsd:double ;
  ieso:conversionOffsetToSIUnit "0.0"^^xsd:double ;
  ieso:unitSymbol "fc"^^rdfs:Literal ;
  .
# !


###  https://www.gecad.isep.ipp.pt/ieso/v1.0.0/Footlambert
ieso:Footlambert
  rdf:type
    owl:NamedIndividual ,
    ieso:LuminanceUnit ;
  rdfs:comment "A foot-lambert or footlambert (fL, sometimes fl or ft-L) is a unit of luminance in United States customary units and some other unit systems. A foot-lambert equals 1/ or 0.3183 candela per square foot, or 3.426 candela per square meter (the corresponding SI unit)."@en ;
  rdfs:label "footlambert"@en ;
  rdfs:isDefinedBy <measure/v1.0.0/> ;
  rdfs:seeAlso
    <https://en.wikipedia.org/wiki/Conversion_of_units#Luminance> ,
    <https://en.wikipedia.org/wiki/Foot-lambert> ;
  ieso:hasSIUnitOfMeasure ieso:CandelaPerSquareMetre ;
  ieso:conversionCoefficientToSIUnit "3.4262590996"^^xsd:double ;
  ieso:conversionOffsetToSIUnit "0.0"^^xsd:double ;
  ieso:unitSymbol "fL"^^rdfs:Literal ;
  .
# !


###  https://www.gecad.isep.ipp.pt/ieso/v1.0.0/FootPerSecond
ieso:FootPerSecond
  rdf:type
    owl:NamedIndividual ,
    ieso:VelocityUnit ;
  rdfs:comment "The foot per second (plural feet per second) is a unit of both speed (scalar) and velocity (vector quantity, which includes direction).It expresses the distance in feet (ft) traveled or displaced, divided by the time in seconds (s)."@en ; #
  rdfs:label "foot per second"@en ;
  rdfs:isDefinedBy <measure/v1.0.0/> ;
  rdfs:seeAlso
    <https://en.wikipedia.org/wiki/Conversion_of_units#Length> ,
    <https://en.wikipedia.org/wiki/Foot_per_second> ;
  ieso:hasSIUnitOfMeasure ieso:MetrePerSecond ;
  ieso:conversionCoefficientToSIUnit "0.3048"^^xsd:double ;
  ieso:conversionOffsetToSIUnit "0.0"^^xsd:double ;
  ieso:unitSymbol "ft/s"^^rdfs:Literal ;
  .
# !


###  https://www.gecad.isep.ipp.pt/ieso/v1.0.0/Gigahertz
ieso:Gigahertz
  rdf:type
    owl:NamedIndividual ,
    ieso:FrequencyUnit ;
  rdfs:comment "The gigahertz (symbol: GHz) is the derived unit of frequency in the International System of Units (SI) and is defined as one thousand megahertz."@en ;
  rdfs:label "gigahertz"@en ;
  rdfs:isDefinedBy <measure/v1.0.0/> ;
  rdfs:seeAlso <https://en.wikipedia.org/wiki/Hertz#SI_multiples> ;
  ieso:hasSIUnitOfMeasure ieso:Hertz ;
  ieso:conversionCoefficientToSIUnit "1.0e9"^^xsd:double ;
  ieso:conversionOffsetToSIUnit "0.0"^^xsd:double ;
  ieso:unitSymbol "GHz"^^rdfs:Literal ;
  .
# !


###  https://www.gecad.isep.ipp.pt/ieso/v1.0.0/Gigawatt
ieso:Gigawatt
  rdf:type
    owl:NamedIndividual ,
    ieso:PowerUnit ,
    ieso:ElectricPowerUnit ;
  rdfs:comment "The gigawatt (GW) is equal to one thousand megawatts. This unit is often used for large power plants or power grids."@en ;
  rdfs:label "gigawatt"@en ;
  rdfs:isDefinedBy <measure/v1.0.0/> ;
  rdfs:seeAlso
    <https://en.wikipedia.org/wiki/Conversion_of_units#Power_or_heat_flow_rate> ,
    <https://en.wikipedia.org/wiki/Watt#Gigawatt> ;
  ieso:hasSIUnitOfMeasure ieso:Watt ;
  ieso:conversionCoefficientToSIUnit "1.0e9"^^xsd:double ;
  ieso:conversionOffsetToSIUnit "0.0"^^xsd:double ;
  ieso:unitSymbol "GW"^^rdfs:Literal ;
  .
# !


###  https://www.gecad.isep.ipp.pt/ieso/v1.0.0/GramPerCubicMetre
ieso:GramPerCubicMetre
  rdf:type
    owl:NamedIndividual ,
    ieso:MassDensityUnit ;
  rdfs:comment "Gram per cubic metre is an SI derived unit of density, defined by mass in grams divided by volume in cubic metres."@en ;
  rdfs:label "gram per cubic metre"@en ;
  rdfs:isDefinedBy <measure/v1.0.0/> ;
  rdfs:seeAlso <https://en.wikipedia.org/wiki/Density#Common_units> ;
  ieso:hasSIUnitOfMeasure ieso:KilogramPerCubicMetre ;
  ieso:conversionCoefficientToSIUnit "1.0e-3"^^xsd:double ;
  ieso:conversionOffsetToSIUnit "0.0"^^xsd:double ;
  ieso:unitSymbol "g/m^3"^^rdfs:Literal ;
  .
# !


###  https://www.gecad.isep.ipp.pt/ieso/v1.0.0/Hectometre
ieso:Hectometre
  rdf:type
    owl:NamedIndividual ,
    ieso:LengthUnit ;
  rdfs:comment "The hectometre (International spelling as used by the International Bureau of Weights and Measures; SI symbol: hm) or hectometer (American spelling) is a unit of length in the metric system, equal to one hundred metres."@en ;
  rdfs:label "hectometre"@en ;
  rdfs:isDefinedBy <measure/v1.0.0/> ;
  rdfs:seeAlso
    <https://en.wikipedia.org/wiki/Conversion_of_units#Length> ,
    <https://en.wikipedia.org/wiki/Metre#SI_prefixed_forms_of_metre> ,
    <https://en.wikipedia.org/wiki/Hectometre> ;
  ieso:hasSIUnitOfMeasure ieso:Metre ;
  ieso:conversionCoefficientToSIUnit "1.0e2"^^xsd:double ;
  ieso:conversionOffsetToSIUnit "0.0"^^xsd:double ;
  ieso:unitSymbol "hm"^^rdfs:Literal ;
  .
# !


###  https://www.gecad.isep.ipp.pt/ieso/v1.0.0/Hectolitre
ieso:Hectolitre
  rdf:type
    owl:NamedIndividual ,
    ieso:VolumeUnit ;
  rdfs:comment "The hectolitre (British English spelling) or hectoliter (American English spelling) (SI symbols hL and hl) is a metric unit of volume. It is equal to hundred cubic decimetres."@en ;
  rdfs:label "hectolitre"@en ;
  rdfs:isDefinedBy <measure/v1.0.0/> ;
  rdfs:seeAlso <https://en.wikipedia.org/wiki/Litre#SI_prefixes_applied_to_the_litre> ;
  ieso:hasSIUnitOfMeasure ieso:CubicMetre ;
  ieso:conversionCoefficientToSIUnit "1.0e-1"^^xsd:double ;
  ieso:conversionOffsetToSIUnit "0.0"^^xsd:double ;
  ieso:unitSymbol "hl"^^rdfs:Literal ;
  .
# !


###  https://www.gecad.isep.ipp.pt/ieso/v1.0.0/Hertz
ieso:Hertz
  rdf:type
    owl:NamedIndividual ,
    ieso:FrequencyUnit ;
  rdfs:comment "The hertz (symbol: Hz) is the derived unit of frequency in the International System of Units (SI) and is defined as one cycle per second."@en ;
  rdfs:label "hertz"@en ;
  rdfs:isDefinedBy <measure/v1.0.0/> ;
  rdfs:seeAlso
    <https://en.wikipedia.org/wiki/Conversion_of_units#Frequency> ,
    <https://en.wikipedia.org/wiki/Hertz> ;
  ieso:hasSIUnitOfMeasure ieso:Hertz ;
  ieso:conversionCoefficientToSIUnit "1.0"^^xsd:double ;
  ieso:conversionOffsetToSIUnit "0.0"^^xsd:double ;
  ieso:unitSymbol "Hz"^^rdfs:Literal ;
  .
# !


###  https://www.gecad.isep.ipp.pt/ieso/v1.0.0/Hour
ieso:Hour
  rdf:type
    owl:NamedIndividual ,
    ieso:TimeUnit ;
  rdfs:comment "An hour (symbol: h; also abbreviated hr) is a unit of time conventionally reckoned as 124 of a day and scientifically reckoned as 35993601 seconds, depending on conditions. There are 60 minutes in an hour, and 24 hours in a day."@en ;
  rdfs:label "hour"@en ;
  rdfs:isDefinedBy <measure/v1.0.0/> ;
  rdfs:seeAlso
    <https://en.wikipedia.org/wiki/Conversion_of_units#Time> ,
    <https://en.wikipedia.org/wiki/Hour> ;
  ieso:hasSIUnitOfMeasure ieso:Second ;
  ieso:conversionCoefficientToSIUnit "3.6e3"^^xsd:double ;
  ieso:conversionOffsetToSIUnit "0.0"^^xsd:double ;
  ieso:unitSymbol "h"^^rdfs:Literal ;
  .
# !


###  https://www.gecad.isep.ipp.pt/ieso/v1.0.0/Joule
ieso:Joule
  rdf:type
    owl:NamedIndividual ,
    ieso:EnergyUnit ;
  rdfs:comment "The joule (symbol: J) is a derived unit of energy in the International System of Units. It is equal to the energy transferred to (or work done on) an object when a force of one newton acts on that object in the direction of the force's motion through a distance of one metre (1 newton metre or Nm). It is also the energy dissipated as heat when an electric current of one ampere passes through a resistance of one ohm for one second."@en ;
  rdfs:label "joule"@en ;
  rdfs:isDefinedBy <measure/v1.0.0/> ;
  rdfs:seeAlso
    <https://en.wikipedia.org/wiki/Conversion_of_units#Energy> ,
    <https://en.wikipedia.org/wiki/Energy#Units_of_measure> ,
    <https://en.wikipedia.org/wiki/Joule> ;
  ieso:hasSIUnitOfMeasure ieso:Joule ;
  ieso:conversionCoefficientToSIUnit "1.0"^^xsd:double ;
  ieso:conversionOffsetToSIUnit "0.0"^^xsd:double ;
  ieso:unitSymbol "J"^^rdfs:Literal ;
  .
# !


###  https://www.gecad.isep.ipp.pt/ieso/v1.0.0/Kelvin
ieso:Kelvin
  rdf:type
    owl:NamedIndividual ,
    ieso:TemperatureUnit ;
  rdfs:comment "The kelvin is the base unit of temperature in the International System of Units (SI), having the unit symbol K."@en ;
  rdfs:label "kelvin"@en ;
  rdfs:isDefinedBy <measure/v1.0.0/> ;
  rdfs:seeAlso
    <https://en.wikipedia.org/wiki/Conversion_of_units#Temperature> ,
    <https://en.wikipedia.org/wiki/Kelvin> ;
  ieso:hasSIUnitOfMeasure ieso:Kelvin ;
  ieso:conversionCoefficientToSIUnit "1.0"^^xsd:double ;
  ieso:conversionOffsetToSIUnit "0.0"^^xsd:double ;
  ieso:unitSymbol "K"^^rdfs:Literal ;
  .
# !


###  https://www.gecad.isep.ipp.pt/ieso/v1.0.0/KilogramPerCubicMetre
ieso:KilogramPerCubicMetre
  rdf:type
    owl:NamedIndividual ,
    ieso:MassDensityUnit ;
  rdfs:comment "Kilogram per cubic metre is an SI derived unit of density, defined by mass in kilograms divided by volume in cubic metres."@en ;
  rdfs:label "kilogram per cubic metre"@en ;
  rdfs:isDefinedBy <measure/v1.0.0/> ;
  rdfs:seeAlso <https://en.wikipedia.org/wiki/Density#Common_units> ;
  ieso:hasSIUnitOfMeasure ieso:KilogramPerCubicMetre ;
  ieso:conversionCoefficientToSIUnit "1.0"^^xsd:double ;
  ieso:conversionOffsetToSIUnit "0.0"^^xsd:double ;
  ieso:unitSymbol "Kg/m^3"^^rdfs:Literal ;
  .
# !


###  https://www.gecad.isep.ipp.pt/ieso/v1.0.0/KilogramPerMetre
ieso:KilogramPerMetre
  rdf:type
    owl:NamedIndividual ,
    ieso:LinearDensityUnit ;
  rdfs:comment "Kilogram Per Meter (kg/m) is a unit in the category of Linear mass density."@en ;
  rdfs:label "kilogram per metre"@en ;
  rdfs:isDefinedBy <measure/v1.0.0/> ;
  rdfs:seeAlso <https://en.wikipedia.org/wiki/Linear_density#Units> ;
  ieso:hasSIUnitOfMeasure ieso:KilogramPerMetre ;
  ieso:conversionCoefficientToSIUnit "1.0"^^xsd:double ;
  ieso:conversionOffsetToSIUnit "0.0"^^xsd:double ;
  ieso:unitSymbol "Kg/m"^^rdfs:Literal ;
  .
# !


###  https://www.gecad.isep.ipp.pt/ieso/v1.0.0/KilogramPerSquareMetre
ieso:KilogramPerSquareMetre
  rdf:type
    owl:NamedIndividual ,
    ieso:AreaDensityUnit ;
  rdfs:comment "Kilogram Per Square Meter (kg/m2) is a unit in the category of Surface density."@en ;
  rdfs:label "kilogram per square metre"@en ;
  rdfs:isDefinedBy <measure/v1.0.0/> ;
  rdfs:seeAlso <https://en.wikipedia.org/wiki/Area_density> ;
  ieso:hasSIUnitOfMeasure ieso:KilogramPerSquareMetre ;
  ieso:conversionCoefficientToSIUnit "1.0"^^xsd:double ;
  ieso:conversionOffsetToSIUnit "0.0"^^xsd:double ;
  ieso:unitSymbol "Kg/m^2"^^rdfs:Literal ;
  .
# !


###  https://www.gecad.isep.ipp.pt/ieso/v1.0.0/Kilohertz
ieso:Kilohertz
  rdf:type
    owl:NamedIndividual ,
    ieso:FrequencyUnit ;
  rdfs:comment "The kilohertz (symbol: kHz) is the derived unit of frequency in the International System of Units (SI) and is defined as one thousand cycles per second."@en ;
  rdfs:label "kilohertz"@en ;
  rdfs:isDefinedBy <measure/v1.0.0/> ;
  rdfs:seeAlso <https://en.wikipedia.org/wiki/Hertz#SI_multiples> ;
  ieso:hasSIUnitOfMeasure ieso:Hertz ;
  ieso:conversionCoefficientToSIUnit "1.0e3"^^xsd:double ;
  ieso:conversionOffsetToSIUnit "0.0"^^xsd:double ;
  ieso:unitSymbol "kHz"^^rdfs:Literal ;
  .
# !


###  https://www.gecad.isep.ipp.pt/ieso/v1.0.0/Kilolitre
ieso:Kilolitre
  rdf:type
    owl:NamedIndividual ,
    ieso:VolumeUnit ;
  rdfs:comment "The kilolitre (British English spelling) or kiloliter (American English spelling) (SI symbols kL and kl) is a metric unit of volume. It is equal to one cubic metre."@en ;
  rdfs:label "kilolitre"@en ;
  rdfs:isDefinedBy <measure/v1.0.0/> ;
  rdfs:seeAlso <https://en.wikipedia.org/wiki/Litre#SI_prefixes_applied_to_the_litre> ;
  ieso:hasSIUnitOfMeasure ieso:CubicMetre ;
  ieso:conversionCoefficientToSIUnit "1.0"^^xsd:double ;
  ieso:conversionOffsetToSIUnit "0.0"^^xsd:double ;
  ieso:unitSymbol "kl"^^rdfs:Literal ;
  .
# !


###  https://www.gecad.isep.ipp.pt/ieso/v1.0.0/Kilometre
ieso:Kilometre
  rdf:type
    owl:NamedIndividual ,
    ieso:LengthUnit ;
  rdfs:comment "The kilometre (SI symbol: km), spelt kilometer in American English, is a unit of length in the metric system, equal to one thousand metres. It is now the measurement unit used for expressing distances between geographical places on land in most of the world."@en ;
  rdfs:label "kilometre"@en ;
  rdfs:isDefinedBy <measure/v1.0.0/> ;
  rdfs:seeAlso
    <https://en.wikipedia.org/wiki/Conversion_of_units#Length> ,
    <https://en.wikipedia.org/wiki/Metre#SI_prefixed_forms_of_metre> ,
    <https://en.wikipedia.org/wiki/Kilometre> ;
  ieso:hasSIUnitOfMeasure ieso:Metre ;
  ieso:conversionCoefficientToSIUnit "1.0e3"^^xsd:double ;
  ieso:conversionOffsetToSIUnit "0.0"^^xsd:double ;
  ieso:unitSymbol "km"^^rdfs:Literal ;
  .
# !


###  https://www.gecad.isep.ipp.pt/ieso/v1.0.0/KilometresPerHour
ieso:KilometresPerHour
  rdf:type
    owl:NamedIndividual ,
    ieso:VelocityUnit ;
  rdfs:comment "The kilometre per hour (SI symbol: km/h; abbreviations: kph, kmph, km/hr) is a unit of speed, expressing the number of kilometres travelled in one hour."@en ; #
  rdfs:label "kilometres per hour"@en ;
  rdfs:isDefinedBy <measure/v1.0.0/> ;
  rdfs:seeAlso
    <https://en.wikipedia.org/wiki/Conversion_of_units#Length> ,
    <https://en.wikipedia.org/wiki/Kilometres_per_hour> ;
  ieso:hasSIUnitOfMeasure ieso:MetrePerSecond ;
  ieso:conversionCoefficientToSIUnit "0.2777777777777778"^^xsd:double ;
  ieso:conversionOffsetToSIUnit "0.0"^^xsd:double ;
  ieso:unitSymbol "km/h"^^rdfs:Literal ;
  .
# !


###  https://www.gecad.isep.ipp.pt/ieso/v1.0.0/Kilovolt
ieso:Kilovolt
  rdf:type
    owl:NamedIndividual ,
    ieso:VoltageUnit ;
  rdfs:comment "The kilovolt (kW) is equal to one thousand volts."@en ;
  rdfs:label "kilovolt"@en ;
  rdfs:isDefinedBy <measure/v1.0.0/> ;
  rdfs:seeAlso
    <https://en.wiktionary.org/wiki/kilovolt> ;
  ieso:hasSIUnitOfMeasure ieso:Volt ;
  ieso:conversionCoefficientToSIUnit "1.0e3"^^xsd:double ;
  ieso:conversionOffsetToSIUnit "0.0"^^xsd:double ;
  ieso:unitSymbol "kV"^^rdfs:Literal ;
  .
# !


###  https://www.gecad.isep.ipp.pt/ieso/v1.0.0/Kilowatt
ieso:Kilowatt
  rdf:type
    owl:NamedIndividual ,
    ieso:PowerUnit ,
    ieso:ElectricPowerUnit ;
  rdfs:comment "The kilowatt (kW) is equal to one thousand watts."@en ;
  rdfs:label "kilowatt"@en ;
  rdfs:isDefinedBy <measure/v1.0.0/> ;
  rdfs:seeAlso
    <https://en.wikipedia.org/wiki/Conversion_of_units#Power_or_heat_flow_rate> ,
    <https://en.wikipedia.org/wiki/Watt#Kilowatt> ;
  ieso:hasSIUnitOfMeasure ieso:Watt ;
  ieso:conversionCoefficientToSIUnit "1.0e3"^^xsd:double ;
  ieso:conversionOffsetToSIUnit "0.0"^^xsd:double ;
  ieso:unitSymbol "kW"^^rdfs:Literal ;
  .
# !


###  https://www.gecad.isep.ipp.pt/ieso/v1.0.0/KilowattHour
ieso:KilowattHour
  rdf:type
    owl:NamedIndividual ,
    ieso:EnergyUnit ,
    ieso:ElectricEnergyUnit ;
  rdfs:comment "The kilowatt-hour (SI symbol: kWh or kW h; commonly written as kWh) is a unit of energy equal to 3600 kilojoules (3.6 megajoules). The kilowatt-hour is commonly used as a billing unit for energy delivered to consumers by electric utilities."@en ;
  rdfs:label "kilowatt hour"@en ;
  rdfs:isDefinedBy <measure/v1.0.0/> ;
  rdfs:seeAlso
    <https://en.wikipedia.org/wiki/Conversion_of_units#Energy> ,
    <https://en.wikipedia.org/wiki/Kilowatt-hour>  ;
  ieso:hasSIUnitOfMeasure ieso:Joule ;
  ieso:conversionCoefficientToSIUnit "3.6e6"^^xsd:double ;
  ieso:conversionOffsetToSIUnit "0.0"^^xsd:double ;
  ieso:unitSymbol "kWh"^^rdfs:Literal ;
  .
# !


###  https://www.gecad.isep.ipp.pt/ieso/v1.0.0/Knot
ieso:Knot
  rdf:type
    owl:NamedIndividual ,
    ieso:VelocityUnit ;
  rdfs:comment "The knot is a unit of speed equal to one nautical mile per hour, exactly 1.852 km/h (approximately 1.15078 mph or 0.514 m/s)."@en ; #
  rdfs:label "knot"@en ;
  rdfs:isDefinedBy <measure/v1.0.0/> ;
  rdfs:seeAlso
    <https://en.wikipedia.org/wiki/Conversion_of_units#Length> ,
    <https://en.wikipedia.org/wiki/Knot_(unit)> ;
  ieso:hasSIUnitOfMeasure ieso:MetrePerSecond ;
  ieso:conversionCoefficientToSIUnit "0.5144444444444445"^^xsd:double ;
  ieso:conversionOffsetToSIUnit "0.0"^^xsd:double ;
  ieso:unitSymbol "kn"^^rdfs:Literal ;
  .
# !


###  https://www.gecad.isep.ipp.pt/ieso/v1.0.0/Lambert
ieso:Lambert
  rdf:type
    owl:NamedIndividual ,
    ieso:LuminanceUnit ;
  rdfs:comment "The lambert (symbol L, la or Lb) is a non-SI metric unit of luminance named for Johann Heinrich Lambert (17281777), a Swiss mathematician, physicist and astronomer. A related unit of luminance, the foot-lambert, is used in the lighting, cinema and flight simulation industries."@en ;
  rdfs:label "lambert"@en ;
  rdfs:isDefinedBy <measure/v1.0.0/> ;
  rdfs:seeAlso
    <https://en.wikipedia.org/wiki/Conversion_of_units#Luminance> ,
    <https://en.wikipedia.org/wiki/Lambert_(unit)> ;
  ieso:hasSIUnitOfMeasure ieso:CandelaPerSquareMetre ;
  ieso:conversionCoefficientToSIUnit "3.1830988618e3"^^xsd:double ;
  ieso:conversionOffsetToSIUnit "0.0"^^xsd:double ;
  ieso:unitSymbol "L"^^rdfs:Literal ;
  .
# !


###  https://www.gecad.isep.ipp.pt/ieso/v1.0.0/Litre
ieso:Litre
  rdf:type
    owl:NamedIndividual ,
    ieso:VolumeUnit ;
  rdfs:comment "The litre (British English spelling) or liter (American English spelling) (SI symbols L and l) is a metric unit of volume. It is equal to 1 cubic decimetre (dm^3), 1000 cubic centimetres (cm^3) or 0.001 cubic metre (m^3). A cubic decimetre (or litre) occupies a volume of 10 cm  10 cm  10 cm and is thus equal to one-thousandth of a cubic metre."@en ;
  rdfs:label "litre"@en ;
  rdfs:isDefinedBy <measure/v1.0.0/> ;
  rdfs:seeAlso
    <https://en.wikipedia.org/wiki/Conversion_of_units#Volume> ,
    <https://en.wikipedia.org/wiki/Litre> ,
    <https://en.wikipedia.org/wiki/Volume#Units> ;
  ieso:hasSIUnitOfMeasure ieso:CubicMetre ;
  ieso:conversionCoefficientToSIUnit "1.0e-3"^^xsd:double ;
  ieso:conversionOffsetToSIUnit "0.0"^^xsd:double ;
  ieso:unitSymbol "l"^^rdfs:Literal ;
  .
# !


###  https://www.gecad.isep.ipp.pt/ieso/v1.0.0/Lumen
ieso:Lumen
  rdf:type
    owl:NamedIndividual ,
    ieso:LuminousFluxUnit ;
  rdfs:comment "The lumen (symbol: lm) is the SI derived unit of luminous flux, a measure of the total quantity of visible light emitted by a source per unit of time. Luminous flux differs from power (radiant flux) in that radiant flux includes all electromagnetic waves emitted, while luminous flux is weighted according to a model (a 'luminosity function') of the human eye's sensitivity to various wavelengths. Lumens are related to lux in that one lux is one lumen per square metre."@en ;
  rdfs:label "lumen"@en ;
  rdfs:isDefinedBy <measure/v1.0.0/> ;
  rdfs:seeAlso
    <https://en.wikipedia.org/wiki/Conversion_of_units#Luminous_flux> ,
    <https://en.wikipedia.org/wiki/Lumen_(unit)> ;
  ieso:hasSIUnitOfMeasure ieso:Lumen ;
  ieso:conversionCoefficientToSIUnit "1.0"^^xsd:double ;
  ieso:conversionOffsetToSIUnit "0.0"^^xsd:double ;
  ieso:unitSymbol "lm"^^rdfs:Literal ;
  .
# !


###  https://www.gecad.isep.ipp.pt/ieso/v1.0.0/LumenPerSquareInch
ieso:LumenPerSquareInch
  rdf:type
    owl:NamedIndividual ,
    ieso:IlluminanceUnit ;
  rdfs:comment "A derived unit from the SI lux unit."@en ;
  rdfs:label "lumen per square inch"@en ;
  rdfs:isDefinedBy <measure/v1.0.0/> ;
  rdfs:seeAlso <https://en.wikipedia.org/wiki/Conversion_of_units#Illuminance> ;
  ieso:hasSIUnitOfMeasure ieso:Lux ;
  ieso:conversionCoefficientToSIUnit "1.5500031e3"^^xsd:double ;
  ieso:conversionOffsetToSIUnit "0.0"^^xsd:double ;
  ieso:unitSymbol "lm/in^2"^^rdfs:Literal ;
  .
# !


###  https://www.gecad.isep.ipp.pt/ieso/v1.0.0/Lux
ieso:Lux
  rdf:type
    owl:NamedIndividual ,
    ieso:IlluminanceUnit ;
  rdfs:comment "The lux (symbol: lx) is the SI derived unit of illuminance, measuring luminous flux per unit area. It is equal to one lumen per square metre (lm/m^2). In photometry, this is used as a measure of the intensity, as perceived by the human eye, of light that hits or passes through a surface."@en ;
  rdfs:label "lux"@en ;
  rdfs:isDefinedBy <measure/v1.0.0/> ;
  rdfs:seeAlso
    <https://en.wikipedia.org/wiki/Conversion_of_units#Illuminance> ,
    <https://en.wikipedia.org/wiki/Lux> ,
    <https://en.wikipedia.org/wiki/Lux#SI_photometry_units> ;
  ieso:hasSIUnitOfMeasure ieso:Lux ;
  ieso:conversionCoefficientToSIUnit "1.0"^^xsd:double ;
  ieso:conversionOffsetToSIUnit "0.0"^^xsd:double ;
  ieso:unitSymbol "lx"^^rdfs:Literal ;
  .
# !


###  https://www.gecad.isep.ipp.pt/ieso/v1.0.0/Megahertz
ieso:Megahertz
  rdf:type
    owl:NamedIndividual ,
    ieso:FrequencyUnit ;
  rdfs:comment "The megahertz (symbol: MHz) is the derived unit of frequency in the International System of Units (SI) and is defined as one million cycles per second."@en ;
  rdfs:label "megahertz"@en ;
  rdfs:isDefinedBy <measure/v1.0.0/> ;
  rdfs:seeAlso <https://en.wikipedia.org/wiki/Hertz#SI_multiples> ;
  ieso:hasSIUnitOfMeasure ieso:Hertz ;
  ieso:conversionCoefficientToSIUnit "1.0e6"^^xsd:double ;
  ieso:conversionOffsetToSIUnit "0.0"^^xsd:double ;
  ieso:unitSymbol "MHz"^^rdfs:Literal ;
  .
# !


###  https://www.gecad.isep.ipp.pt/ieso/v1.0.0/Megawatt
ieso:Megawatt
  rdf:type
    owl:NamedIndividual ,
    ieso:PowerUnit ,
    ieso:ElectricPowerUnit ;
  rdfs:comment "The megawatt (MW) is equal to one million watts."@en ;
  rdfs:label "megawatt"@en ;
  rdfs:isDefinedBy <measure/v1.0.0/> ;
  rdfs:seeAlso
    <https://en.wikipedia.org/wiki/Conversion_of_units#Power_or_heat_flow_rate> ,
    <https://en.wikipedia.org/wiki/Watt#Megawatt> ;
  ieso:hasSIUnitOfMeasure ieso:Watt ;
  ieso:conversionCoefficientToSIUnit "1.0e6"^^xsd:double ;
  ieso:conversionOffsetToSIUnit "0.0"^^xsd:double ;
  ieso:unitSymbol "MW"^^rdfs:Literal ;
  .
# !


###  https://www.gecad.isep.ipp.pt/ieso/v1.0.0/MegawattHour
ieso:MegawattHour
  rdf:type
    owl:NamedIndividual ,
    ieso:EnergyUnit ,
    ieso:ElectricEnergyUnit ;
  rdfs:comment "The megawatt-hour (SI symbol: MWh or MW h; commonly written as MWh) is a unit of energy equal to 3600 megajoules."@en ;
  rdfs:label "megawatt hour"@en ;
  rdfs:isDefinedBy <measure/v1.0.0/> ;
  rdfs:seeAlso
    <https://en.wikipedia.org/wiki/Conversion_of_units#Energy> ,
    <https://en.wikipedia.org/wiki/Kilowatt-hour#Multiples>  ;
  ieso:hasSIUnitOfMeasure ieso:Joule ;
  ieso:conversionCoefficientToSIUnit "3.6e9"^^xsd:double ;
  ieso:conversionOffsetToSIUnit "0.0"^^xsd:double ;
  ieso:unitSymbol "MWh"^^rdfs:Literal ;
  .
# !


###  https://www.gecad.isep.ipp.pt/ieso/v1.0.0/Metre
ieso:Metre
  rdf:type
    owl:NamedIndividual ,
    ieso:LengthUnit ;
  rdfs:comment "The metre (Commonwealth spelling) or meter (American spelling) is the base unit of length in the International System of Units (SI). The SI unit symbol is m."@en ;
  rdfs:label "metre"@en ;
  rdfs:isDefinedBy <measure/v1.0.0/> ;
  rdfs:seeAlso
    <https://en.wikipedia.org/wiki/Conversion_of_units#Length> ,
    <https://en.wikipedia.org/wiki/Metre> ;
  ieso:hasSIUnitOfMeasure ieso:Metre ;
  ieso:conversionCoefficientToSIUnit "1.0"^^xsd:double ;
  ieso:conversionOffsetToSIUnit "0.0"^^xsd:double ;
  ieso:unitSymbol "m"^^rdfs:Literal ;
  .
# !


###  https://www.gecad.isep.ipp.pt/ieso/v1.0.0/MetrePerSecond
ieso:MetrePerSecond
  rdf:type
    owl:NamedIndividual ,
    ieso:VelocityUnit ;
  rdfs:comment "The metre per second is an SI derived unit of both speed (scalar quantity) and velocity (vector quantity (which have direction and magnitude)), equal to the speed of a body covering a distance of one metre in a time of one second."@en ; #
  rdfs:label "metre per second"@en ;
  rdfs:isDefinedBy <measure/v1.0.0/> ;
  rdfs:seeAlso
    <https://en.wikipedia.org/wiki/Conversion_of_units#Length> ,
    <https://en.wikipedia.org/wiki/Metre_per_second> ;
  ieso:hasSIUnitOfMeasure ieso:MetrePerSecond ;
  ieso:conversionCoefficientToSIUnit "1.0"^^xsd:double ;
  ieso:conversionOffsetToSIUnit "0.0"^^xsd:double ;
  ieso:unitSymbol "m/s"^^rdfs:Literal ;
  .
# !


###  https://www.gecad.isep.ipp.pt/ieso/v1.0.0/MicrogramPerCubicMetre
ieso:MicrogramPerCubicMetre
  rdf:type
    owl:NamedIndividual ,
    ieso:MassDensityUnit ;
  rdfs:comment "Microgram per cubic metre is an SI derived unit of density, defined by mass in micrograms divided by volume in cubic metres."@en ;
  rdfs:label "microgram per cubic metre"@en ;
  rdfs:isDefinedBy <measure/v1.0.0/> ;
  rdfs:seeAlso <https://en.wikipedia.org/wiki/Density#Common_units> ;
  ieso:hasSIUnitOfMeasure ieso:KilogramPerCubicMetre ;
  ieso:conversionCoefficientToSIUnit "1.0e-9"^^xsd:double ;
  ieso:conversionOffsetToSIUnit "0.0"^^xsd:double ;
  ieso:unitSymbol "g/m^3"^^rdfs:Literal ;
  .
# !


###  https://www.gecad.isep.ipp.pt/ieso/v1.0.0/MilesPerHour
ieso:MilesPerHour
  rdf:type
    owl:NamedIndividual ,
    ieso:VelocityUnit ;
  rdfs:comment "Miles per hour (mph or mi/h) is a British imperial and United States customary unit of speed expressing the number of miles travelled in one hour."@en ; #
  rdfs:label "miles per hour"@en ;
  rdfs:isDefinedBy <measure/v1.0.0/> ;
  rdfs:seeAlso
    <https://en.wikipedia.org/wiki/Conversion_of_units#Length> ,
    <https://en.wikipedia.org/wiki/Miles_per_hour> ;
  ieso:hasSIUnitOfMeasure ieso:MetrePerSecond ;
  ieso:conversionCoefficientToSIUnit "0.44704"^^xsd:double ;
  ieso:conversionOffsetToSIUnit "0.0"^^xsd:double ;
  ieso:unitSymbol "mph"^^rdfs:Literal ;
  .
# !


###  https://www.gecad.isep.ipp.pt/ieso/v1.0.0/Milliampere
ieso:Milliampere
  rdf:type
    owl:NamedIndividual ,
    ieso:ElectricCurrentUnit ;
  rdfs:comment "The milliampere is the SI derived unit of electric current with symbol mA."@en ;
  rdfs:label "milliampere"@en ;
  rdfs:isDefinedBy <measure/v1.0.0/> ;
  rdfs:seeAlso
    <https://en.wikipedia.org/wiki/Conversion_of_units#Electric_current> ,
    <https://en.wikipedia.org/wiki/Milliampere> ;
  ieso:hasSIUnitOfMeasure ieso:Ampere ;
  ieso:conversionCoefficientToSIUnit "1.0e-3"^^xsd:double ;
  ieso:conversionOffsetToSIUnit "0.0"^^xsd:double ;
  ieso:unitSymbol "mA"^^rdfs:Literal ;
  .
# !


###  https://www.gecad.isep.ipp.pt/ieso/v1.0.0/MilliampereHour
ieso:MilliampereHour
  rdf:type
    owl:NamedIndividual ,
    ieso:ElectricChargeUnit ;
  rdfs:comment "The commonly seen milliampere hour (symbol: mAh, mA h, or unofficially mAh) is one-thousandth of an ampere hour (3.6 coulombs)."@en ;
  rdfs:label "milliampere hour"@en ;
  rdfs:isDefinedBy <measure/v1.0.0/> ;
  rdfs:seeAlso
    <https://en.wikipedia.org/wiki/Conversion_of_units#Electric_charge> ,
    <https://en.wikipedia.org/wiki/Milliampere-hour> ;
  ieso:hasSIUnitOfMeasure ieso:Coulomb ;
  ieso:conversionCoefficientToSIUnit "3.6"^^xsd:double ;
  ieso:conversionOffsetToSIUnit "0.0"^^xsd:double ;
  ieso:unitSymbol "mAh"^^rdfs:Literal ;
  .
# !


###  https://www.gecad.isep.ipp.pt/ieso/v1.0.0/Millilitre
ieso:Millilitre
  rdf:type
    owl:NamedIndividual ,
    ieso:VolumeUnit ;
  rdfs:comment "The millilitre (British English spelling) or milliliter (American English spelling) (SI symbols mL and ml) is a metric unit of volume. It is equal to 1 cubic centimetre (cm^3)"@en ;
  rdfs:label "millilitre"@en ;
  rdfs:isDefinedBy <measure/v1.0.0/> ;
  rdfs:seeAlso
    <https://en.wikipedia.org/wiki/Litre#SI_prefixes_applied_to_the_litre> ,
    <https://en.wikipedia.org/wiki/Volume#Units> ;
  ieso:hasSIUnitOfMeasure ieso:CubicMetre ;
  ieso:conversionCoefficientToSIUnit "1.0e-6"^^xsd:double ;
  ieso:conversionOffsetToSIUnit "0.0"^^xsd:double ;
  ieso:unitSymbol "ml"^^rdfs:Literal ;
  .
# !


###  https://www.gecad.isep.ipp.pt/ieso/v1.0.0/Millimetre
ieso:Millimetre
  rdf:type
    owl:NamedIndividual ,
    ieso:LengthUnit ;
  rdfs:comment "The millimetre (international spelling; SI unit symbol mm) or millimeter (American spelling) is a unit of length in the metric system, equal to one thousandth of a metre, which is the SI base unit of length. Therefore, there are one thousand millimetres in a metre. There are ten millimetres in a centimetre."@en ;
  rdfs:label "millimetre"@en ;
  rdfs:isDefinedBy <measure/v1.0.0/> ;
  rdfs:seeAlso
    <https://en.wikipedia.org/wiki/Conversion_of_units#Length> ,
    <https://en.wikipedia.org/wiki/Metre#SI_prefixed_forms_of_metre> ,
    <https://en.wikipedia.org/wiki/Millimetre> ;
  ieso:hasSIUnitOfMeasure ieso:Metre ;
  ieso:conversionCoefficientToSIUnit "1.0e-3"^^xsd:double ;
  ieso:conversionOffsetToSIUnit "0.0"^^xsd:double ;
  ieso:unitSymbol "mm"^^rdfs:Literal ;
  .
# !


###  https://www.gecad.isep.ipp.pt/ieso/v1.0.0/Millisecond
ieso:Millisecond
  rdf:type
    owl:NamedIndividual ,
    ieso:TimeUnit ;
  rdfs:comment "A millisecond (from milli- and second; symbol: ms) is a thousandth (0.001 or 10^3 or 1/1000) of a second."@en ;
  rdfs:label "millisecond"@en ;
  rdfs:isDefinedBy <measure/v1.0.0/> ;
  rdfs:seeAlso
    <https://en.wikipedia.org/wiki/Conversion_of_units#Time> ,
    <https://en.wikipedia.org/wiki/Millisecond> ;
  ieso:hasSIUnitOfMeasure ieso:Second ;
  ieso:conversionCoefficientToSIUnit "1.0e-3"^^xsd:double ;
  ieso:conversionOffsetToSIUnit "0.0"^^xsd:double ;
  ieso:unitSymbol "ms"^^rdfs:Literal ;
  .
# !


###  https://www.gecad.isep.ipp.pt/ieso/v1.0.0/Minute
ieso:Minute
  rdf:type
    owl:NamedIndividual ,
    ieso:TimeUnit ;
  rdfs:comment "The minute is a unit of time usually equal to 1/60 (the first sexagesimal fraction) of an hour, or 60 seconds. In the UTC time standard, a minute on rare occasions has 61 seconds, a consequence of leap seconds (there is a provision to insert a negative leap second, which would result in a 59-second minute, but this has never happened in more than 40 years under this system). Although not an SI unit, the minute is accepted for use with SI units. The SI symbol for minute or minutes is min (without a dot)."@en ;
  rdfs:label "minute"@en ;
  rdfs:isDefinedBy <measure/v1.0.0/> ;
  rdfs:seeAlso
    <https://en.wikipedia.org/wiki/Conversion_of_units#Time> ,
    <https://en.wikipedia.org/wiki/Minute> ;
  ieso:hasSIUnitOfMeasure ieso:Second ;
  ieso:conversionCoefficientToSIUnit "60.0"^^xsd:double ;
  ieso:conversionOffsetToSIUnit "0.0"^^xsd:double ;
  ieso:unitSymbol "min"^^rdfs:Literal ;
  .
# !


###  https://www.gecad.isep.ipp.pt/ieso/v1.0.0/Month
ieso:Month
  rdf:type
    owl:NamedIndividual ,
    ieso:TimeUnit ;
  rdfs:comment "A month is a unit of time, used with calendars, which is approximately as long as a natural period related to the motion of the Moon; month and Moon are cognates. The traditional concept arose with the cycle of Moon phases; such months (lunations) are synodic months and last approximately 29.530589 days (average)."@en ;
  rdfs:label "month (synodic)"@en ;
  rdfs:isDefinedBy <measure/v1.0.0/> ;
  rdfs:seeAlso
    <https://en.wikipedia.org/wiki/Conversion_of_units#Time> ,
    <https://en.wikipedia.org/wiki/Month> ;
  ieso:hasSIUnitOfMeasure ieso:Second ;
  ieso:conversionCoefficientToSIUnit "2.551442976e6"^^xsd:double ;
  ieso:conversionOffsetToSIUnit "0.0"^^xsd:double ;
  ieso:unitSymbol "mo"^^rdfs:Literal ;
  .
# !


###  https://www.gecad.isep.ipp.pt/ieso/v1.0.0/Ohm
ieso:Ohm
  rdf:type
    owl:NamedIndividual ,
    ieso:ElectricalImpedanceUnit ,
    ieso:ElectricalReactanceUnit ,
    ieso:ElectricalResistanceUnit ;
  rdfs:comment "The ohm (symbol: ) is the SI derived unit of electrical resistance, reactance, and impedance."@en ;
  rdfs:label "ohm"@en ;
  rdfs:isDefinedBy <measure/v1.0.0/> ;
  rdfs:seeAlso
    <https://en.wikipedia.org/wiki/Conversion_of_units#Electrical_resistance> ,
    <https://en.wikipedia.org/wiki/Ohm> ;
  ieso:hasSIUnitOfMeasure ieso:Ohm ;
  ieso:conversionCoefficientToSIUnit "1.0"^^xsd:double ;
  ieso:conversionOffsetToSIUnit "0.0"^^xsd:double ;
  ieso:unitSymbol ""^^rdfs:Literal ;
  .
# !


### FIX HERE ###
###  https://www.gecad.isep.ipp.pt/ieso/v1.0.0/OhmPerKilometer
ieso:OhmPerKilometer
  rdf:type
    owl:NamedIndividual ,
    ieso:ElectricalImpedanceUnit ,
    ieso:ElectricalReactanceUnit ,
    ieso:ElectricalResistanceUnit ; # <|--subclassof-- ConductorResistance ????
  rdfs:comment "The ohm per kilometer (symbol: /km) measures the rresistance, reactance, and impedance of a conducture ??? ."@en ;
  rdfs:label "ohm per kilometer"@en ;
  rdfs:isDefinedBy <measure/v1.0.0/> ;
  #rdfs:seeAlso
  #  <https://en.wikipedia.org/wiki/Conversion_of_units#Electrical_resistance> ,
  #  <https://en.wikipedia.org/wiki/Ohm> ;
  #ieso:hasSIUnitOfMeasure ieso:Ohm ;
  #ieso:conversionCoefficientToSIUnit "1.0"^^xsd:double ;
  #ieso:conversionOffsetToSIUnit "0.0"^^xsd:double ;
  ieso:unitSymbol "/Km"^^rdfs:Literal ;
  .
# !


###  https://www.gecad.isep.ipp.pt/ieso/v1.0.0/PartsPerBillion
ieso:PartsPerBillion
  rdf:type
    owl:NamedIndividual ,
    ieso:PartsPerNotationUnit ;
  rdfs:comment "One part per billion (ppb) denotes one part per 1,000,000,000 (10^9) parts, and a value of 10^9. This is equivalent to about three seconds out of a century."@en ;
  rdfs:label "parts-per-billion"@en ;
  rdfs:isDefinedBy <measure/v1.0.0/> ;
  rdfs:seeAlso <https://en.wikipedia.org/wiki/Parts-per_notation#Parts-per_expressions> ;
  ieso:unitSymbol "ppb"^^rdfs:Literal ;
  .
# !


###  https://www.gecad.isep.ipp.pt/ieso/v1.0.0/PartsPerHundred
ieso:PartsPerHundred
  rdf:type
    owl:NamedIndividual ,
    ieso:PartsPerNotationUnit ;
  rdfs:comment "One part per hundred is generally represented by the percent sign (%) and denotes one part per 100 (10^2) parts, and a value of 10^2. This is equivalent to about fifteen minutes out of one day."@en ;
  rdfs:label "parts-per-hundred"@en ;
  rdfs:isDefinedBy <measure/v1.0.0/> ;
  rdfs:seeAlso <https://en.wikipedia.org/wiki/Parts-per_notation#Parts-per_expressions> ;
  ieso:unitSymbol "%"^^rdfs:Literal ;
  .
# !


###  https://www.gecad.isep.ipp.pt/ieso/v1.0.0/PartsPerMillion
ieso:PartsPerMillion
  rdf:type
    owl:NamedIndividual ,
    ieso:PartsPerNotationUnit ;
  rdfs:comment "One part per million (ppm) denotes one part per 1,000,000 (10^6) parts, and a value of 10^6. It is equivalent to about 32 seconds out of a year or 1 mm of error per km of distance traversed."@en ;
  rdfs:label "parts-per-million"@en ;
  rdfs:isDefinedBy <measure/v1.0.0/> ;
  rdfs:seeAlso <https://en.wikipedia.org/wiki/Parts-per_notation#Parts-per_expressions> ;
  ieso:unitSymbol "ppm"^^rdfs:Literal ;
  .
# !


###  https://www.gecad.isep.ipp.pt/ieso/v1.0.0/PartsPerQuadrillion
ieso:PartsPerQuadrillion
  rdf:type
    owl:NamedIndividual ,
    ieso:PartsPerNotationUnit ;
  rdfs:comment "One part per quadrillion (ppq) denotes one part per 1,000,000,000,000,000 (10^15) parts, and a value of 10^15. This is equivalent to about two and a half minutes out of the age of the Earth (4.5 billion years). Although relatively uncommon in analytical chemistry, measurements at the ppq level are sometimes performed."@en ;
  rdfs:label "parts-per-quadrillion"@en ;
  rdfs:isDefinedBy <measure/v1.0.0/> ;
  rdfs:seeAlso <https://en.wikipedia.org/wiki/Parts-per_notation#Parts-per_expressions> ;
  ieso:unitSymbol "ppq"^^rdfs:Literal ;
  .
# !


###  https://www.gecad.isep.ipp.pt/ieso/v1.0.0/PartsPerThousand
ieso:PartsPerThousand
  rdf:type
    owl:NamedIndividual ,
    ieso:PartsPerNotationUnit ;
  rdfs:comment "One part per thousand should generally be spelled out in full and not as 'ppt' (which is usually understood to represent 'parts per trillion'). It may also be denoted by the permille sign (). Note however, that specific disciplines such as oceanography, as well as educational exercises, do use the 'ppt' abbreviation. One part per thousand denotes one part per 1,000 (10^3) parts, and a value of 10^3. This is equivalent to about one and a half minutes out of one day."@en ;
  rdfs:label "parts-per-thousand"@en ;
  rdfs:isDefinedBy <measure/v1.0.0/> ;
  rdfs:seeAlso <https://en.wikipedia.org/wiki/Parts-per_notation#Parts-per_expressions> ;
  ieso:unitSymbol ""^^rdfs:Literal ;
  .
# !


###  https://www.gecad.isep.ipp.pt/ieso/v1.0.0/PartsPerTrillion
ieso:PartsPerTrillion
  rdf:type
    owl:NamedIndividual ,
    ieso:PartsPerNotationUnit ;
  rdfs:comment "One part per trillion (ppt) denotes one part per 1,000,000,000,000 (10^12) parts, and a value of 10^12. This is equivalent to about thirty seconds out of every million years."@en ;
  rdfs:label "parts-per-trillion"@en ;
  rdfs:isDefinedBy <measure/v1.0.0/> ;
  rdfs:seeAlso <https://en.wikipedia.org/wiki/Parts-per_notation#Parts-per_expressions> ;
  ieso:unitSymbol "ppt"^^rdfs:Literal ;
  .
# !


###  https://www.gecad.isep.ipp.pt/ieso/v1.0.0/Percent
ieso:Percent
  rdf:type
    owl:NamedIndividual ,
    ieso:PercentageUnit ;
  rdfs:comment "The term 'percent' is derived from the Latin per centum, meaning 'hundred' or 'by the hundred'."@en ;
  rdfs:label "percent"@en ;
  rdfs:isDefinedBy <measure/v1.0.0/> ;
  rdfs:seeAlso <https://en.wikipedia.org/wiki/Percentage#Percent_sign> ;
  ieso:unitSymbol "%"^^rdfs:Literal ;
  .
# !


###  https://www.gecad.isep.ipp.pt/ieso/v1.0.0/PercentObscurationPerFoot
ieso:PercentObscurationPerFoot
  rdf:type
    owl:NamedIndividual ,
    ieso:ObscurationUnit ;
  rdfs:comment "Percent obscuration per foot - Obscuration is any atmospheric phenomenon, except clouds, that restricts vertical visibility (e.g., dust, rain, snow, etc.). Percent obscuration per foot is the unit to measure the amount of Obscuration per foot. This unit is usually used in smoke detectors."@en ;
  rdfs:label "percent obscuration per foot"@en ;
  rdfs:isDefinedBy <measure/v1.0.0/> ;
  rdfs:seeAlso <http://automationwiki.com/index.php/Percent-obscuration-per-foot> ;
  ieso:unitSymbol "% obs/ft"^^rdfs:Literal ;
  .
# !


###  https://www.gecad.isep.ipp.pt/ieso/v1.0.0/PercentObscurationPerMetre
ieso:PercentObscurationPerMetre
  rdf:type
    owl:NamedIndividual ,
    ieso:ObscurationUnit ;
  rdfs:comment "Percent obscuration per meter - Obscuration is any atmospheric phenomenon, except clouds, that restricts vertical visibility (e.g., dust, rain, snow, etc.). Percent obscuration per meter is the unit to measure the amount of Obscuration per meter. This unit is usually used in smoke detectors."@en ;
  rdfs:label "percent obscuration per metre"@en ;
  rdfs:isDefinedBy <measure/v1.0.0/> ;
  rdfs:seeAlso <http://automationwiki.com/index.php/Percent-obscuration-per-metre> ;
  ieso:unitSymbol "% obs/m"^^rdfs:Literal ;
  .
# !


###  https://www.gecad.isep.ipp.pt/ieso/v1.0.0/Phot
ieso:Phot
  rdf:type
    owl:NamedIndividual ,
    ieso:IlluminanceUnit ;
  rdfs:comment "A phot (ph) is a photometric unit of illuminance, or luminous flux through an area. It is not an SI unit, but rather is associated with the older centimetregramsecond system of units."@en ;
  rdfs:label "phot"@en ;
  rdfs:isDefinedBy <measure/v1.0.0/> ;
  rdfs:seeAlso
    <https://en.wikipedia.org/wiki/Conversion_of_units#Illuminance> ,
    <https://en.wikipedia.org/wiki/Phot> ;
  ieso:hasSIUnitOfMeasure ieso:Lux ;
  ieso:conversionCoefficientToSIUnit "1.0e4"^^xsd:double ;
  ieso:conversionOffsetToSIUnit "0.0"^^xsd:double ;
  ieso:unitSymbol "ph"^^rdfs:Literal ;
  .
# !


###  https://www.gecad.isep.ipp.pt/ieso/v1.0.0/PoundSterling
ieso:PoundSterling
  rdf:type
    owl:NamedIndividual ,
    ieso:CurrencyUnit ;
  rdfs:comment "The pound sterling (symbol: ; code: GBP), known in some contexts simply as the pound or sterling, is the official currency of the United Kingdom, Jersey, Guernsey, the Isle of Man, Gibraltar, South Georgia and the South Sandwich Islands, the British Antarctic Territory, and Tristan da Cunha. It is the fourth most-traded currency in the foreign exchange market."@en ;
  rdfs:label "Pound sterling"@en ;
  rdfs:isDefinedBy <measure/v1.0.0/> ;
  rdfs:seeAlso <https://en.wikipedia.org/wiki/Pound_sterling> ;
  ieso:unitCode "GBP"^^rdfs:Literal ;
  ieso:unitSymbol ""^^rdfs:Literal ;
  .
# !


###  https://www.gecad.isep.ipp.pt/ieso/v1.0.0/Radian
ieso:Radian
  rdf:type
    owl:NamedIndividual ,
    ieso:PlaneAngleUnit ;
  rdfs:comment "The radian, denoted by the symbol rad, is the SI unit for measuring angles, and is the standard unit of angular measure used in many areas of mathematics."@en ;
  rdfs:label "radian"@en ;
  rdfs:isDefinedBy <measure/v1.0.0/> ;
  rdfs:seeAlso
    <https://en.wikipedia.org/wiki/Conversion_of_units#Plane_angle> ,
    <https://en.wikipedia.org/wiki/Radian> ;
  ieso:hasSIUnitOfMeasure ieso:Radian ;
  ieso:conversionCoefficientToSIUnit "1.0"^^xsd:double ;
  ieso:conversionOffsetToSIUnit "0.0"^^xsd:double ;
  ieso:unitSymbol "rad"^^rdfs:Literal ;
  .
# !


###  https://www.gecad.isep.ipp.pt/ieso/v1.0.0/Rankine
ieso:Rankine
  rdf:type
    owl:NamedIndividual ,
    ieso:TemperatureUnit ;
  rdfs:comment "The Rankine scale is an absolute scale of thermodynamic temperature named after the Glasgow University engineer and physicist Macquorn Rankine, who proposed it in 1859. The symbol for degrees Rankine is R."@en ;
  rdfs:label "rankine"@en ;
  rdfs:isDefinedBy <measure/v1.0.0/> ;
  rdfs:seeAlso
    <https://en.wikipedia.org/wiki/Conversion_of_units#Temperature> ,
    <https://en.wikipedia.org/wiki/Rankine_scale> ;
  ieso:hasSIUnitOfMeasure ieso:Kelvin ;
  ieso:conversionCoefficientToSIUnit "1.8"^^xsd:double ;
  ieso:conversionOffsetToSIUnit "0.0"^^xsd:double ;
  ieso:unitSymbol "R"^^rdfs:Literal ;
  .
# !


###  https://www.gecad.isep.ipp.pt/ieso/v1.0.0/Second
ieso:Second
  rdf:type
    owl:NamedIndividual ,
    ieso:TimeUnit ;
  rdfs:comment "The second (symbol: s, abbreviation: sec) is the base unit of time in the International System of Units (SI), commonly understood and historically defined as 186400 of a day  this factor derived from the division of the day first into 24 hours, then to 60 minutes and finally to 60 seconds each."@en ;
  rdfs:label "second"@en ;
  rdfs:isDefinedBy <measure/v1.0.0/> ;
  rdfs:seeAlso
    <https://en.wikipedia.org/wiki/Conversion_of_units#Time> ,
    <https://en.wikipedia.org/wiki/Second> ;
  ieso:hasSIUnitOfMeasure ieso:Second ;
  ieso:conversionCoefficientToSIUnit "1.0"^^xsd:double ;
  ieso:conversionOffsetToSIUnit "0.0"^^xsd:double ;
  ieso:unitSymbol "s"^^rdfs:Literal ;
  .
# !


###  https://www.gecad.isep.ipp.pt/ieso/v1.0.0/Siemens
ieso:Siemens
  rdf:type
    owl:NamedIndividual ,
    ieso:ElectricalAdmittanceUnit ,
    ieso:ElectricalConductanceUnit ,
    ieso:ElectricalSusceptanceUnit ;
  rdfs:comment "The siemens (symbol: S) is the derived unit of electric conductance, electric susceptance, and electric admittance in the International System of Units (SI). Conductance, susceptance, and admittance are the reciprocals of resistance, reactance, and impedance respectively; hence one siemens is redundantly equal to the reciprocal of one ohm (1) and is also referred to as the mho."@en ;
  rdfs:label "siemens"@en ;
  rdfs:isDefinedBy <measure/v1.0.0/> ;
  rdfs:seeAlso
    <https://en.wikipedia.org/wiki/Conversion_of_units#Electrical_resistance> ,
    <https://en.wikipedia.org/wiki/Siemens_(unit)> ,
    <https://en.wikipedia.org/wiki/Ohm> ;
  ieso:hasSIUnitOfMeasure ieso:Ohm ;
  ieso:conversionCoefficientToSIUnit "1.0"^^xsd:double ;
  ieso:conversionOffsetToSIUnit "0.0"^^xsd:double ;
  ieso:unitSymbol "S"^^rdfs:Literal ;
  .
# !


###  https://www.gecad.isep.ipp.pt/ieso/v1.0.0/Microsiemens
ieso:Microsiemens
  rdf:type
    owl:NamedIndividual ,
    ieso:ElectricalAdmittanceUnit ,
    ieso:ElectricalConductanceUnit ,
    ieso:ElectricalSusceptanceUnit ;
  rdfs:comment "The microsiemens (symbol: S) is a submultiple of siemens in the order of 10^-6."@en ;
  rdfs:label "microsiemens"@en ;
  rdfs:isDefinedBy <measure/v1.0.0/> ;
  rdfs:seeAlso
    <https://en.wikipedia.org/wiki/Conversion_of_units#Electrical_resistance> ,
    <https://en.wikipedia.org/wiki/Siemens_(unit)> ,
    <https://en.wikipedia.org/wiki/Ohm> ;
  ieso:hasSIUnitOfMeasure ieso:Ohm ;
  ieso:conversionCoefficientToSIUnit "0.000001"^^xsd:double ;
  ieso:conversionOffsetToSIUnit "0.0"^^xsd:double ;
  ieso:unitSymbol "S"^^rdfs:Literal ;
  .
# !


###  https://www.gecad.isep.ipp.pt/ieso/v1.0.0/SPARQLQuerySIUnitConversionTemplate
ieso:SPARQLQuerySIUnitConversionTemplate
  rdf:type
    owl:NamedIndividual ,
    ieso:SIUnitConverterTemplate ;
    rdfs:comment "The 'SPARQL Query SI unit conversion template' individual holds a SPARQL Query conversion template with three tags to be replaced by the respective individuals, namely, MEASUREMENT_INDIVIDUAL, UNIT_INDIVIDUAL_1, and UNIT_INDIVIDUAL_2.\n\nThe MEASUREMENT_INDIVIDUAL tag identifies the 'Measurement' individual that as a 'Measurement value' with unit of measure UNIT_INDIVIDUAL_1. The tag UNIT_INDIVIDUAL_1 is required since it is possible to have a 'Measurement' related to several 'Measurement value'(s) having different units. The tag UNIT_INDIVIDUAL_2 identifies the unit of measure to which we want the value to be converted.\n\nThis query checks if the unit individuals are not the same individual and if the units have the same SI unit of measure; otherwise, it won't make sense to make the conversion. The query result returns the converted value in the '?convertedValue' variable."@en ;
    rdfs:label "SPARQL Query SI unit conversion template"@en ;
  rdfs:isDefinedBy <measure/v1.0.0/> ;
  ieso:conversionTemplateSyntax "SPARQL" ;
  ieso:conversionTemplate "PREFIX  ieso: <https://www.gecad.isep.ipp.pt/ieso/v1.0.0/>\n\nSELECT  ?convertedValue\nWHERE\n  { MEASUREMENT_INDIVIDUAL\n        a           ieso:Measurement ;\n        ieso:hasMeasurementValue  ?mv .\n  ?mv     a           ieso:MeasurementValue ;\n        ieso:hasLiteralValue  ?mvValue ;\n        ieso:hasUnitOfMeasure  UNIT_INDIVIDUAL_1 .\n  UNIT_INDIVIDUAL_1  ieso:conversionCoefficientToSIUnit  ?mvUnitCoefficient ;\n        ieso:conversionOffsetToSIUnit  ?mvUnitOffset ;\n        ieso:hasSIUnitOfMeasure  ?SI .\n  UNIT_INDIVIDUAL_2\n        ieso:conversionCoefficientToSIUnit  ?umCoefficient ;\n        ieso:conversionOffsetToSIUnit  ?umOffset ;\n        ieso:hasSIUnitOfMeasure  ?SI\n  FILTER( UNIT_INDIVIDUAL_1 != UNIT_INDIVIDUAL_2 )\n  BIND(( ( ( ( ?mvValue + ?mvUnitOffset ) * ?mvUnitCoefficient ) / ?umCoefficient ) - ?umOffset ) AS ?convertedValue)\n  }"^^xsd:string ;
  .
# !


###  https://www.gecad.isep.ipp.pt/ieso/v1.0.0/SPARQLUpdateSIUnitConversionTemplate
ieso:SPARQLUpdateSIUnitConversionTemplate
  rdf:type
    owl:NamedIndividual ,
    ieso:SIUnitConverterTemplate ;
    rdfs:comment "The 'SPARQL Update SI unit conversion template' individual holds a SPARQL Update conversion template to add a new 'Measurement value' to the given 'Measurement' individual. It holds four tags, namely, 'MEASUREMENT_VALUE_INDIVIDUAL', MEASUREMENT_INDIVIDUAL, UNIT_INDIVIDUAL_1, and UNIT_INDIVIDUAL_2.\n\nThe 'MEASUREMENT_VALUE_INDIVIDUAL' identifies the new 'Measurement value' individual to add to the 'Measurement' individual identified by the MEASUREMENT_INDIVIDUAL tag. The MEASUREMENT_INDIVIDUAL tag identifies the 'Measurement' individual that as a 'Measurement value' with unit of measure UNIT_INDIVIDUAL_1. The tag UNIT_INDIVIDUAL_1 is required since it is possible to have a 'Measurement' related to several 'Measurement value'(s) having different units. The tag UNIT_INDIVIDUAL_2 identifies the unit of measure to which we want the value to be converted.\n\nThis update checks if the unit individuals are not the same individual and if the units have the same SI unit of measure; otherwise, it won't make sense to make the conversion nor add the new measurement value. The update result adds the converted value to the respective measurement."@en ;
    rdfs:label "SPARQL Update SI unit conversion template"@en ;
  rdfs:isDefinedBy <measure/v1.0.0/> ;
  ieso:conversionTemplateSyntax "SPARQL" ;
  ieso:conversionTemplate "PREFIX  ieso: <https://www.gecad.isep.ipp.pt/ieso/v1.0.0/>\n\nINSERT {\n  MEASUREMENT_VALUE_INDIVIDUAL a ieso:MeasurementValue .\n  MEASUREMENT_VALUE_INDIVIDUAL ieso:hasUnitOfMeasure UNIT_INDIVIDUAL_2 .\n  MEASUREMENT_VALUE_INDIVIDUAL ieso:hasLiteralValue ?convertedValue .\n  MEASUREMENT_INDIVIDUAL ieso:hasMeasurementValue MEASUREMENT_VALUE_INDIVIDUAL .\n}\nWHERE\n  { MEASUREMENT_INDIVIDUAL\n        a           ieso:Measurement ;\n        ieso:hasMeasurementValue  ?mv .\n  ?mv     a           ieso:MeasurementValue ;\n        ieso:hasLiteralValue  ?mvValue ;\n        ieso:hasUnitOfMeasure  UNIT_INDIVIDUAL_1 .\n  UNIT_INDIVIDUAL_1  ieso:conversionCoefficientToSIUnit  ?mvUnitCoefficient ;\n        ieso:conversionOffsetToSIUnit  ?mvUnitOffset ;\n        ieso:hasSIUnitOfMeasure  ?SI .\n  UNIT_INDIVIDUAL_2\n        ieso:conversionCoefficientToSIUnit  ?umCoefficient ;\n        ieso:conversionOffsetToSIUnit  ?umOffset ;\n        ieso:hasSIUnitOfMeasure  ?SI\n  FILTER ( UNIT_INDIVIDUAL_1 != UNIT_INDIVIDUAL_2 )\n  BIND(( ( ( ( ?mvValue + ?mvUnitOffset ) * ?mvUnitCoefficient ) / ?umCoefficient ) - ?umOffset ) AS ?convertedValue)\n  }"^^xsd:string ;
  .
# !


###  https://www.gecad.isep.ipp.pt/ieso/v1.0.0/SquareCentimetre
ieso:SquareCentimetre
  rdf:type
    owl:NamedIndividual ,
    ieso:AreaUnit ;
  rdfs:comment "The square centimetre (international spelling as used by the International Bureau of Weights and Measures) or square centimeter (American spelling) is the SI derived unit of area with symbol cm^2."@en ;
  rdfs:label "square centimetre"@en ;
  rdfs:isDefinedBy <measure/v1.0.0/> ;
  rdfs:seeAlso <https://en.wikipedia.org/wiki/Square_metre#SI_prefixes_applied> ;
  ieso:hasSIUnitOfMeasure ieso:SquareMetre ;
  ieso:conversionCoefficientToSIUnit "1.0e-4"^^xsd:double ;
  ieso:conversionOffsetToSIUnit "0.0"^^xsd:double ;
  ieso:unitSymbol "cm^2"^^rdfs:Literal ;
  .
# !


###  https://www.gecad.isep.ipp.pt/ieso/v1.0.0/SquareDecametre
ieso:SquareDecametre
  rdf:type
    owl:NamedIndividual ,
    ieso:AreaUnit ;
  rdfs:comment "The square decametre (international spelling as used by the International Bureau of Weights and Measures) or square decameter (American spelling) is the SI derived unit of area with symbol dam^2."@en ;
  rdfs:label "square decametre (are)"@en ;
  rdfs:isDefinedBy <measure/v1.0.0/> ;
  rdfs:seeAlso <https://en.wikipedia.org/wiki/Square_metre#SI_prefixes_applied> ;
  ieso:hasSIUnitOfMeasure ieso:SquareMetre ;
  ieso:conversionCoefficientToSIUnit "1.0e2"^^xsd:double ;
  ieso:conversionOffsetToSIUnit "0.0"^^xsd:double ;
  ieso:unitSymbol "dam^2"^^rdfs:Literal ;
  .
# !


###  https://www.gecad.isep.ipp.pt/ieso/v1.0.0/SquareDecimetre
ieso:SquareDecimetre
  rdf:type
    owl:NamedIndividual ,
    ieso:AreaUnit ;
  rdfs:comment "The square decimetre (international spelling as used by the International Bureau of Weights and Measures) or square decimeter (American spelling) is the SI derived unit of area with symbol dm^2."@en ;
  rdfs:label "square decimetre"@en ;
  rdfs:isDefinedBy <measure/v1.0.0/> ;
  rdfs:seeAlso <https://en.wikipedia.org/wiki/Square_metre#SI_prefixes_applied> ;
  ieso:hasSIUnitOfMeasure ieso:SquareMetre ;
  ieso:conversionCoefficientToSIUnit "1.0e-2"^^xsd:double ;
  ieso:conversionOffsetToSIUnit "0.0"^^xsd:double ;
  ieso:unitSymbol "dm^2"^^rdfs:Literal ;
  .
# !


###  https://www.gecad.isep.ipp.pt/ieso/v1.0.0/SquareDegree
ieso:SquareDegree
  rdf:type
    owl:NamedIndividual ,
    ieso:SolidAngleUnit ;
  rdfs:comment "A square degree (deg^2) is a non-SI unit measure of solid angle. Just as degrees are used to measure parts of a circle, square degrees are used to measure parts of a sphere."@en ;
  rdfs:label "square degree"@en ;
  rdfs:isDefinedBy <measure/v1.0.0/> ;
  rdfs:seeAlso
    <https://en.wikipedia.org/wiki/Conversion_of_units#Solid_angle> ,
    <https://en.wikipedia.org/wiki/Square_degree> ;
  ieso:hasSIUnitOfMeasure ieso:Steradian ;
  ieso:conversionCoefficientToSIUnit "0.30461742e-3"^^xsd:double ;
  ieso:conversionOffsetToSIUnit "0.0"^^xsd:double ;
  ieso:unitSymbol "deg^2"^^rdfs:Literal ;
  .
# !


###  https://www.gecad.isep.ipp.pt/ieso/v1.0.0/SquareHectometre
ieso:SquareHectometre
  rdf:type
    owl:NamedIndividual ,
    ieso:AreaUnit ;
  rdfs:comment "The square hectometre (international spelling as used by the International Bureau of Weights and Measures) or square hectometer (American spelling) is the SI derived unit of area with symbol hm^2."@en ;
  rdfs:label "square hectometre (hectare)"@en ;
  rdfs:isDefinedBy <measure/v1.0.0/> ;
  rdfs:seeAlso <https://en.wikipedia.org/wiki/Square_metre#SI_prefixes_applied> ;
  ieso:hasSIUnitOfMeasure ieso:SquareMetre ;
  ieso:conversionCoefficientToSIUnit "1.0e4"^^xsd:double ;
  ieso:conversionOffsetToSIUnit "0.0"^^xsd:double ;
  ieso:unitSymbol "hm^2"^^rdfs:Literal ;
  .
# !


###  https://www.gecad.isep.ipp.pt/ieso/v1.0.0/SquareKilometre
ieso:SquareKilometre
  rdf:type
    owl:NamedIndividual ,
    ieso:AreaUnit ;
  rdfs:comment "The square kilometre (international spelling as used by the International Bureau of Weights and Measures) or square kilometer (American spelling) is the SI derived unit of area with symbol km^2."@en ;
  rdfs:label "square kilometre"@en ;
  rdfs:isDefinedBy <measure/v1.0.0/> ;
  rdfs:seeAlso <https://en.wikipedia.org/wiki/Square_metre#SI_prefixes_applied> ;
  ieso:hasSIUnitOfMeasure ieso:SquareMetre ;
  ieso:conversionCoefficientToSIUnit "1.0e6"^^xsd:double ;
  ieso:conversionOffsetToSIUnit "0.0"^^xsd:double ;
  ieso:unitSymbol "km^2"^^rdfs:Literal ;
  .
# !


###  https://www.gecad.isep.ipp.pt/ieso/v1.0.0/SquareMetre
ieso:SquareMetre
  rdf:type
    owl:NamedIndividual ,
    ieso:AreaUnit ;
  rdfs:comment "The square metre (international spelling as used by the International Bureau of Weights and Measures) or square meter (American spelling) is the SI derived unit of area with symbol m^2."@en ;
  rdfs:label "square metre"@en ;
  rdfs:isDefinedBy <measure/v1.0.0/> ;
  rdfs:seeAlso <https://en.wikipedia.org/wiki/Square_metre> ;
  ieso:hasSIUnitOfMeasure ieso:SquareMetre ;
  ieso:conversionCoefficientToSIUnit "1.0"^^xsd:double ;
  ieso:conversionOffsetToSIUnit "0.0"^^xsd:double ;
  ieso:unitSymbol "m^2"^^rdfs:Literal ;
  .
# !


###  https://www.gecad.isep.ipp.pt/ieso/v1.0.0/SquareMillimetre
ieso:SquareMillimetre
  rdf:type
    owl:NamedIndividual ,
    ieso:AreaUnit ;
  rdfs:comment "The square millimetre (international spelling as used by the International Bureau of Weights and Measures) or square millimeter (American spelling) is the SI derived unit of area with symbol mm^2."@en ;
  rdfs:label "square millimetre"@en ;
  rdfs:isDefinedBy <measure/v1.0.0/> ;
  rdfs:seeAlso <https://en.wikipedia.org/wiki/Square_metre#SI_prefixes_applied> ;
  ieso:hasSIUnitOfMeasure ieso:SquareMetre ;
  ieso:conversionCoefficientToSIUnit "1.0e-6"^^xsd:double ;
  ieso:conversionOffsetToSIUnit "0.0"^^xsd:double ;
  ieso:unitSymbol "mm^2"^^rdfs:Literal ;
  .
# !


###  https://www.gecad.isep.ipp.pt/ieso/v1.0.0/SQWRLQuerySIUnitConversionTemplate
ieso:SQWRLQuerySIUnitConversionTemplate
  rdf:type
    owl:NamedIndividual ,
    ieso:SIUnitConverterTemplate ;
    rdfs:comment "The 'SQWRL Query SI unit conversion template' individual holds a SQWRL conversion template with three tags to be replaced by the respective individuals, namely, MEASUREMENT_INDIVIDUAL, UNIT_INDIVIDUAL_1, and UNIT_INDIVIDUAL_2.\n\nThe MEASUREMENT_INDIVIDUAL tag identifies the 'Measurement' individual that as a 'Measurement value' with unit of measure UNIT_INDIVIDUAL_1. The tag UNIT_INDIVIDUAL_1 is required since it is possible to have a 'Measurement' related to several 'Measurement value'(s) having different units. The tag UNIT_INDIVIDUAL_2 identifies the unit of measure to which we want the value to be converted.\n\nThis query checks if the units have the same SI unit of measure; otherwise, it won't make sense to make the conversion. The query result returns the converted value in the '?convertedValue' variable."@en ;
    rdfs:label "SQWRL Query SI unit conversion template"@en ;
  rdfs:isDefinedBy <measure/v1.0.0/> ;
  ieso:conversionTemplateSyntax "SQWRL" ;
  ieso:conversionTemplate """ieso:Measurement(MEASUREMENT_INDIVIDUAL)\n ^ ieso:hasMeasurementValue(MEASUREMENT_INDIVIDUAL, ?mv)\n ^ ieso:MeasurementValue(?mv)\n ^ ieso:hasLiteralValue(?mv, ?mvValue)\n ^ ieso:hasUnitOfMeasure(?mv, UNIT_INDIVIDUAL_1)\n ^ ieso:conversionOffsetToSIUnit(UNIT_INDIVIDUAL_1, ?mvUnitOffset)\n ^ ieso:conversionCoefficientToSIUnit(UNIT_INDIVIDUAL_1, ?mvUnitCoefficient)\n ^ ieso:hasSIUnitOfMeasure(UNIT_INDIVIDUAL_1, ?SI)\n ^ ieso:hasSIUnitOfMeasure(UNIT_INDIVIDUAL_2, ?SI)\n ^ ieso:UnitOfMeasure(UNIT_INDIVIDUAL_2)\n ^ ieso:conversionCoefficientToSIUnit(UNIT_INDIVIDUAL_2, ?umCoefficient)\n ^ ieso:conversionOffsetToSIUnit(UNIT_INDIVIDUAL_2, ?umOffset)\n ^ swrlb:add(?sum, ?mvValue, ?mvUnitOffset)\n ^ swrlb:multiply(?mul, ?sum, ?mvUnitCoefficient)\n ^ swrlb:divide(?div, ?mul, ?umCoefficient)\n ^ swrlb:subtract(?convertedValue, ?div, ?umOffset)\n->\n sqwrl:select(?convertedValue)"""^^xsd:string ;
  .
# !


###  https://www.gecad.isep.ipp.pt/ieso/v1.0.0/Statvolt
ieso:Statvolt
  rdf:type
    owl:NamedIndividual ,
    ieso:VoltageUnit ;
  rdfs:comment "The statvolt is a unit of voltage and electrical potential used in the CGS-ESU and gaussian systems of units. It is a useful unit for electromagnetism because, in a vacuum, an electric field of one statvolt per centimetre has the same energy density as a magnetic field of one gauss."@en ;
  rdfs:label "statvolt"@en ;
  rdfs:isDefinedBy <measure/v1.0.0/> ;
  rdfs:seeAlso
    <https://en.wikipedia.org/wiki/Conversion_of_units#Electromotive_force,_electric_potential_difference> ,
    <https://en.wikipedia.org/wiki/Statvolt> ;
  ieso:hasSIUnitOfMeasure ieso:Volt ;
  ieso:conversionCoefficientToSIUnit "2.99792458e2"^^xsd:double ;
  ieso:conversionOffsetToSIUnit "0.0"^^xsd:double ;
  ieso:unitSymbol "statV"^^rdfs:Literal ;
  .
# !


###  https://www.gecad.isep.ipp.pt/ieso/v1.0.0/Steradian
ieso:Steradian
  rdf:type
    owl:NamedIndividual ,
    ieso:SolidAngleUnit ;
  rdfs:comment "The steradian (symbol: sr) or square radian is the SI unit of solid angle. It is used in three-dimensional geometry, and is analogous to the radian, which quantifies planar angles. Whereas an angle in radians, projected onto a circle, gives a length on the circumference, a solid angle in steradians, projected onto a sphere, gives an area on the surface."@en ;
  rdfs:label "steradian"@en ;
  rdfs:isDefinedBy <measure/v1.0.0/> ;
  rdfs:seeAlso
    <https://en.wikipedia.org/wiki/Conversion_of_units#Solid_angle> ,
    <https://en.wikipedia.org/wiki/Steradian> ;
  ieso:hasSIUnitOfMeasure ieso:Steradian ;
  ieso:conversionCoefficientToSIUnit "1.0"^^xsd:double ;
  ieso:conversionOffsetToSIUnit "0.0"^^xsd:double ;
  ieso:unitSymbol "sr"^^rdfs:Literal ;
  .
# !


###  https://www.gecad.isep.ipp.pt/ieso/v1.0.0/Stilb
ieso:Stilb
  rdf:type
    owl:NamedIndividual ,
    ieso:LuminanceUnit ;
  rdfs:comment "The stilb (sb) is the CGS unit of luminance for objects that are not self-luminous. It is equal to one candela per square centimeter or 104 nits (candelas per square meter)."@en ;
  rdfs:label "stilb"@en ;
  rdfs:isDefinedBy <measure/v1.0.0/> ;
  rdfs:seeAlso
    <https://en.wikipedia.org/wiki/Conversion_of_units#Luminance> ,
    <https://en.wikipedia.org/wiki/Stilb_(unit)> ;
  ieso:hasSIUnitOfMeasure ieso:CandelaPerSquareMetre ;
  ieso:conversionCoefficientToSIUnit "1.0e4"^^xsd:double ;
  ieso:conversionOffsetToSIUnit "0.0"^^xsd:double ;
  ieso:unitSymbol "L"^^rdfs:Literal ;
  .
# !


###  https://www.gecad.isep.ipp.pt/ieso/v1.0.0/Terahertz
ieso:Terahertz
  rdf:type
    owl:NamedIndividual ,
    ieso:FrequencyUnit ;
  rdfs:comment "The terahertz (symbol: THz) is the derived unit of frequency in the International System of Units (SI) and is defined as one thousand gigahertz."@en ;
  rdfs:label "terahertz"@en ;
  rdfs:isDefinedBy <measure/v1.0.0/> ;
  rdfs:seeAlso <https://en.wikipedia.org/wiki/Hertz#SI_multiples> ;
  ieso:hasSIUnitOfMeasure ieso:Hertz ;
  ieso:conversionCoefficientToSIUnit "1.0e12"^^xsd:double ;
  ieso:conversionOffsetToSIUnit "0.0"^^xsd:double ;
  ieso:unitSymbol "THz"^^rdfs:Literal ;
  .
# !


###  https://www.gecad.isep.ipp.pt/ieso/v1.0.0/Terawatt
ieso:Terawatt
  rdf:type
    owl:NamedIndividual ,
    ieso:PowerUnit ,
    ieso:ElectricPowerUnit ;
  rdfs:comment "The terawatt (TW) is equal to one thousand gigawatts. The total power used by humans worldwide is commonly measured in terawatts."@en ;
  rdfs:label "terawatt"@en ;
  rdfs:isDefinedBy <measure/v1.0.0/> ;
  rdfs:seeAlso
    <https://en.wikipedia.org/wiki/Conversion_of_units#Power_or_heat_flow_rate> ,
    <https://en.wikipedia.org/wiki/Watt#Terawatt> ;
  ieso:hasSIUnitOfMeasure ieso:Watt ;
  ieso:conversionCoefficientToSIUnit "1.0e12"^^xsd:double ;
  ieso:conversionOffsetToSIUnit "0.0"^^xsd:double ;
  ieso:unitSymbol "TW"^^rdfs:Literal ;
  .
# !


###  https://www.gecad.isep.ipp.pt/ieso/v1.0.0/UnitedStatesDollar
ieso:UnitedStatesDollar
  rdf:type
    owl:NamedIndividual ,
    ieso:CurrencyUnit ;
  rdfs:comment "The United States dollar (symbol: $; code: USD; also abbreviated US$ or U.S. Dollar, to distinguish it from other dollar-denominated currencies; referred to as the dollar, U.S. dollar, or American dollar) is the official currency of the United States."@en ;
  rdfs:label "United States dollar"@en ;
  rdfs:isDefinedBy <measure/v1.0.0/> ;
  rdfs:seeAlso <https://en.wikipedia.org/wiki/United_States_dollar> ;
  ieso:unitCode "USD"^^rdfs:Literal ;
  ieso:unitSymbol "$"^^rdfs:Literal ;
  .
# !


###  https://www.gecad.isep.ipp.pt/ieso/v1.0.0/Volt
ieso:Volt
  rdf:type
    owl:NamedIndividual ,
    ieso:VoltageUnit ;
  rdfs:comment "The volt (symbol: V) is the derived unit for electric potential, electric potential difference (voltage), and electromotive force."@en ;
  rdfs:label "volt"@en ;
  rdfs:isDefinedBy <measure/v1.0.0/> ;
  rdfs:seeAlso
    <https://en.wikipedia.org/wiki/Conversion_of_units#Electromotive_force,_electric_potential_difference> ,
    <https://en.wikipedia.org/wiki/Voltage#Volt> ,
    <https://en.wikipedia.org/wiki/Volt> ;
  ieso:hasSIUnitOfMeasure ieso:Volt ;
  ieso:conversionCoefficientToSIUnit "1.0"^^xsd:double ;
  ieso:conversionOffsetToSIUnit "0.0"^^xsd:double ;
  ieso:unitSymbol "V"^^rdfs:Literal ;
  .
# !


###  https://www.gecad.isep.ipp.pt/ieso/v1.0.0/Volt-ampere
ieso:Volt-ampere
  rdf:type
    owl:NamedIndividual ,
    ieso:PowerUnit ;
  rdfs:comment "A volt-ampere (SI symbol: VA or V A; also VA) is the unit used for the apparent power in an electrical circuit. The apparent power equals the product of root mean square voltage and root mean square current. In direct current (DC) circuits, this product is equal to the real power in watts. Volt-amperes are usually used for analyzing alternating current (AC) circuits. The volt-ampere is dimensionally equivalent to the watt (in SI units, 1 VA = 1 W). VA rating is most useful in rating wires and switches (and other power handling equipment) for inductive loads."@en ;
  rdfs:label "volt-ampere"@en ;
  rdfs:isDefinedBy <measure/v1.0.0/> ;
  rdfs:seeAlso <https://en.wikipedia.org/wiki/Volt-ampere> ;
  ieso:hasSIUnitOfMeasure ieso:Volt-ampere ;
  ieso:conversionCoefficientToSIUnit "1.0"^^xsd:double ;
  ieso:conversionOffsetToSIUnit "0.0"^^xsd:double ;
  ieso:unitSymbol "VA"^^rdfs:Literal ;
  .
# !


###  https://www.gecad.isep.ipp.pt/ieso/v1.0.0/Kilovolt-ampere
ieso:Kilovolt-ampere
  rdf:type
    owl:NamedIndividual ,
    ieso:PowerUnit ;
  rdfs:comment "A kilovolt-ampere (SI symbol: kVA or kV A; also kVA) is a multiple of volt-ampere in the order of magnitude 10^3."@en ;
  rdfs:label "kilovolt-ampere"@en ;
  rdfs:isDefinedBy <measure/v1.0.0/> ;
  rdfs:seeAlso <https://en.wikipedia.org/wiki/Volt-ampere> ;
  ieso:hasSIUnitOfMeasure ieso:Volt-ampere ;
  ieso:conversionCoefficientToSIUnit "1000.0"^^xsd:double ;
  ieso:conversionOffsetToSIUnit "0.0"^^xsd:double ;
  ieso:unitSymbol "kVA"^^rdfs:Literal ;
  .
# !


###  https://www.gecad.isep.ipp.pt/ieso/v1.0.0/Megavolt-ampere
ieso:Megavolt-ampere
  rdf:type
    owl:NamedIndividual ,
    ieso:PowerUnit ;
  rdfs:comment "A megavolt-ampere (SI symbol: MVA or MV A; also MVA) is a multiple of volt-ampere in the order of magnitude 10^6."@en ;
  rdfs:label "megavolt-ampere"@en ;
  rdfs:isDefinedBy <measure/v1.0.0/> ;
  rdfs:seeAlso <https://en.wikipedia.org/wiki/Volt-ampere> ;
  ieso:hasSIUnitOfMeasure ieso:Volt-ampere ;
  ieso:conversionCoefficientToSIUnit "1000000.0"^^xsd:double ;
  ieso:conversionOffsetToSIUnit "0.0"^^xsd:double ;
  ieso:unitSymbol "MVA"^^rdfs:Literal ;
  .
# !


###  https://www.gecad.isep.ipp.pt/ieso/v1.0.0/Volt-ampereReactive
ieso:Volt-ampereReactive
  rdf:type
    owl:NamedIndividual ,
    ieso:PowerUnit ;
  rdfs:comment "A volt-ampere reactive (SI symbol: VAr or V Ar; also VAr) is a the unit used for the reactive power in an electrical circuit."@en ;
  rdfs:label "volt-ampere reactive"@en ;
  rdfs:isDefinedBy <measure/v1.0.0/> ;
  rdfs:seeAlso <https://en.wikipedia.org/wiki/Volt-ampere> ;
  ieso:hasSIUnitOfMeasure ieso:Volt-ampereReactive ;
  ieso:conversionCoefficientToSIUnit "1.0"^^xsd:double ;
  ieso:conversionOffsetToSIUnit "0.0"^^xsd:double ;
  ieso:unitSymbol "VAr"^^rdfs:Literal ;
  .
# !


###  https://www.gecad.isep.ipp.pt/ieso/v1.0.0/Megavolt-ampereReactive
ieso:Megavolt-ampereReactive
  rdf:type
    owl:NamedIndividual ,
    ieso:PowerUnit ;
  rdfs:comment "A megavolt-ampere reactive (SI symbol: MVAr or MV Ar; also MVAr) is a multiple of volt-ampere reactive in the order of magnitude 10^6."@en ;
  rdfs:label "megavolt-ampere reactive"@en ;
  rdfs:isDefinedBy <measure/v1.0.0/> ;
  rdfs:seeAlso <https://en.wikipedia.org/wiki/Volt-ampere> ;
  ieso:hasSIUnitOfMeasure ieso:Volt-ampereReactive ;
  ieso:conversionCoefficientToSIUnit "1000000.0"^^xsd:double ;
  ieso:conversionOffsetToSIUnit "0.0"^^xsd:double ;
  ieso:unitSymbol "MVAr"^^rdfs:Literal ;
  .
# !


###  https://www.gecad.isep.ipp.pt/ieso/v1.0.0/Watt
ieso:Watt
  rdf:type
    owl:NamedIndividual ,
    ieso:PowerUnit ,
    ieso:ElectricPowerUnit ;
  rdfs:comment "The watt (symbol: W) is a unit of power or radiant flux. In the International System of Units (SI), it is defined as a derived unit of (in SI base units) 1 kgm2s3 or, equivalently, 1 joule per second. It is used to quantify the rate of energy transfer."@en ;
  rdfs:label "watt"@en ;
  rdfs:isDefinedBy <measure/v1.0.0/> ;
  rdfs:seeAlso
    <https://en.wikipedia.org/wiki/Conversion_of_units#Power_or_heat_flow_rate> ,
    <https://en.wikipedia.org/wiki/Watt> ;
  ieso:hasSIUnitOfMeasure ieso:Watt ;
  ieso:conversionCoefficientToSIUnit "1.0"^^xsd:double ;
  ieso:conversionOffsetToSIUnit "0.0"^^xsd:double ;
  ieso:unitSymbol "W"^^rdfs:Literal ;
  .
# !


###  https://www.gecad.isep.ipp.pt/ieso/v1.0.0/WattHour
ieso:WattHour
  rdf:type
    owl:NamedIndividual ,
    ieso:EnergyUnit ,
    ieso:ElectricEnergyUnit ;
  rdfs:comment "The watt-hour (SI symbol: Wh or W h; commonly written as Wh) is a unit of energy equal to 3600 joules (3.6 kilojoules)."@en ;
  rdfs:label "watt hour"@en ;
  rdfs:isDefinedBy <measure/v1.0.0/> ;
  rdfs:seeAlso
    <https://en.wikipedia.org/wiki/Conversion_of_units#Energy> ,
    <https://en.wikipedia.org/wiki/Watt_hour>  ;
  ieso:hasSIUnitOfMeasure ieso:Joule ;
  ieso:conversionCoefficientToSIUnit "3.6e3"^^xsd:double ;
  ieso:conversionOffsetToSIUnit "0.0"^^xsd:double ;
  ieso:unitSymbol "Wh"^^rdfs:Literal ;
  .
# !


###  https://www.gecad.isep.ipp.pt/ieso/v1.0.0/WattPerSquareMetre
ieso:WattPerSquareMetre
  rdf:type
    owl:NamedIndividual ,
    ieso:IrradianceUnit ;
  rdfs:comment "The watt per square metre is a unit of irradiance defined as the power received per area. This is a unit in the category of Energy flux. This is sometimes also confusingly called 'intensity'."@en ;
  rdfs:label "watt per square metre"@en ;
  rdfs:isDefinedBy <measure/v1.0.0/> ;
  rdfs:seeAlso
    <https://en.wikipedia.org/wiki/Light#Units_and_measures> ,
    <https://en.wikipedia.org/wiki/Irradiance#SI_radiometry_units> ;
  ieso:hasSIUnitOfMeasure ieso:Watt ;
  ieso:conversionCoefficientToSIUnit "1.0"^^xsd:double ;
  ieso:conversionOffsetToSIUnit "0.0"^^xsd:double ;
  ieso:unitSymbol "W/m^2"^^rdfs:Literal ;
  .
# !


###  https://www.gecad.isep.ipp.pt/ieso/v1.0.0/WattSecond
ieso:WattSecond
  rdf:type
    owl:NamedIndividual ,
    ieso:EnergyUnit ,
    ieso:ElectricEnergyUnit ;
  rdfs:comment "The watt-second (SI symbol: Ws or W s; commonly written as Ws) is a unit of energy equal to 1 joule."@en ;
  rdfs:label "watt second"@en ;
  rdfs:isDefinedBy <measure/v1.0.0/> ;
  rdfs:seeAlso
    <https://en.wikipedia.org/wiki/Conversion_of_units#Energy> ,
    <https://en.wikipedia.org/wiki/Watt_second>  ;
  ieso:hasSIUnitOfMeasure ieso:Joule ;
  ieso:conversionCoefficientToSIUnit "1.0"^^xsd:double ;
  ieso:conversionOffsetToSIUnit "0.0"^^xsd:double ;
  ieso:unitSymbol "Ws"^^rdfs:Literal ;
  .
# !


###  https://www.gecad.isep.ipp.pt/ieso/v1.0.0/Week
ieso:Week
  rdf:type
    owl:NamedIndividual ,
    ieso:TimeUnit ;
  rdfs:comment "A week is a time unit equal to seven days. It is the standard time period used for cycles of rest days in most parts of the world, mostly alongside  although not strictly part of  the Gregorian calendar."@en ;
  rdfs:label "week"@en ;
  rdfs:isDefinedBy <measure/v1.0.0/> ;
  rdfs:seeAlso
    <https://en.wikipedia.org/wiki/Conversion_of_units#Time> ,
    <https://en.wikipedia.org/wiki/Week> ;
  ieso:hasSIUnitOfMeasure ieso:Second ;
  ieso:conversionCoefficientToSIUnit "6.048e5"^^xsd:double ;
  ieso:conversionOffsetToSIUnit "0.0"^^xsd:double ;
  ieso:unitSymbol "wk"^^rdfs:Literal ;
  .
# !


###  https://www.gecad.isep.ipp.pt/ieso/v1.0.0/Year
ieso:Year
  rdf:type
    owl:NamedIndividual ,
    ieso:TimeUnit ;
  rdfs:comment "A year is the orbital period of a planetary body, for example, the Earth, moving in its orbit around the Sun. In astronomy, the Julian year is a unit of time; it is defined as 365.25 days of exactly 86400 seconds (SI base unit), totalling exactly 31557600 seconds in the Julian astronomical year."@en ;
  rdfs:label "year (Julian)"@en ;
  rdfs:isDefinedBy <measure/v1.0.0/> ;
  rdfs:seeAlso
    <https://en.wikipedia.org/wiki/Conversion_of_units#Time> ,
    <https://en.wikipedia.org/wiki/Year> ;
  ieso:hasSIUnitOfMeasure ieso:Second ;
  ieso:conversionCoefficientToSIUnit "3.15576e7"^^xsd:double ;
  ieso:conversionOffsetToSIUnit "0.0"^^xsd:double ;
  ieso:unitSymbol "a"^^rdfs:Literal ;
  .
# !


#################################################################
#  General axioms
#################################################################


###  owl:Thing Level
[
  rdf:type owl:AllDisjointClasses ;
  owl:members (
    ieso:Measurement
    ieso:MeasurementValue
    ieso:TypeOfMeasure
    ieso:UnitOfMeasure
  )
] .
# !